Rename clos_inlineXX theories to clos_knownXX

compiler/backend/proofs/clos_knownProofScript.sml
@@ -1,220 +1,23 @@
-open preamble
-open closPropsTheory clos_knownTheory closSemTheory
-open clos_knownPropsTheory
+open preamble backendPropsTheory
+open closPropsTheory clos_knownTheory clos_knownPropsTheory closSemTheory
 open bagTheory
+open mp_then
+open closLangTheory
 
 val _ = new_theory "clos_knownProof";
 
-val value_CASES = TypeBase.nchotomy_of ``:closSem$v``
-val v_case_eq =
-    prove_case_eq_thm{case_def = TypeBase.case_def_of ``:closSem$v``,
-                      nchotomy = value_CASES}
-
-val ref_CASES = TypeBase.nchotomy_of ``:α closSem$ref``
-
-val va_case_eq =
-    prove_case_eq_thm{case_def = TypeBase.case_def_of ``:val_approx``,
-                      nchotomy = TypeBase.nchotomy_of ``:val_approx``}
-val result_ty = ``:(α,β)semanticPrimitives$result``
-val result_CASES = TypeBase.nchotomy_of result_ty
-val result_case_eq =
-    prove_case_eq_thm{case_def = TypeBase.case_def_of result_ty,
-                      nchotomy = result_CASES}
-val error_ty = ``:α semanticPrimitives$error_result``
-val error_CASES = TypeBase.nchotomy_of error_ty
-val error_case_eq =
-    prove_case_eq_thm{case_def = TypeBase.case_def_of error_ty,
-                      nchotomy = error_CASES}
-
-(* TODO: MOVE candidates *)
-fun sel_ihpc f = first_x_assum (first_assum o mp_then (Pos f) mp_tac)
-fun resolve_selected f th = first_assum (mp_then (Pos f) mp_tac th)
-
 fun patresolve p f th = Q.PAT_ASSUM p (mp_then (Pos f) mp_tac th)
+fun say0 pfx s g = (print (pfx ^ ": " ^ s ^ "\n"); ALL_TAC g)
 
 (* repeated resolution, requiring that all preconditions get removed *)
-fun nailIHx k = first_x_assum (drule_all_then k)
+fun nailIHx k =
+  first_x_assum
+    (REPEAT_GTCL
+       (fn ttcl => fn th => first_assum (mp_then (Pos hd) ttcl th))
+       (k o assert (not o is_imp o #2 o strip_forall o concl)) o
+     assert (is_imp o #2 o strip_forall o concl))
 
-infix >~
-fun (f >~ g) th = f th >> g
-
-(* unused *)
-(* val evaluate_list_members_individually = Q.store_thm( *)
-(*   "evaluate_list_members_individually", *)
-(*   `∀es env (s0:'a closSem$state) vs s. *)
-(*      closSem$evaluate (es, env, s0) = (Rval vs, s) ⇒ *)
-(*      ∀n. n < LENGTH es ⇒ *)
-(*          ∃(s0':'a closSem$state) s'. *)
-(*            evaluate([EL n es], env, s0') = (Rval [EL n vs], s')`, *)
-(*   Induct >> simp[] >> Cases_on `es` >> fs[] *)
-(*   >- (rpt strip_tac >> rename1 `evaluate ([exp], env, _)` >> *)
-(*       `∃v. vs = [v]` by metis_tac[evaluate_SING] >> rw[] >> metis_tac[]) >> *)
-(*   dsimp[evaluate_def, pair_case_eq, result_case_eq] >> *)
-(*   rpt strip_tac >> reverse (Cases_on `n` >> fs[]) >- metis_tac[] >> *)
-(*   imp_res_tac evaluate_SING >> rw[] >> metis_tac[]); *)
-
-(* TODO: MOVE-HOL candidate; unused here *)
-val union_idem = Q.store_thm(
-  "union_idem[simp]",
-  `∀spt. union spt spt = spt`,
-  Induct >> simp[union_def]);
-
-(* simple properties of constants from clos_known: i.e., merge and known *)
-val known_op_changed_globals = Q.store_thm(
-  "known_op_changed_globals",
-  `∀opn as g0 a g.
-     known_op opn as g0 = (a,g) ⇒
-     ∀i. i ∈ domain g ∧ (i ∈ domain g0 ⇒ lookup i g ≠ lookup i g0) ⇒
-         i ∈ SET_OF_BAG (op_gbag opn)`,
-  rpt gen_tac >> Cases_on `opn` >>
-  simp[known_op_def, case_eq_thms, op_gbag_def, pair_case_eq, va_case_eq,
-       bool_case_eq] >> rw[] >>
-  fs[bool_case_eq, lookup_insert]);
-
-val known_changed_globals = Q.store_thm(
-  "known_changed_globals",
-  `∀es as g0 alist g.
-     known es as g0 = (alist, g) ⇒
-     ∀i. i ∈ domain g ∧ (i ∈ domain g0 ⇒ lookup i g ≠ lookup i g0) ⇒
-         i ∈ SET_OF_BAG (elist_globals es)`,
-  ho_match_mp_tac known_ind >> simp[known_def] >> rpt strip_tac >>
-  rpt (pairarg_tac >> fs[]) >> rveq >> fs[]
-  >- (map_every rename1 [`known [exp1] as g0 = (al,g')`,`i ∈ domain g`] >>
-      Cases_on `i ∈ domain g'` >> fs[] >>
-      Cases_on `i ∈ domain g0` >> fs[] >>
-      Cases_on `lookup i g' = lookup i g0` >> fs[])
-  >- (map_every rename1 [
-        `known [exp1] as g0 = (al1,g1)`,
-        `known [exp2] as g1 = (al2,g2)`,
-        `known [exp3] as g2 = (al3,g3)`] >>
-      Cases_on `i ∈ domain g2` >> fs[] >>
-      Cases_on `i ∈ domain g1` >> fs[] >>
-      Cases_on `i ∈ domain g0` >> fs[] >>
-      Cases_on `lookup i g1 = lookup i g0` >> fs[] >>
-      Cases_on `lookup i g2 = lookup i g1` >> fs[])
-  >- (rename1 `known exps as g0 = (al1,g1)` >>
-      Cases_on `i ∈ domain g1` >> fs[] >>
-      Cases_on `i ∈ domain g0` >> fs[] >>
-      Cases_on `lookup i g1 = lookup i g0` >> fs[])
-  >- (rename1 `known _ _  g0 = (al1,g1)` >>
-      Cases_on `i ∈ domain g1` >> fs[] >>
-      Cases_on `i ∈ domain g0` >> fs[] >>
-      Cases_on `lookup i g1 = lookup i g0` >> fs[])
-  >- (rename1 `known _ _  g0 = (_,g1)` >>
-      rename1 `known_op opn` >>
-      Cases_on `i ∈ domain g1` >> fs[]
-      >- (Cases_on `i ∈ domain g0` >> fs[] >>
-          Cases_on `lookup i g1 = lookup i g0` >> fs[] >>
-          resolve_selected hd known_op_changed_globals >> simp[]) >>
-      resolve_selected hd known_op_changed_globals >> simp[])
-  >- (rename1 `known _ _ g0 = (_, g1)` >>
-      Cases_on `i ∈ domain g1` >> fs[] >>
-      Cases_on `lookup i g1 = lookup i g0` >> fs[] >>
-      Cases_on `lookup i g = lookup i g1` >> fs[]));
-
-val subspt_better_definedg = Q.store_thm(
-  "subspt_better_definedg",
-  `subspt sp1 sp3 ∧ better_definedg sp1 sp2 ∧ better_definedg sp2 sp3 ⇒
-   subspt sp1 sp2`,
-  simp[subspt_def, better_definedg_def] >> rpt strip_tac >>
-  spose_not_then assume_tac >>
-  `k ∈ domain sp2 ∧ k ∈ domain sp3` by metis_tac [] >>
-  `∃v1 v2 v3. lookup k sp1 = SOME v1 ∧ lookup k sp2 = SOME v2 ∧
-              lookup k sp3 = SOME v3` by metis_tac[domain_lookup] >>
-  `v3 = v1` by metis_tac[SOME_11] >> rveq >>
-  `v1 ◁ v2 ∧ v2 ◁ v1` by metis_tac[THE_DEF] >>
-  metis_tac[subapprox_antisym])
-
-val subspt_known_elist_globals = Q.store_thm(
-  "subspt_known_elist_globals",
-  `∀es1 as1 g0 al1 g1 es2 as2 al2 g2.
-     known es1 as1 g0 = (al1, g1) ∧ known es2 as2 g1 = (al2, g2) ∧
-     subspt g0 g2 ∧ BAG_DISJOINT (elist_globals es1) (elist_globals es2) ⇒
-     subspt g0 g1 ∧ subspt g1 g2`,
-  rpt gen_tac >> strip_tac >>
-  `subspt g0 g1` by metis_tac[known_better_definedg, subspt_better_definedg] >>
-  simp[] >> fs[subspt_def] >>
-  rpt (gen_tac ORELSE disch_then strip_assume_tac) >>
-  `better_definedg g1 g2` by metis_tac[known_better_definedg] >>
-  `k ∈ domain g2` by fs[better_definedg_def] >> simp[] >>
-  spose_not_then strip_assume_tac >>
-  `k ∈ SET_OF_BAG (elist_globals es2)` by metis_tac[known_changed_globals] >>
-  Cases_on `k ∈ domain g0` >- metis_tac[] >>
-  `k ∈ SET_OF_BAG (elist_globals es1)` by metis_tac[known_changed_globals] >>
-  fs[BAG_DISJOINT, DISJOINT_DEF, EXTENSION] >> metis_tac[])
-
-val subspt_known_op_elist_globals = Q.store_thm(
-  "subspt_known_op_elist_globals",
-  `∀es as1 g0 al1 g1 opn as2 g2 a.
-      known es as1 g0 = (al1,g1) ∧ known_op opn as2 g1 = (a,g2) ∧ subspt g0 g2 ∧
-      BAG_DISJOINT (op_gbag opn) (elist_globals es) ⇒
-      subspt g0 g1 ∧ subspt g1 g2`,
-  rpt gen_tac >> strip_tac >>
-  `subspt g0 g1`
-    by metis_tac[known_better_definedg, subspt_better_definedg,
-                 known_op_better_definedg] >> simp[] >>
-  fs[subspt_def] >> rpt (gen_tac ORELSE disch_then strip_assume_tac) >>
-  `better_definedg g1 g2` by metis_tac[known_op_better_definedg] >>
-  `k ∈ domain g2` by fs[better_definedg_def] >> simp[] >>
-  spose_not_then strip_assume_tac >>
-  `k ∈ SET_OF_BAG (op_gbag opn)` by metis_tac[known_op_changed_globals] >>
-  Cases_on `k ∈ domain g0` >- metis_tac[] >>
-  `k ∈ SET_OF_BAG (elist_globals es)` by metis_tac[known_changed_globals] >>
-  fs[BAG_DISJOINT, DISJOINT_DEF, EXTENSION] >> metis_tac[])
-
-val FINITE_BAG_FOLDR = Q.store_thm(
-  "FINITE_BAG_FOLDR",
-  `∀l f a.
-     FINITE_BAG a ∧ (∀e a. FINITE_BAG a ∧ MEM e l ⇒ FINITE_BAG (f e a)) ⇒
-     FINITE_BAG (FOLDR f a l)`,
-  Induct >> simp[]);
-
-val FINITE_set_globals = Q.store_thm(
-  "FINITE_set_globals[simp]",
-  `(∀e. FINITE_BAG (set_globals e)) ∧ ∀es. FINITE_BAG (elist_globals es)`,
-  ho_match_mp_tac set_globals_ind >> simp[] >> rpt strip_tac >>
-  rename1 `op_gbag opn` >> Cases_on `opn` >> simp[op_gbag_def]);
-
-val state_globals_approx_def = Define`
-  state_globals_approx s g ⇔
-    ∀k v.
-      get_global k s.globals = SOME (SOME v) ⇒
-      ∃a. lookup k g = SOME a ∧ val_approx_val a v
-`;
-
-val state_approx_better_definedg = Q.store_thm(
-  "state_approx_better_definedg",
-  `better_definedg g1 g2 ∧ state_globals_approx s g1 ⇒
-   state_globals_approx s g2`,
-  csimp[better_definedg_def, state_globals_approx_def, domain_lookup,
-        PULL_EXISTS] >>
-  metis_tac[val_approx_better_approx]);
-
-val mapped_globals_def = Define`
-  mapped_globals (s:('c,'ffi) closSem$state) =
-    { i | ∃v. get_global i s.globals = SOME (SOME v) }
-`;
-
-val mapped_globals_refupdate = Q.store_thm(
-  "mapped_globals_refupdate[simp]",
-  `mapped_globals (s with refs updated_by f) = mapped_globals s`,
-  simp[mapped_globals_def]);
-
-val mapped_globals_ffiupdate = Q.store_thm(
-  "mapped_globals_ffiupdate[simp]",
-  `mapped_globals (s with ffi updated_by v) = mapped_globals s`,
-  simp[mapped_globals_def]);
-
-val mapped_globals_clockupdate = Q.store_thm(
-  "mapped_globals_clockupdate[simp]",
-  `mapped_globals (s with clock updated_by f) = mapped_globals s`,
-  simp[mapped_globals_def]);
-
-val mapped_globals_dec_clock = Q.store_thm(
-  "mapped_globals_dec_clock[simp]",
-  `mapped_globals (dec_clock n s) = mapped_globals s`,
-  simp[mapped_globals_def, dec_clock_def])
-
+(* fixeqs flips any equations in the assumption that have evaluate on the rhs *)
 val evaluate_t = ``closSem$evaluate``
 val fixeqs = let
   fun c t =
@@ -228,6 +31,247 @@ val fixeqs = let
 in
   RULE_ASSUM_TAC (CONV_RULE (TRY_CONV c))
 end
+
+
+val va_case_eq =
+    prove_case_eq_thm{case_def = TypeBase.case_def_of ``:val_approx``,
+                      nchotomy = TypeBase.nchotomy_of ``:val_approx``}
+
+val result_ty = ``:(α,β)semanticPrimitives$result``
+val result_CASES = TypeBase.nchotomy_of result_ty
+val result_case_eq =
+    prove_case_eq_thm{case_def = TypeBase.case_def_of result_ty,
+                      nchotomy = result_CASES}
+
+(*
+val error_ty = ``:α semanticPrimitives$error_result``
+val error_CASES = TypeBase.nchotomy_of error_ty
+val error_case_eq =
+    prove_case_eq_thm{case_def = TypeBase.case_def_of error_ty,
+                      nchotomy = error_CASES}
+*)
+
+(* simple properties of constants from clos_known: i.e., merge and known *)
+
+val known_op_changed_globals = Q.store_thm(
+  "known_op_changed_globals",
+  `!opn aenv g0 a g.
+     known_op opn aenv g0 = (a, g) ==>
+     !i. i ∈ domain g /\ (i ∈ domain g0 ==> lookup i g <> lookup i g0) ==>
+         i ∈ SET_OF_BAG (op_gbag opn)`,
+  rpt gen_tac \\ Cases_on `opn`
+  \\ simp [known_op_def, case_eq_thms, op_gbag_def,
+           pair_case_eq, bool_case_eq, va_case_eq]
+  \\ rw []
+  \\ fs [lookup_insert, bool_case_eq])
+
+val known_changed_globals = Q.store_thm(
+  "known_changed_globals",
+  `!limit xs aenv g0 alist g.
+     known limit xs aenv g0 = (alist, g) ==>
+     !i. i ∈ domain g ∧ (i ∈ domain g0 ==> lookup i g <> lookup i g0) ==>
+         i ∈ SET_OF_BAG (elist_globals xs)`,
+  ho_match_mp_tac known_ind \\ simp [known_def] \\ rpt strip_tac
+  \\ rpt (pairarg_tac \\ fs []) \\ rveq \\ fs []
+  THEN1
+   (rename1 `known _ [x] aenv g0 = (_, g1)`
+    \\ Cases_on `i ∈ domain g1` \\ fs[]
+    \\ Cases_on `i ∈ domain g0` \\ fs[]
+    \\ Cases_on `lookup i g1 = lookup i g0` \\ fs[])
+  THEN1
+   (map_every rename1 [
+      `known _ [x1] aenv g0 = (ea1, g1)`,
+      `known _ [x2] aenv g1 = (ea2, g2)`,
+      `known _ [x3] aenv g2 = (ea3, g3)`]
+    \\ Cases_on `i ∈ domain g2` \\ fs[]
+    \\ Cases_on `i ∈ domain g1` \\ fs[]
+    \\ Cases_on `i ∈ domain g0` \\ fs[]
+    \\ Cases_on `lookup i g1 = lookup i g0` \\ fs []
+    \\ Cases_on `lookup i g2 = lookup i g1` \\ fs [])
+  THEN1
+   (rename1 `known _ xs aenv g0 = (ea1, g1)`
+    \\ Cases_on `i ∈ domain g1` \\ fs[]
+    \\ Cases_on `i ∈ domain g0` \\ fs[]
+    \\ Cases_on `lookup i g1 = lookup i g0` \\ fs [])
+  THEN1
+   (rename1 `known _ [x1] aenv g0 = (ee1, g1)`
+    \\ Cases_on `i ∈ domain g1` \\ fs[]
+    \\ Cases_on `i ∈ domain g0` \\ fs[]
+    \\ Cases_on `lookup i g1 = lookup i g0` \\ fs [])
+  THEN1
+   (rename1 `known _ xs aenv g0 = (ee1, g1)`
+    \\ imp_res_tac known_op_changed_globals
+    \\ Cases_on `i ∈ domain g1` \\ fs[]
+    \\ Cases_on `i ∈ domain g0` \\ fs[]
+    \\ Cases_on `lookup i g1 = lookup i g0` \\ fs[])
+  \\ Cases_on `SND limit = 0` \\ fs [] \\ rveq
+  THEN1
+   (rename1 `known _ _ aenv g0 = (_, g1)`
+    \\ rename1 `known _ _ aenv g1 = (_, g2)`
+    \\ Cases_on `i ∈ domain g1` \\ fs[]
+    \\ Cases_on `i ∈ domain g0` \\ fs[]
+    \\ Cases_on `lookup i g1 = lookup i g0` \\ fs[])
+  \\ Cases_on `body_opt` \\ fs [] \\ rveq
+  THEN1
+   (rename1 `known _ _ aenv g0 = (_, g1)`
+    \\ rename1 `known _ _ aenv g1 = (_, g2)`
+    \\ Cases_on `i ∈ domain g1` \\ fs[]
+    \\ Cases_on `i ∈ domain g0` \\ fs[]
+    \\ Cases_on `lookup i g1 = lookup i g0` \\ fs[])
+  \\ Cases_on `pure x` \\ fs [] \\ rveq
+  \\ rpt (pairarg_tac \\ fs [])
+  \\ rename1 `known _ _ aenv g0 = (_, g1)`
+  \\ rename1 `known _ _ aenv g1 = (_, g2)`
+  \\ Cases_on `i ∈ domain g1` \\ fs[]
+  \\ Cases_on `i ∈ domain g0` \\ fs[]
+  \\ Cases_on `lookup i g1 = lookup i g0` \\ fs[]);
+
+val known_unchanged_globals = Q.store_thm(
+  "known_unchanged_globals",
+  `!limit xs aenv g0 eas1 g1.
+     known limit xs aenv g0 = (eas1, g1) /\
+     elist_globals xs = {||} ==> g0 = g1`,
+  ho_match_mp_tac known_ind
+  \\ simp [known_def]
+  \\ rpt strip_tac
+  \\ rpt (pairarg_tac \\ fs []) \\ rveq
+  THEN1 (Cases_on `op`
+         \\ fs [known_op_def, bool_case_eq,
+                case_eq_thms, va_case_eq, op_gbag_def])
+  THEN1 (fs [bool_case_eq, case_eq_thms]
+         \\ rpt (pairarg_tac \\ fs [])));
+
+(* Take first n expressions returned by the compile oracle. *)
+val first_n_exps_def = Define `
+  first_n_exps co n = GENLIST (FST o SND o co) n`;
+
+val first_n_exps_shift_seq = Q.store_thm("first_n_exps_shift_seq",
+  `!co n k. first_n_exps co (n + k) = first_n_exps co k ++ first_n_exps (shift_seq k co) n`,
+  Induct_on `n`
+  \\ rpt strip_tac
+  \\ fs [first_n_exps_def]
+  \\ REWRITE_TAC [Q.prove (`k + SUC n = SUC (k + n)`, decide_tac)]
+  \\ fs [GENLIST]
+  \\ fs [shift_seq_def])
+
+(* All globals set in the program and in code returned by
+   the compile oracle are unique. *)
+val unique_set_globals_def = Define `
+  unique_set_globals es co <=>
+    !n. BAG_ALL_DISTINCT (elist_globals (es ++ first_n_exps co n))`;
+
+val unique_set_globals_shift_seq = Q.store_thm(
+  "unique_set_globals_shift_seq",
+  `!es co k. unique_set_globals es co ==> unique_set_globals es (shift_seq k co)`,
+  fs [unique_set_globals_def]
+  \\ rpt strip_tac
+  \\ pop_assum (qspec_then `n + k` assume_tac)
+  \\ fs [first_n_exps_shift_seq]
+  \\ fs [elist_globals_append]
+  \\ fs [BAG_ALL_DISTINCT_BAG_UNION]);
+
+val unique_set_globals_evaluate = Q.store_thm(
+  "unique_set_globals_evaluate",
+  `!es xs env s1 s2 res. unique_set_globals xs s1.compile_oracle /\
+   evaluate (es,env,s1) = (res, s2) ==> unique_set_globals xs s2.compile_oracle`,
+  rpt strip_tac \\ imp_res_tac evaluate_code \\ fs []
+  \\ simp [unique_set_globals_shift_seq]);
+
+(* Compile oracle globals are disjoint from given map. *)
+val co_disjoint_globals_def = Define `
+  co_disjoint_globals g co =
+    !n. DISJOINT (domain g) (SET_OF_BAG (set_globals (FST (SND (co n)))))`;
+
+val co_disjoint_globals_shift_seq = Q.store_thm(
+  "co_disjoint_globals_shift_seq",
+  `co_disjoint_globals g co ==>
+   co_disjoint_globals g (shift_seq k co)`,
+  fs [co_disjoint_globals_def, shift_seq_def]);
+
+val co_disjoint_globals_evaluate = Q.store_thm(
+  "co_disjoint_globals_evaluate",
+  `!g s0 es env res s1.
+     co_disjoint_globals g s0.compile_oracle /\
+     evaluate (es, env, s0) = (res, s1) ==>
+     co_disjoint_globals g s1.compile_oracle`,
+  rw [] \\ imp_res_tac evaluate_code \\ simp [co_disjoint_globals_shift_seq]);
+
+val co_disjoint_globals_first_n_exps = Q.store_thm(
+  "co_disjoint_globals_first_n_exps",
+  `!g co. co_disjoint_globals g co ==>
+     !n. DISJOINT (domain g) (SET_OF_BAG (elist_globals (first_n_exps co n)))`,
+  rpt gen_tac
+  \\ simp [first_n_exps_def, co_disjoint_globals_def]
+  \\ strip_tac
+  \\ Induct \\ simp []
+  \\ simp [GENLIST, SNOC_APPEND, elist_globals_append,
+           SET_OF_BAG_UNION]
+  \\ simp [DISJOINT_SYM]);
+
+val direct_subexp_def = Define `
+  (direct_subexp es [] <=> es = []) /\
+  (direct_subexp es (x1::x2::xs) <=> es = [x1] \/ es = (x2::xs)) /\
+  (direct_subexp es [Var t n] <=> F) /\
+  (direct_subexp es [If t x1 x2 x3] <=> es = [x1] \/ es = [x2] \/ es = [x3]) /\
+  (direct_subexp es [Let t xs x1] <=> es = xs \/ es = [x1]) /\
+  (direct_subexp es [Raise t x1] <=> es = [x1]) /\
+  (direct_subexp es [Handle t x1 x2] <=> es = [x1] \/ es = [x2]) /\
+  (direct_subexp es [Op t opn xs] <=> es = xs) /\
+  (direct_subexp es [Fn t loc_opt vsopt num_args x1] <=> es = [x1]) /\
+  (direct_subexp es [Letrec t loc_opt vsopt fns x1] <=> es = (MAP SND fns) \/ es = [x1]) /\
+  (direct_subexp es [App t loc_opt x1 xs] <=> es = [x1] \/ es = xs) /\
+  (direct_subexp es [Tick t x1] <=> es = [x1]) /\
+  (direct_subexp es [Call t ticks dest xs] <=> es = xs)`;
+
+val direct_subexp_def = save_thm(
+  "direct_subexp_def[simp]",
+  direct_subexp_def |> SIMP_RULE (srw_ss()) []);
+
+val BAG_DISJOINT_SYM = Q.prove(
+  `!b1 b2. BAG_DISJOINT b1 b2 <=> BAG_DISJOINT b2 b1`,
+  simp [BAG_DISJOINT, DISJOINT_SYM]);
+
+val unique_set_globals_subexps = Q.store_thm("unique_set_globals_subexps",
+ `(unique_set_globals (x1::x2::xs) co ==>
+     unique_set_globals [x1] co /\ unique_set_globals (x2::xs) co) /\
+  (unique_set_globals [If t x1 x2 x3] co ==>
+     unique_set_globals [x1] co /\ unique_set_globals [x2] co /\ unique_set_globals [x3] co) /\
+  (unique_set_globals [Let t xs x2] co ==>
+     unique_set_globals xs co /\ unique_set_globals [x2] co) /\
+  (unique_set_globals [Raise t x1] co ==>
+     unique_set_globals [x1] co) /\
+  (unique_set_globals [Handle t x1 x2] co ==>
+     unique_set_globals [x1] co /\ unique_set_globals [x2] co) /\
+  (unique_set_globals [Op t opn xs] co ==>
+     unique_set_globals xs co) /\
+  (unique_set_globals [Fn t loc_opt vsopt num_args x1] co ==>
+     unique_set_globals [x1] co) /\
+  (unique_set_globals [Letrec t loc_opt vsopt fns x1] co ==>
+     unique_set_globals [x1] co /\ unique_set_globals (MAP SND fns) co) /\
+  (unique_set_globals [App t loc_opt x1 xs] co ==>
+     unique_set_globals [x1] co /\ unique_set_globals xs co) /\
+  (unique_set_globals [Tick t x1] co ==>
+     unique_set_globals [x1] co) /\
+  (unique_set_globals [Call t ticks dest xs] co ==>
+     unique_set_globals xs co)`,
+  rpt strip_tac
+  \\ fs [unique_set_globals_def]
+  \\ fs [elist_globals_append]
+  \\ fs [BAG_ALL_DISTINCT_BAG_UNION]);
+
+val unique_set_globals_subexps = GEN_ALL unique_set_globals_subexps;
+
+val unique_set_globals_IMP_es_distinct_elist_globals = Q.store_thm(
+  "unique_set_globals_IMP_es_distinct_elist_globals",
+  `!es co. unique_set_globals es co ==> BAG_ALL_DISTINCT (elist_globals es)`,
+  simp [unique_set_globals_def, elist_globals_append, BAG_ALL_DISTINCT_BAG_UNION]);
+
+(* State globals agree with the approximated globals. *)
+val state_globals_approx_def = Define `
+  state_globals_approx s g ⇔
+    ∀k v.
+      get_global k s.globals = SOME (SOME v) ⇒
+      !a. lookup k g = SOME a ==> val_approx_val a v`;
 
 val state_globals_approx_clock_fupd = Q.store_thm(
   "state_globals_approx_clock_fupd[simp]",
@@ -252,12 +296,57 @@ val state_globals_approx_ffifupd = Q.store_thm(
    state_globals_approx s g`,
   simp[state_globals_approx_def]);
 
-val value_ind =
-  TypeBase.induction_of ``:closSem$v``
-   |> Q.SPECL [`P`, `EVERY P`]
-   |> SIMP_RULE (srw_ss()) []
-   |> UNDISCH |> CONJUNCT1 |> DISCH_ALL |> Q.GEN `P`
+val state_globals_approx_codeupd = Q.store_thm(
+  "state_globals_approx_codeupd[simp]",
+  `state_globals_approx (s with code updated_by f) g ⇔
+   state_globals_approx s g`,
+  simp[state_globals_approx_def]);
 
+val state_globals_approx_coupd = Q.store_thm(
+  "state_globals_approx_coupd[simp]",
+  `state_globals_approx (s with compile_oracle updated_by f) g ⇔
+   state_globals_approx s g`,
+  simp[state_globals_approx_def]);
+
+
+(* Mapped globals *)
+
+val mapped_globals_def = Define`
+  mapped_globals (s:('c,'ffi) closSem$state) =
+    { i | ∃v. get_global i s.globals = SOME (SOME v) }
+`;
+
+val mapped_globals_refupdate = Q.store_thm(
+  "mapped_globals_refupdate[simp]",
+  `mapped_globals (s with refs updated_by f) = mapped_globals s`,
+  simp[mapped_globals_def]);
+
+val mapped_globals_ffiupdate = Q.store_thm(
+  "mapped_globals_ffiupdate[simp]",
+  `mapped_globals (s with ffi updated_by v) = mapped_globals s`,
+  simp[mapped_globals_def]);
+
+val mapped_globals_clockupdate = Q.store_thm(
+  "mapped_globals_clockupdate[simp]",
+  `mapped_globals (s with clock updated_by f) = mapped_globals s`,
+  simp[mapped_globals_def]);
+
+val mapped_globals_dec_clock = Q.store_thm(
+  "mapped_globals_dec_clock[simp]",
+  `mapped_globals (dec_clock n s) = mapped_globals s`,
+  simp[mapped_globals_def, dec_clock_def]);
+
+val mapped_globals_codeupdate = Q.store_thm(
+  "mapped_globals_codeupdate[simp]",
+  `mapped_globals (s with code updated_by f) g = mapped_globals s g`,
+  simp[mapped_globals_def]);
+
+val mapped_globals_coupdate = Q.store_thm(
+  "mapped_globals_coupdate[simp]",
+  `mapped_globals (s with compile_oracle updated_by f) g = mapped_globals s g`,
+  simp[mapped_globals_def]);
+
+(* Extending mapped globals *)
 
 val mglobals_extend_def = Define`
   mglobals_extend s1 mgs s2 ⇔
@@ -272,13 +361,13 @@ val mglobals_extend_refl = Q.store_thm(
 
 val mglobals_extend_trans = Q.store_thm(
   "mglobals_extend_trans",
-  `mglobals_extend s0 g1 s1 ∧ mglobals_extend s1 g2 s2 ⇒
+  `!s0 s1 s2 g1 g2. mglobals_extend s0 g1 s1 ∧ mglobals_extend s1 g2 s2 ⇒
    mglobals_extend s0 (g1 ∪ g2) s2`,
   simp[mglobals_extend_def, SUBSET_DEF] >> metis_tac[]);
 
 val mglobals_extend_SUBSET = Q.store_thm(
   "mglobals_extend_SUBSET",
-  `mglobals_extend s0 g1 s ∧ g1 ⊆ g2 ⇒ mglobals_extend s0 g2 s`,
+  `!s0 s g1 g2. mglobals_extend s0 g1 s ∧ g1 ⊆ g2 ⇒ mglobals_extend s0 g2 s`,
   simp[mglobals_extend_def, SUBSET_DEF] >> metis_tac[]);
 
 val mglobals_extend_refupdate = Q.store_thm(
@@ -311,6 +400,175 @@ val mglobals_extend_decclock = Q.store_thm(
    (mglobals_extend s0 gs (dec_clock n s) ⇔ mglobals_extend s0 gs s)`,
   simp[dec_clock_def]);
 
+val mapped_globals_codeupdate = Q.store_thm(
+  "mglobals_extend_codeupdate[simp]",
+  `(mglobals_extend s0 gs (s with code updated_by f) ⇔
+      mglobals_extend s0 gs s) /\
+   (mglobals_extend (s0 with code updated_by f) gs s ⇔
+      mglobals_extend s0 gs s)`,
+  simp[mglobals_extend_def,mapped_globals_def]);
+
+val mglobals_extend_co_update = Q.store_thm(
+  "mglobals_extend_co_update[simp]",
+  `(mglobals_extend s0 gs (s with compile_oracle updated_by f) ⇔
+      mglobals_extend s0 gs s) /\
+   (mglobals_extend (s0 with compile_oracle updated_by f) gs s ⇔
+      mglobals_extend s0 gs s)`,
+  simp[mglobals_extend_def,mapped_globals_def]);
+
+
+val subspt_better_definedg = Q.store_thm(
+  "subspt_better_definedg",
+  `!sp1 sp2 sp3. subspt sp1 sp3 ∧ better_definedg sp1 sp2 ∧ better_definedg sp2 sp3 ⇒
+   subspt sp1 sp2`,
+  simp[subspt_def, better_definedg_def] >> rpt strip_tac >>
+  spose_not_then assume_tac >>
+  `k ∈ domain sp2 ∧ k ∈ domain sp3` by metis_tac [] >>
+  `∃v1 v2 v3. lookup k sp1 = SOME v1 ∧ lookup k sp2 = SOME v2 ∧
+              lookup k sp3 = SOME v3` by metis_tac[domain_lookup] >>
+  `v3 = v1` by metis_tac[SOME_11] >> rveq >>
+  `v1 ◁ v2 ∧ v2 ◁ v1` by metis_tac[THE_DEF] >>
+  metis_tac[subapprox_antisym])
+
+val subspt_known_elist_globals = Q.store_thm(
+  "subspt_known_elist_globals",
+  `∀limit es1 as1 g0 al1 g1 es2 as2 al2 g2.
+     known limit es1 as1 g0 = (al1, g1) ∧ known limit es2 as2 g1 = (al2, g2) ∧
+     subspt g0 g2 ∧ BAG_DISJOINT (elist_globals es1) (elist_globals es2) ⇒
+     subspt g0 g1 ∧ subspt g1 g2`,
+  rpt gen_tac >> strip_tac >>
+  `subspt g0 g1` by metis_tac[known_better_definedg, subspt_better_definedg] >>
+  simp[] >> fs[subspt_def] >>
+  rpt (gen_tac ORELSE disch_then strip_assume_tac) >>
+  `better_definedg g1 g2` by metis_tac[known_better_definedg] >>
+  `k ∈ domain g2` by fs[better_definedg_def] >> simp[] >>
+  spose_not_then strip_assume_tac >>
+  `k ∈ SET_OF_BAG (elist_globals es2)` by metis_tac[known_changed_globals] >>
+  Cases_on `k ∈ domain g0` >- metis_tac[] >>
+  `k ∈ SET_OF_BAG (elist_globals es1)` by metis_tac[known_changed_globals] >>
+  fs[BAG_DISJOINT, DISJOINT_DEF, EXTENSION] >> metis_tac[])
+
+
+
+val subspt_known_op_elist_globals = Q.store_thm(
+  "subspt_known_op_elist_globals",
+  `∀limit es as1 g0 al1 g1 opn as2 g2 a.
+      known limit es as1 g0 = (al1,g1) ∧ known_op opn as2 g1 = (a,g2) ∧ subspt g0 g2 ∧
+      BAG_DISJOINT (op_gbag opn) (elist_globals es) ⇒
+      subspt g0 g1 ∧ subspt g1 g2`,
+  rpt gen_tac >> strip_tac >>
+  `subspt g0 g1`
+    by metis_tac[known_better_definedg, subspt_better_definedg,
+                 known_op_better_definedg] >> simp[] >>
+  fs[subspt_def] >> rpt (gen_tac ORELSE disch_then strip_assume_tac) >>
+  `better_definedg g1 g2` by metis_tac[known_op_better_definedg] >>
+  `k ∈ domain g2` by fs[better_definedg_def] >> simp[] >>
+  spose_not_then strip_assume_tac >>
+  `k ∈ SET_OF_BAG (op_gbag opn)` by metis_tac[known_op_changed_globals] >>
+  Cases_on `k ∈ domain g0` >- metis_tac[] >>
+  `k ∈ SET_OF_BAG (elist_globals es)` by metis_tac[known_changed_globals] >>
+  fs[BAG_DISJOINT, DISJOINT_DEF, EXTENSION] >> metis_tac[])
+
+
+val known_op_correct_approx = Q.store_thm("known_op_correct_approx",
+  `!opn args g0 a g vs s0 g' v s.
+   known_op opn args g0 = (a,g) ∧ LIST_REL val_approx_val args vs ∧
+   state_globals_approx s0 g' ∧ subspt g g' /\
+   do_app opn vs s0 = Rval (v, s) ⇒
+   state_globals_approx s g' ∧ val_approx_val a v`,
+  rpt gen_tac
+  \\ `?this_is_case. this_is_case opn` by (qexists_tac `K T` \\ fs [])
+  \\ Cases_on `opn`
+  \\ simp [known_op_def, do_app_def, case_eq_thms, va_case_eq, bool_case_eq,
+           pair_case_eq]
+  \\ rpt strip_tac \\ rveq \\ fs[]
+  THEN1
+   (fs [state_globals_approx_def] \\ res_tac
+    \\ metis_tac [SOME_11, subspt_lookup])
+  THEN1
+   (fs [subspt_lookup, lookup_insert]
+    \\ fs [state_globals_approx_def] \\ rw []
+    \\ fs [get_global_def, EL_LUPDATE, bool_case_eq] \\ rveq \\ fs []
+    THEN1 (first_x_assum (qspecl_then [`k`, `a'`] assume_tac) \\ fs [])
+    THEN1 metis_tac [])
+  THEN1
+   (fs [subspt_lookup, lookup_insert]
+    \\ fs [state_globals_approx_def] \\ rw []
+    \\ fs [get_global_def, EL_LUPDATE, bool_case_eq] \\ rveq \\ fs []
+    THEN1 (first_x_assum (qspecl_then [`k`, `merge other a'`] assume_tac)
+           \\ fs [] \\ metis_tac [val_approx_val_merge_I])
+    THEN1 metis_tac [])
+  THEN1
+   (fs [state_globals_approx_def, get_global_def,
+        EL_APPEND_EQN, bool_case_eq]
+    \\ rw [] THEN1 (metis_tac [])
+    \\ rename1 `nn - LENGTH (ss:('a,'b) closSem$state).globals`
+    \\ `nn = LENGTH ss.globals` by simp [] \\ fs [])
+  THEN1
+   (rveq \\ fs [LIST_REL_EL_EQN]));
+
+
+val ssgc_free_co_shift_seq = Q.store_thm(
+  "ssgc_free_co_shift_seq",
+  `ssgc_free s ==> ssgc_free (s with compile_oracle := shift_seq k s.compile_oracle)`,
+  simp [ssgc_free_def] \\ strip_tac \\ rpt conj_tac \\ fs []
+  \\ rpt gen_tac \\ strip_tac \\ fs [shift_seq_def] \\ res_tac \\ simp []);
+
+val shift_seq_zero = Q.store_thm(
+  "shift_seq_zero[simp]",
+  `!co. shift_seq 0 co = co`,
+  simp [shift_seq_def, ETA_THM]);
+
+val shift_seq_add = Q.store_thm(
+  "shift_seq_add[simp]",
+  `!co k1 k2. shift_seq k2 (shift_seq k1 co) = shift_seq (k1 + k2) co`,
+  simp [shift_seq_def]);
+
+val ssgc_free_do_install = Q.store_thm(
+  "ssgc_free_do_install",
+  `!s. ssgc_free s ==>
+   ssgc_free (s with <|compile_oracle := shift_seq 1 (s.compile_oracle);
+                       code := s.code |++ SND (SND (s.compile_oracle 0))|>)`,
+  gen_tac \\ simp [ssgc_free_def] \\ strip_tac \\ rpt conj_tac
+  THEN1 (`?exp aux. SND (s.compile_oracle 0) = (exp, aux)`
+           by (Cases_on `SND (s.compile_oracle 0)` \\ simp [])
+         \\ res_tac \\ simp []
+         \\ rpt strip_tac
+         \\ fs [flookup_fupdate_list]
+         \\ fs [case_eq_thms] THEN1 res_tac
+         \\ imp_res_tac ALOOKUP_MEM
+         \\ fs [MEM_REVERSE]
+         \\ fs [MEM_SPLIT]
+         \\ rveq
+         \\ fs [MAP_APPEND, elist_globals_append])
+  THEN1 (rw [] \\ res_tac)
+  THEN1 (simp [shift_seq_def] \\ rw [] \\ res_tac));
+
+val do_install_ssgc = Q.store_thm(
+  "do_install_ssgc",
+  `!vs s0 e s1. do_install vs s0 = (Rval e, s1) /\ ssgc_free s0 ==>
+   ssgc_free s1 /\ esgc_free e /\
+   s1.compile_oracle = shift_seq 1 s0.compile_oracle /\
+   first_n_exps s0.compile_oracle 1 = [e] /\
+   mglobals_extend s0 (SET_OF_BAG (set_globals e)) s1`,
+   rpt gen_tac \\ strip_tac
+   \\ fs [do_install_def, case_eq_thms]
+   \\ pairarg_tac \\ fs []
+   \\ fs [case_eq_thms, bool_case_eq, pair_case_eq]
+   \\ rveq
+   \\ simp [first_n_exps_def]
+   \\ imp_res_tac ssgc_free_do_install \\ rfs []
+   \\ pop_assum kall_tac
+   \\ fs [ssgc_free_def]
+   \\ Cases_on `SND (s0.compile_oracle 0)`
+   \\ res_tac \\ rfs []);
+
+val value_ind =
+  TypeBase.induction_of ``:closSem$v``
+   |> Q.SPECL [`P`, `EVERY P`]
+   |> SIMP_RULE (srw_ss()) []
+   |> UNDISCH |> CONJUNCT1 |> DISCH_ALL |> Q.GEN `P`
+
 (* TODO closProps? *)
 val list_to_v_EVERY_APPEND = Q.store_thm("list_to_v_EVERY_APPEND",
   `!(x: closSem$v) y xs ys.
@@ -333,13 +591,14 @@ val list_to_v_EVERY_APPEND = Q.store_thm("list_to_v_EVERY_APPEND",
 
 val do_app_ssgc = Q.store_thm(
   "do_app_ssgc",
-  `∀opn args s0 res.
-     do_app opn args s0 = res ⇒
-     EVERY vsgc_free args ∧ ssgc_free s0 ⇒
-     (∀v s. res = Rval(v,s) ⇒
-            vsgc_free v ∧ ssgc_free s ∧
-            mglobals_extend s0 (SET_OF_BAG (op_gbag opn)) s) ∧
-     (∀v. res = Rerr (Rraise v) ⇒ vsgc_free v)`,
+  `!opn args s0 res.
+     do_app opn args s0 = res /\
+     EVERY vsgc_free args /\ ssgc_free s0 ==>
+     (!v s. res = Rval (v, s) ==>
+            vsgc_free v /\ ssgc_free s /\
+            s.compile_oracle = s0.compile_oracle /\
+            mglobals_extend s0 (SET_OF_BAG (op_gbag opn)) s) /\
+     (!v. res = Rerr (Rraise v) ==> vsgc_free v)`,
   Cases_on `opn` >>
   simp[do_app_def, case_eq_thms, op_gbag_def, PULL_EXISTS, bool_case_eq,
        pair_case_eq]
@@ -351,6 +610,8 @@ val do_app_ssgc = Q.store_thm(
       >- metis_tac[]
       >- metis_tac[]
       >- (fs[MEM_LUPDATE] >> metis_tac[MEM_EL])
+      >- metis_tac[]
+      >- metis_tac[]
       >- (dsimp[SUBSET_DEF, get_global_def,
                 EL_LUPDATE, bool_case_eq] >> metis_tac[])
       >- (fs[get_global_def, EL_LUPDATE]))
@@ -389,12 +650,6 @@ val do_app_ssgc = Q.store_thm(
       >- first_assum MATCH_ACCEPT_TAC >> fs[] >>
       dsimp[FLOOKUP_UPDATE, bool_case_eq, EVERY_REPLICATE] >> metis_tac[])
   >- (dsimp[ssgc_free_def,FLOOKUP_UPDATE,bool_case_eq] \\ rw[] \\ metis_tac[])
-  >- (* ListAppend *)
-   (rw [] \\ fs []
-    \\ match_mp_tac list_to_v_EVERY_APPEND
-    \\ simp [vsgc_free_def]
-    \\ asm_exists_tac \\ fs []
-    \\ asm_exists_tac \\ fs [])
   >- (simp[PULL_FORALL] >> rpt gen_tac >> rename1 `v_to_list v = SOME vs` >>
       map_every qid_spec_tac [`vs`, `v`] >> ho_match_mp_tac value_ind >>
       simp[v_to_list_def] >> Cases >>
@@ -411,6 +666,8 @@ val do_app_ssgc = Q.store_thm(
       rpt strip_tac
       >- metis_tac[]
       >- (irule IMP_EVERY_LUPDATE >> simp[] >> metis_tac[])
+      >- metis_tac[]
+      >- metis_tac[]
       >- metis_tac[])
   >- (dsimp[ssgc_free_def, FLOOKUP_UPDATE, bool_case_eq] >> metis_tac[])
   >> dsimp[]);
@@ -420,6 +677,2543 @@ val EVERY_lookup_vars = Q.store_thm(
   `∀vs env env'. EVERY P env ∧ lookup_vars vs env = SOME env' ⇒ EVERY P env'`,
   Induct >> simp[lookup_vars_def, case_eq_thms, PULL_EXISTS] >>
   metis_tac[MEM_EL, EVERY_MEM]);
+
+
+val dest_closure_Full_sgc_free = Q.store_thm(
+  "dest_closure_Full_sgc_free",
+  `dest_closure max_app loc_opt f (arg1::args) =
+     SOME (Full_app fbody env rest_args) /\
+   vsgc_free f /\ vsgc_free arg1 /\ EVERY vsgc_free args ==>
+   set_globals fbody = {||} /\ EVERY vsgc_free env /\ EVERY vsgc_free rest_args`,
+   rpt gen_tac \\ strip_tac
+   \\ imp_res_tac dest_closure_is_closure
+   \\ imp_res_tac dest_closure_full_length
+   \\ rename [`is_closure f`]
+   \\ Cases_on `f` \\ fs [is_closure_def]
+   \\ fs [dest_closure_def]
+   THEN1 (rveq
+          \\ simp [EVERY_REVERSE]
+          \\ conj_tac
+          THEN1 (irule EVERY_TAKE \\ simp [EVERY_REVERSE])
+          THEN1 (irule EVERY_DROP \\ simp [EVERY_REVERSE]))
+   \\ rpt (pairarg_tac \\ fs [])
+   \\ rveq
+   \\ rename [`EL n funs = _`]
+   \\ qmatch_assum_abbrev_tac `EL n funs = funn`
+   \\ `MEM funn funs` by (simp [MEM_EL] \\ qexists_tac `n` \\ simp [])
+   \\ unabbrev_all_tac
+   \\ fs [MEM_SPLIT] \\ fs [elist_globals_append]
+   \\ simp [EVERY_REVERSE, EVERY_GENLIST, elist_globals_append]
+   \\ conj_tac
+   THEN1 (irule EVERY_TAKE \\ simp [EVERY_REVERSE])
+   THEN1 (irule EVERY_DROP \\ simp [EVERY_REVERSE]));
+
+val say = say0 "evaluate_changed_globals_0";
+
+(* Evaluate  *)
+val evaluate_changed_globals_0 = Q.prove(
+  `(!es env (s0:('c,'ffi) closSem$state) res s.
+      evaluate (es, env, s0) = (res, s) /\
+      ssgc_free s0 /\ EVERY esgc_free es /\
+      EVERY vsgc_free env ==>
+        ssgc_free s /\ rsgc_free res /\
+        ?n.
+          s.compile_oracle = shift_seq n s0.compile_oracle /\
+          mglobals_extend s0
+            (SET_OF_BAG (elist_globals es) ∪
+             SET_OF_BAG (elist_globals (first_n_exps s0.compile_oracle n))) s) /\
+   (!loc_opt f args (s0:('c,'ffi) closSem$state) res s.
+      evaluate_app loc_opt f args s0 = (res, s) /\
+      ssgc_free s0 /\ vsgc_free f /\ EVERY vsgc_free args ==>
+        ssgc_free s /\ rsgc_free res /\
+        ?n.
+          s.compile_oracle = shift_seq n s0.compile_oracle /\
+          mglobals_extend s0
+            (SET_OF_BAG (elist_globals (first_n_exps s0.compile_oracle n))) s)`,
+  ho_match_mp_tac (evaluate_ind |> Q.SPEC `\(x1,x2,x3). P0 x1 x2 x3`
+                   |> Q.GEN `P0` |> SIMP_RULE std_ss [FORALL_PROD])
+  \\ rpt conj_tac \\ rpt (gen_tac ORELSE disch_then strip_assume_tac)
+  THEN1
+   (say "NIL"
+    \\ fs [evaluate_def] \\ rveq \\ simp []
+    \\ qexists_tac `0` \\ simp [])
+  THEN1
+   (say "CONS"
+    \\ fs [evaluate_def, pair_case_eq]
+    \\ reverse (fs [result_case_eq]) \\ rveq \\ fs []
+    THEN1 (qexists_tac `n` \\ fs [SET_OF_BAG_UNION]
+           \\ match_mp_tac mglobals_extend_SUBSET
+           \\ goal_assum drule
+           \\ simp [GSYM UNION_ASSOC])
+    \\ reverse (fs [pair_case_eq, result_case_eq]) \\ rveq \\ fs []
+    \\ imp_res_tac evaluate_SING \\ rveq \\ fs []
+    \\ qexists_tac `n' + n` \\ simp [first_n_exps_shift_seq]
+    \\ qmatch_asmsub_abbrev_tac `mglobals_extend s0 g1 s1`
+    \\ qmatch_asmsub_abbrev_tac `mglobals_extend s1 g2 s`
+    \\ qmatch_goalsub_abbrev_tac `mglobals_extend s0 g3 s`
+    \\ `g3 = g1 ∪ g2` suffices_by metis_tac [mglobals_extend_trans]
+    \\ fs [elist_globals_append, SET_OF_BAG_UNION]
+    \\ unabbrev_all_tac \\ rpt (pop_assum kall_tac)
+    \\ metis_tac [UNION_ASSOC, UNION_COMM])
+  THEN1
+   (say "Var"
+    \\ fs [evaluate_def, bool_case_eq, EVERY_EL]
+    \\ qexists_tac `0` \\ simp [])
+  THEN1
+   (say "If"
+    \\ reverse (fs [evaluate_def, pair_case_eq, case_eq_thms])
+    \\ rveq \\ fs []
+    THEN1 (qexists_tac `n` \\ simp [SET_OF_BAG_UNION]
+           \\ match_mp_tac mglobals_extend_SUBSET
+           \\ goal_assum drule
+           \\ metis_tac [UNION_ASSOC, UNION_COMM, SUBSET_UNION])
+    \\ rename1 `Rval vs`
+    \\ reverse (Cases_on `Boolv T = HD vs \/ (Boolv T <> HD vs /\ Boolv F = HD vs)`)
+    THEN1 (fs [] \\ fs [] \\ rveq \\ fs []
+           \\ qexists_tac `n` \\ simp [SET_OF_BAG_UNION]
+           \\ match_mp_tac mglobals_extend_SUBSET
+           \\ goal_assum drule
+           \\ metis_tac [UNION_ASSOC, UNION_COMM, SUBSET_UNION])
+    \\ fs [] \\ fs []
+    \\ qexists_tac `n' + n`
+    \\ simp [first_n_exps_shift_seq]
+    \\ qmatch_asmsub_abbrev_tac `mglobals_extend s0 g1 s1`
+    \\ qmatch_asmsub_abbrev_tac `mglobals_extend s1 g2 s`
+    \\ qmatch_goalsub_abbrev_tac `mglobals_extend s0 g3 s`
+    \\ `g1 ∪ g2 ⊆ g3` suffices_by metis_tac [mglobals_extend_trans, mglobals_extend_SUBSET]
+    \\ fs [elist_globals_append, SET_OF_BAG_UNION]
+    \\ unabbrev_all_tac \\ rpt (pop_assum kall_tac)
+    \\ metis_tac [UNION_ASSOC, UNION_COMM, SUBSET_UNION])
+  THEN1
+   (say "Let"
+    \\ fs [evaluate_def, pair_case_eq, case_eq_thms]
+    \\ rveq \\ fs []
+    THEN1 (qexists_tac `n + n'` \\ simp [first_n_exps_shift_seq]
+           \\ qmatch_asmsub_abbrev_tac `mglobals_extend s0 g1 s1`
+           \\ qmatch_asmsub_abbrev_tac `mglobals_extend s1 g2 s`
+           \\ qmatch_goalsub_abbrev_tac `mglobals_extend s0 g3 s`
+           \\ `g3 = g1 ∪ g2` suffices_by metis_tac [mglobals_extend_trans]
+           \\ unabbrev_all_tac
+           \\ simp [elist_globals_append, SET_OF_BAG_UNION]
+           \\ metis_tac [UNION_ASSOC, UNION_COMM])
+    THEN1 (qexists_tac `n` \\ simp [SET_OF_BAG_UNION]
+           \\ match_mp_tac mglobals_extend_SUBSET
+           \\ goal_assum drule
+           \\ metis_tac [UNION_ASSOC, UNION_COMM, SUBSET_UNION]))
+  THEN1
+   (say "Raise"
+    \\ fs [evaluate_def, pair_case_eq, case_eq_thms]
+    \\ rveq \\ imp_res_tac evaluate_SING \\ fs [])
+  THEN1
+   (say "Handle"
+    \\ fs [evaluate_def, pair_case_eq, case_eq_thms]
+    \\ rveq \\ fs []
+    \\ fs [SET_OF_BAG_UNION]
+    THEN1 (qexists_tac `n` \\ simp []
+           \\ match_mp_tac mglobals_extend_SUBSET
+           \\ goal_assum drule
+           \\ metis_tac [UNION_ASSOC, UNION_COMM, SUBSET_UNION])
+    THEN1 (qexists_tac `n + n'` \\ simp [first_n_exps_shift_seq]
+           \\ qmatch_asmsub_abbrev_tac `mglobals_extend s0 g1 s1`
+           \\ qmatch_asmsub_abbrev_tac `mglobals_extend s1 g2 s`
+           \\ qmatch_goalsub_abbrev_tac `mglobals_extend s0 g3 s`
+           \\ `g3 = g1 ∪ g2` suffices_by metis_tac [mglobals_extend_trans]
+           \\ fs [elist_globals_append, SET_OF_BAG_UNION]
+           \\ unabbrev_all_tac \\ rpt (pop_assum kall_tac)
+           \\ metis_tac [UNION_ASSOC, UNION_COMM])
+    THEN1 (qexists_tac `n` \\ simp []
+           \\ match_mp_tac mglobals_extend_SUBSET
+           \\ goal_assum drule
+           \\ metis_tac [UNION_ASSOC, UNION_COMM, SUBSET_UNION]))
+  THEN1
+   (say "Op"
+    \\ fs [evaluate_def]
+    \\ reverse (fs [pair_case_eq, result_case_eq]) \\ rveq \\ fs []
+    THEN1 (qexists_tac `n` \\ fs [SET_OF_BAG_UNION]
+           \\ metis_tac [mglobals_extend_SUBSET, UNION_ASSOC, SUBSET_UNION])
+    \\ rename1 `evaluate (_, _, s0) = (_, s1)`
+    \\ Cases_on `op = Install` \\ fs []
+    THEN1
+     (reverse (fs [pair_case_eq, result_case_eq]) \\ rveq \\ fs []
+      THEN1
+       (fs [do_install_def, case_eq_thms, bool_case_eq] \\ rveq \\ fs []
+        \\ TRY (qexists_tac `n` \\ fs [SET_OF_BAG_UNION]
+                \\ metis_tac [mglobals_extend_SUBSET, UNION_ASSOC, SUBSET_UNION])
+        \\ pairarg_tac \\ fs []
+        \\ fs [case_eq_thms, bool_case_eq, pair_case_eq] \\ rveq \\ fs []
+        \\ TRY (qexists_tac `n` \\ fs [SET_OF_BAG_UNION]
+                \\ metis_tac [mglobals_extend_SUBSET, UNION_ASSOC, SUBSET_UNION])
+        \\ conj_tac THEN1 (imp_res_tac ssgc_free_do_install \\ rfs [])
+        \\ TRY (qexists_tac `n + 1`
+                \\ fs [first_n_exps_def, GSYM ADD1, GENLIST,
+                       SNOC_APPEND, elist_globals_append]
+                \\ fs [SET_OF_BAG_UNION]
+                \\ metis_tac [mglobals_extend_SUBSET, UNION_ASSOC, SUBSET_UNION]))
+      \\ drule do_install_ssgc
+      \\ disch_then drule
+      \\ strip_tac \\ fs []
+      \\ qexists_tac `n' + (1 + n)`
+      \\ simp [first_n_exps_shift_seq]
+      \\ rename1 `do_install _ _ = (_, s2)`
+      \\ qmatch_asmsub_abbrev_tac `mglobals_extend s0 g1 s1`
+      \\ qmatch_asmsub_abbrev_tac `mglobals_extend s1 g2 s2`
+      \\ qmatch_asmsub_abbrev_tac `mglobals_extend s2 g3 s`
+      \\ qmatch_goalsub_abbrev_tac `mglobals_extend s0 g4 s`
+      \\ rfs []
+      \\ `g1 ∪ g2 ∪ g3 ⊆ g4` suffices_by metis_tac [mglobals_extend_trans, mglobals_extend_SUBSET]
+      \\ unabbrev_all_tac
+      \\ rpt (pop_assum kall_tac)
+      \\ fs [elist_globals_append, SET_OF_BAG_UNION]
+      \\ metis_tac [UNION_ASSOC, UNION_COMM, SUBSET_UNION])
+    \\ reverse (fs [result_case_eq, pair_case_eq]) \\ rveq \\ fs []
+    \\ drule do_app_ssgc \\ fs [EVERY_REVERSE]
+    \\ strip_tac \\ rveq \\ fs []
+    THEN1 (rename1 `do_app _ _ _ = Rerr err`
+           \\ Cases_on `err` \\ simp []
+           \\ qexists_tac `n` \\ fs [SET_OF_BAG_UNION]
+           \\ metis_tac [mglobals_extend_SUBSET, UNION_ASSOC, SUBSET_UNION])
+    \\ qexists_tac `n` \\ simp []
+    \\ qmatch_asmsub_abbrev_tac `mglobals_extend s0 g1 s1`
+    \\ qmatch_asmsub_abbrev_tac `mglobals_extend s1 g2 s`
+    \\ qmatch_goalsub_abbrev_tac `mglobals_extend s0 g3 s`
+    \\ `g3 = g1 ∪ g2` suffices_by metis_tac [mglobals_extend_trans]
+    \\ unabbrev_all_tac \\ rpt (pop_assum kall_tac)
+    \\ simp [elist_globals_append, SET_OF_BAG_UNION]
+    \\ metis_tac [UNION_ASSOC, UNION_COMM])
+  THEN1
+   (say "Fn"
+    \\ fs [evaluate_def, bool_case_eq, case_eq_thms]
+    \\ rveq \\ fs []
+    \\ imp_res_tac lookup_vars_MEM
+    \\ imp_res_tac lookup_vars_SOME
+    \\ fs [EVERY_EL]
+    \\ qexists_tac `0` \\ simp [])
+  THEN1
+   (say "Letrec"
+    \\ reverse (fs [evaluate_def, bool_case_eq])
+    THEN1 (qexists_tac `0` \\ simp [])
+    \\ fs [Once case_eq_thms] \\ rveq \\ fs []
+    THEN1 (qexists_tac `0` \\ simp [])
+    \\ `EVERY vsgc_free ed`
+       by (fs [case_eq_thms] \\ rveq
+           \\ fs [EVERY_GENLIST]
+           \\ metis_tac [EVERY_lookup_vars])
+    \\ fs [case_eq_thms] \\ rveq \\ fs []
+    \\ qexists_tac `n` \\ simp [])
+  THEN1
+   (say "App"
+    \\ reverse (fs [evaluate_def, bool_case_eq]) \\ rveq \\ fs []
+    THEN1 (qexists_tac `0` \\ simp [])
+    \\ reverse (fs [pair_case_eq, Once case_eq_thms]) \\ rveq \\ fs []
+    THEN1 (qexists_tac `n` \\ simp [SET_OF_BAG_UNION]
+           \\ match_mp_tac mglobals_extend_SUBSET
+           \\ goal_assum drule
+           \\ metis_tac [UNION_ASSOC, UNION_COMM, SUBSET_UNION])
+    \\ reverse (fs [pair_case_eq, case_eq_thms]) \\ rveq \\ fs []
+    THEN1 (qexists_tac `n + n'` \\ simp [first_n_exps_shift_seq]
+           \\ qmatch_asmsub_abbrev_tac `mglobals_extend s0 g1 s1`
+           \\ qmatch_asmsub_abbrev_tac `mglobals_extend s1 g2 s`
+           \\ qmatch_goalsub_abbrev_tac `mglobals_extend s0 g3 s`
+           \\ `g3 = g1 ∪ g2` suffices_by metis_tac [mglobals_extend_trans]
+           \\ unabbrev_all_tac
+           \\ simp [elist_globals_append, SET_OF_BAG_UNION]
+           \\ metis_tac [UNION_ASSOC, UNION_COMM])
+    \\ imp_res_tac evaluate_SING \\ rveq \\ fs []
+    \\ qexists_tac `(n'' + n) + n'` \\ simp [first_n_exps_shift_seq]
+    \\ qmatch_asmsub_abbrev_tac `mglobals_extend s0 g1 s1`
+    \\ qmatch_asmsub_abbrev_tac `mglobals_extend s1 g2 s2`
+    \\ qmatch_asmsub_abbrev_tac `mglobals_extend s2 g3 s`
+    \\ qmatch_goalsub_abbrev_tac `mglobals_extend s0 g4 s`
+    \\ `g1 ∪ g2 ∪ g3 ⊆ g4` suffices_by metis_tac [mglobals_extend_trans, mglobals_extend_SUBSET]
+    \\ fs [elist_globals_append, SET_OF_BAG_UNION]
+    \\ unabbrev_all_tac
+    \\ rpt (pop_assum kall_tac)
+    \\ metis_tac [UNION_ASSOC, UNION_COMM, SUBSET_UNION])
+  THEN1
+   (say "Tick"
+    \\ fs [evaluate_def, bool_case_eq] \\ rveq \\ fs []
+    THEN1 (qexists_tac `0` \\ simp [])
+    \\ qpat_x_assum `_ = evaluate _` (assume_tac o GSYM)
+    \\ fs [dec_clock_def]
+    \\ qexists_tac `n` \\ simp [])
+  THEN1
+   (say "Call"
+    \\ fs [evaluate_def, pair_case_eq, case_eq_thms, bool_case_eq]
+    \\ rveq \\ fs []
+    \\ qpat_x_assum `_ = evaluate _` (assume_tac o GSYM)
+    \\ fs [dec_clock_def]
+    \\ rename [`find_code _ _ s1.code = SOME (args, code)`]
+    \\ fs [find_code_def, case_eq_thms, pair_case_eq, bool_case_eq]
+    \\ rveq \\ fs []
+    \\ `set_globals code = {||}` by metis_tac [ssgc_free_def]
+    \\ fs [set_globals_empty_esgc_free]
+    \\ qexists_tac `n' + n` \\ simp [first_n_exps_shift_seq]
+    \\ qmatch_asmsub_abbrev_tac `mglobals_extend s0 g1 s1`
+    \\ qmatch_asmsub_abbrev_tac `mglobals_extend s1 g2 s`
+    \\ qmatch_goalsub_abbrev_tac `mglobals_extend s0 g3 s`
+    \\ `g3 = g1 ∪ g2` suffices_by metis_tac [mglobals_extend_trans]
+    \\ fs [elist_globals_append, SET_OF_BAG_UNION]
+    \\ metis_tac [UNION_ASSOC, UNION_COMM])
+  THEN1
+   (say "evaluate_app NIL"
+    \\ fs [] \\ rveq \\ simp []
+    \\ qexists_tac `0` \\ simp [])
+  THEN1
+   (say "evaluate_app CONS"
+    \\ fs [evaluate_def]
+    \\ fs [case_eq_thms] \\ rveq \\ fs []
+    THEN1 (qexists_tac `0` \\ simp [])
+    THEN1 (fs [bool_case_eq] \\ rveq \\ fs []
+           THEN1 (qexists_tac `0` \\ simp [])
+           \\ fs [dest_closure_def, case_eq_thms]
+           \\ rpt (pairarg_tac \\ fs [])
+           \\ fs [bool_case_eq]
+           \\ rveq \\ fs [dec_clock_def]
+           \\ qexists_tac `0` \\ simp [])
+    \\ fs [bool_case_eq] \\ rveq \\ fs []
+    THEN1 (qexists_tac `0` \\ simp [])
+    \\ fs [pair_case_eq] \\ fs []
+    \\ drule dest_closure_Full_sgc_free \\ simp [] \\ strip_tac
+    \\ fs [set_globals_empty_esgc_free, dec_clock_def]
+    \\ fs [case_eq_thms] \\ rveq \\ fs []
+    THEN1 (qexists_tac `n' + n` \\ simp [first_n_exps_shift_seq]
+           \\ qmatch_asmsub_abbrev_tac `mglobals_extend s0 g1 s1`
+           \\ qmatch_asmsub_abbrev_tac `mglobals_extend s1 g2 s`
+           \\ qmatch_goalsub_abbrev_tac `mglobals_extend s0 g3 s`
+           \\ `g3 = g1 ∪ g2` suffices_by metis_tac [mglobals_extend_trans]
+           \\ fs [elist_globals_append, SET_OF_BAG_UNION]
+           \\ metis_tac [UNION_ASSOC, UNION_COMM])
+    \\ qexists_tac `n` \\ fs []));
+
+val evaluate_changed_globals = save_thm(
+   "evaluate_changed_globals",
+   CONJUNCT1 evaluate_changed_globals_0);
+
+val evaluate_app_changed_globals = save_thm(
+   "evaluate_app_changed_globals",
+   CONJUNCT2 evaluate_changed_globals_0);
+
+
+val mk_Ticks_set_globals = Q.store_thm(
+  "mk_Ticks_set_globals[simp]",
+  `!t tc n exp. set_globals (mk_Ticks t tc n exp) = set_globals exp`,
+  Induct_on `n` \\ simp [mk_Ticks_def]);
+
+
+val mglobals_extend_DISJOINT_state_globals_approx = Q.store_thm(
+  "mglobals_extend_DISJOINT_state_globals_approx",
+  `!s1 gd s2 g. mglobals_extend s1 gd s2 /\ state_globals_approx s1 g /\ DISJOINT (domain g) gd ==>
+   state_globals_approx s2 g`,
+  rpt strip_tac
+  \\ simp [state_globals_approx_def]
+  \\ rpt gen_tac \\ strip_tac
+  \\ fs [mglobals_extend_def]
+  \\ first_x_assum drule
+  \\ reverse (Cases_on `k ∈ gd`)
+  \\ fs []
+  THEN1 (fs [state_globals_approx_def] \\ metis_tac [])
+  THEN1 (`k ∉ domain g` by fs [Once DISJOINT_SYM, DISJOINT_ALT]
+         \\ fs [domain_lookup]));
+
+
+val known_op_install_correct_approx = Q.store_thm("known_op_install_correct_approx",
+  `!args g0 a g vs (s0:('c, 'ffi) closSem$state) g' e s1 res s.
+   known_op Install args g0 = (a,g) /\
+   do_install vs s0 = (Rval e, s1) /\
+   LIST_REL val_approx_val args vs /\
+   co_disjoint_globals g' s0.compile_oracle /\
+   state_globals_approx s0 g' /\
+   ssgc_free s0 /\
+   evaluate ([e], [], s1) = (res, s) ⇒
+   state_globals_approx s g'`,
+  rpt gen_tac \\ disch_then strip_assume_tac
+  \\ drule evaluate_changed_globals
+  \\ imp_res_tac do_install_ssgc \\ simp []
+  \\ strip_tac
+  \\ qmatch_asmsub_abbrev_tac `mglobals_extend s1 gd s`
+  \\ `gd = SET_OF_BAG (elist_globals (first_n_exps s0.compile_oracle (n + 1)))`
+     by simp [first_n_exps_shift_seq, SET_OF_BAG_UNION]
+  \\ `DISJOINT (domain g') gd`
+     by simp [co_disjoint_globals_first_n_exps]
+  \\ `state_globals_approx s1 g'`
+     by (fs [do_install_def, case_eq_thms] \\ rveq \\ fs []
+         \\ pairarg_tac \\ fs []
+         \\ fs [bool_case_eq, pair_case_eq, case_eq_thms])
+  \\ metis_tac [mglobals_extend_DISJOINT_state_globals_approx]);
+
+val mk_Ticks_esgc_free = Q.store_thm(
+  "mk_Ticks_esgc_free[simp]",
+  `!t tc n exp. esgc_free (mk_Ticks t tc n exp) <=> esgc_free exp`,
+  Induct_on `n` \\ fs [mk_Ticks_def]);
+
+
+val val_approx_sgc_free_def = tDefine "val_approx_gc_free" `
+  (val_approx_sgc_free (Clos m n NONE) <=> T) /\
+  (val_approx_sgc_free (Clos m n (SOME e)) <=> set_globals e = {||}) /\
+  (val_approx_sgc_free (Tuple tag vas) <=> EVERY val_approx_sgc_free vas) /\
+  (val_approx_sgc_free _ <=> T)
+` (WF_REL_TAC `measure val_approx_size`
+   \\ Induct_on `vas` \\ simp []
+   \\ rw [] THEN1 simp [val_approx_size_def]
+   \\ first_x_assum drule
+   \\ disch_then (qspec_then `tag` assume_tac)
+   \\ fs [val_approx_size_def]);
+
+val val_approx_sgc_free_def = save_thm(
+  "val_approx_sgc_free_def[simp]",
+  val_approx_sgc_free_def |> SIMP_RULE (srw_ss() ++ ETA_ss) []);
+
+val val_approx_sgc_free_merge = Q.store_thm(
+  "val_approx_sgc_free_merge",
+  `!a1 a2. val_approx_sgc_free a1 /\ val_approx_sgc_free a2 ==>
+   val_approx_sgc_free (merge a1 a2)`,
+  ho_match_mp_tac merge_ind \\ simp []
+  \\ rpt strip_tac
+  \\ IF_CASES_TAC \\ fs [] \\ rveq
+  \\ fs [EVERY_MEM]
+  \\ simp [MAP2_MAP, MEM_MAP, PULL_EXISTS]
+  \\ simp [MEM_ZIP, PULL_EXISTS]
+  \\ fs [MEM_EL]
+  \\ metis_tac []);
+
+val globals_approx_sgc_free_def = Define `
+  globals_approx_sgc_free g <=>
+  !n a. lookup n g = SOME a ==> val_approx_sgc_free a`;
+
+val known_op_preserves_esgc_free = Q.store_thm(
+  "known_op_preserves_esgc_free",
+  `!opn args g0 a g.
+     known_op opn args g0 = (a, g) /\
+     EVERY val_approx_sgc_free args /\
+     globals_approx_sgc_free g0 ==>
+     val_approx_sgc_free a /\ globals_approx_sgc_free g
+`,
+  rpt gen_tac \\ strip_tac
+  \\ Cases_on `opn`
+  \\ fs [known_op_def] \\ rveq \\ fs []
+  THEN1 (fs [bool_case_eq, case_eq_thms] \\ rveq \\ fs []
+         \\ metis_tac [globals_approx_sgc_free_def])
+  THEN1 (fs [case_eq_thms] \\ rveq \\ fs []
+         \\ fs [globals_approx_sgc_free_def]
+         \\ rw [] \\ fs [lookup_insert, bool_case_eq]
+         \\ metis_tac [val_approx_sgc_free_merge])
+  THEN1 (fs [case_eq_thms, va_case_eq, bool_case_eq] \\ rveq \\ fs []
+         \\ imp_res_tac integerTheory.NUM_POSINT_EXISTS \\ fs []
+         \\ fs [EVERY_EL]));
+
+val elist_globals_empty = Q.store_thm(
+  "elist_globals_empty",
+  `!es. elist_globals es = {||} <=>
+        !e. MEM e es ==> set_globals e = {||}`,
+  Induct \\ fs [] \\ rw [] \\ eq_tac \\ rw [] \\ fs []);
+
+val clos_gen_noinline_val_approx_sgc_free = Q.store_thm(
+  "clos_gen_noinline_val_approx_sgc_free",
+  `!n i fns. elist_globals (MAP SND fns) = {||} ==>
+               EVERY val_approx_sgc_free (clos_gen_noinline n i fns)`,
+  ho_match_mp_tac clos_gen_noinline_ind
+  \\ rw [] \\ fs [clos_gen_noinline_def, clos_approx_def]);
+
+val known_preserves_esgc_free_0 = Q.store_thm(
+  "known_preserves_esgc_free_0",
+  `!limit es aenv g0 eas1 g.
+     known limit es aenv g0 = (eas1, g) /\
+     EVERY esgc_free es /\
+     EVERY val_approx_sgc_free aenv /\
+     globals_approx_sgc_free g0 ==>
+     elist_globals (MAP FST eas1) ≤ elist_globals es /\
+     EVERY esgc_free (MAP FST eas1) /\
+     EVERY val_approx_sgc_free (MAP SND eas1) /\
+     globals_approx_sgc_free g`,
+  ho_match_mp_tac known_ind
+  \\ rpt conj_tac \\ rpt (gen_tac ORELSE disch_then strip_assume_tac)
+  \\ fs [known_def] \\ rpt (pairarg_tac \\ fs []) \\ rveq
+  \\ imp_res_tac known_sing_EQ_E \\ fs [] \\ rveq \\ fs []
+  \\ simp [val_approx_sgc_free_merge, SUB_BAG_UNION]
+  THEN1 (simp [any_el_ALT] \\ IF_CASES_TAC \\ fs [EVERY_EL])
+  THEN1 (drule known_op_preserves_esgc_free
+         \\ simp [EVERY_REVERSE]
+         \\ strip_tac
+         \\ every_case_tac \\ simp []
+         \\ rename [`isGlobal opn`] \\ Cases_on `opn` \\ fs [isGlobal_def]
+         \\ fs [known_op_def, op_gbag_def])
+  THEN1 (fs [bool_case_eq, SUB_BAG_UNION]
+         \\ Cases_on `body_opt` \\ fs [SUB_BAG_UNION]
+         \\ fs [bool_case_eq]
+         \\ rpt (pairarg_tac \\ fs []) \\ rveq
+         \\ fs [case_eq_thms, pair_case_eq, bool_case_eq] \\ rveq
+         \\ imp_res_tac known_sing_EQ_E \\ fs [] \\ rveq
+         \\ imp_res_tac set_globals_empty_esgc_free \\ fs []
+         \\ fs [SNOC_APPEND, elist_globals_append, SUB_BAG_UNION])
+  THEN1 (fs [EVERY_REPLICATE]
+         \\ imp_res_tac set_globals_empty_esgc_free \\ fs []
+         \\ TOP_CASE_TAC \\ simp [clos_approx_def]
+         \\ IF_CASES_TAC \\ simp [])
+  THEN1 (Cases_on `loc_opt` \\ fs []
+         \\ imp_res_tac clos_gen_noinline_val_approx_sgc_free \\ fs [] \\ pop_assum kall_tac
+         \\ fs [EVERY_REPLICATE]
+         \\ conj_asm2_tac \\ simp []
+         \\ fs [elist_globals_empty]
+         \\ simp [MAP_MAP_o, o_DEF, LAMBDA_PROD]
+         \\ simp [MEM_MAP] \\ rw []
+         \\ qmatch_assum_rename_tac `MEM fff fns`
+         \\ `MEM (SND fff) (MAP SND fns)` by metis_tac [MEM_MAP]
+         \\ PairCases_on `fff` \\ fs []
+         \\ first_x_assum drule \\ strip_tac
+         \\ imp_res_tac set_globals_empty_esgc_free
+         \\ qmatch_goalsub_abbrev_tac `known limit k1 k2 k3`
+         \\ Cases_on `known limit k1 k2 k3`
+         \\ unabbrev_all_tac
+         \\ imp_res_tac known_sing_EQ_E
+         \\ fs [] \\ rveq
+         \\ first_x_assum drule \\ fs []));
+
+val known_preserves_esgc_free = Q.store_thm(
+  "known_preserves_esgc_free",
+  `!limit es aenv g0 eas1 g.
+     known limit es aenv g0 = (eas1, g) /\
+     EVERY esgc_free es /\
+     EVERY val_approx_sgc_free aenv /\
+     globals_approx_sgc_free g0 ==>
+     EVERY esgc_free (MAP FST eas1) /\
+     EVERY val_approx_sgc_free (MAP SND eas1) /\
+     globals_approx_sgc_free g`,
+  rpt gen_tac \\ rpt (disch_then strip_assume_tac)
+  \\ metis_tac [known_preserves_esgc_free_0]);
+
+val known_elglobals_dont_grow = Q.store_thm(
+  "known_elglobals_dont_grow",
+  `!limit es aenv g0 eas1 g.
+     known limit es aenv g0 = (eas1, g) /\
+     EVERY esgc_free es /\
+     EVERY val_approx_sgc_free aenv /\
+     globals_approx_sgc_free g0 ==>
+     elist_globals (MAP FST eas1) ≤ elist_globals es`,
+  rpt gen_tac \\ rpt (disch_then strip_assume_tac)
+  \\ metis_tac [known_preserves_esgc_free_0]);
+
+val known_preserves_pure = Q.store_thm(
+  "known_preserves_pure",
+  `!limit es aenv g0 eas1 g.
+     known limit es aenv g0 = (eas1, g) /\
+     EVERY pure es ==>
+     EVERY pure (MAP FST eas1)`,
+  ho_match_mp_tac known_ind
+  \\ simp [known_def]
+  \\ rpt strip_tac
+  \\ rpt (pairarg_tac \\ fs [])
+  \\ imp_res_tac known_sing_EQ_E
+  \\ fs [] \\ rveq
+  \\ fs [closLangTheory.pure_def]
+  \\ every_case_tac
+  \\ fs [closLangTheory.pure_def, closLangTheory.pure_op_def, ETA_THM]);
+
+val evaluate_mk_Ticks = Q.store_thm(
+  "evaluate_mk_Ticks",
+  `!t tc n exp env (s0:('c,'ffi) closSem$state) res s.
+     evaluate ([mk_Ticks t tc n exp], env, s0) = (res, s) ==>
+     (res = Rerr (Rabort Rtimeout_error) /\ s = s0 with clock := 0) \/
+     (evaluate ([exp], env, dec_clock n s0) = (res, s))`,
+  Induct_on `n` \\ rpt strip_tac
+  THEN1 (fs [mk_Ticks_def, dec_clock_def])
+  \\ fs [mk_Ticks_def, evaluate_def]
+  \\ Cases_on `s0.clock = 0` \\ fs []
+  THEN1 (rveq \\ simp [state_component_equality])
+  \\ res_tac
+  \\ fs [dec_clock_def, ADD1])
+
+
+val evaluate_mk_Ticks_EQ = Q.store_thm(
+  "evaluate_mk_Ticks_EQ",
+  `!t tc n exp env (s:('c,'ffi) closSem$state).
+     evaluate ([mk_Ticks t tc n exp], env, s) =
+     if s.clock < n then (Rerr (Rabort Rtimeout_error), s with clock := 0)
+     else evaluate ([exp], env, dec_clock n s)`,
+  Induct_on `n`
+  THEN1 simp [mk_Ticks_def, dec_clock_def]
+  \\ rw []
+  \\ fs [mk_Ticks_def, evaluate_def, dec_clock_def, ADD1]
+  \\ IF_CASES_TAC \\ simp [state_component_equality])
+
+val clos_gen_noinline_eq = Q.prove(`
+  !n c fns.
+  clos_gen_noinline n c fns =
+  GENLIST (λi. Clos (2 * (i+c) + n) (FST (EL i fns)) NONE) (LENGTH fns)`,
+  Induct_on`fns`>>fs[FORALL_PROD,clos_gen_noinline_def,GENLIST_CONS]>>rw[]>>
+  simp[o_DEF,ADD1])
+
+
+val letrec_case_eq = Q.prove(`
+  !limit loc fns.
+  (case loc of
+    NONE => REPLICATE (LENGTH fns) Other
+  | SOME n => clos_gen_noinline n 0 fns) =
+  GENLIST (case loc of NONE => K Other |
+                       SOME n => λi. Clos (n + 2*i) (FST (EL i fns)) NONE) (LENGTH fns)`,
+  Cases_on`loc`>>fs[clos_gen_noinline_eq,REPLICATE_GENLIST])
+
+
+val say = say0 "known_correct_approx";
+
+val known_correct_approx = Q.store_thm(
+  "known_correct_approx",
+  `!limit es aenv g1 eas g g' env (s1:('c, 'ffi) closSem$state) res s.
+   known limit es aenv g1 = (eas,g) /\
+   evaluate (MAP FST eas, env, s1) = (res, s) /\
+   unique_set_globals es s1.compile_oracle /\
+   LIST_REL val_approx_val aenv env /\
+   state_globals_approx s1 g' /\
+   subspt g1 g /\ subspt g g' /\
+   co_disjoint_globals g' s1.compile_oracle /\
+   ssgc_free s1 /\ EVERY vsgc_free env /\ EVERY esgc_free es /\
+   EVERY val_approx_sgc_free aenv /\ globals_approx_sgc_free g1 ==>
+     state_globals_approx s g' /\
+     !vs. res = Rval vs ==> LIST_REL val_approx_val (MAP SND eas) vs`,
+  (**)
+  ho_match_mp_tac known_ind \\ simp [known_def]
+  \\ rpt conj_tac \\ rpt (gen_tac ORELSE disch_then strip_assume_tac)
+  THEN1
+   (say "NIL" \\ fs [evaluate_def] \\ rveq \\ fs [])
+  THEN1
+   (say "CONS"
+    \\ rpt (pairarg_tac \\ fs []) \\ rveq
+    \\ imp_res_tac known_LENGTH_EQ_E
+    \\ fs [LENGTH_EQ_NUM, LENGTH_EQ_NUM_compute]
+    \\ rveq \\ fs []
+    \\ rename1 `known limit [exp1] aenv g1 = ([ea1], g2)`
+    \\ `?exp1' a1. ea1 = (exp1', a1)` by (Cases_on `ea1` \\ simp []) \\ rveq
+    \\ rename1 `known limit (exp2::exps) aenv g2 = (ea2::eas, g)`
+    \\ `?exp2' a2. ea2 = (exp2', a2)` by (Cases_on `ea2` \\ simp []) \\ rveq
+    \\ fs []
+    \\ fs [evaluate_def]
+    \\ `?res1 s2. evaluate ([exp1'],env,s1) = (res1, s2)` by fs [pair_case_eq]
+    \\ `?res2 s3. evaluate (exp2'::MAP FST eas,env,s2) = (res2, s3)`
+         by (Cases_on `evaluate (exp2'::MAP FST eas,env,s2)` \\ fs [])
+    \\ imp_res_tac unique_set_globals_subexps
+    \\ `unique_set_globals (exp2::exps) s2.compile_oracle`
+         by (imp_res_tac evaluate_code \\ metis_tac [unique_set_globals_shift_seq])
+    \\ `subspt g1 g2 /\ subspt g2 g`
+       by (match_mp_tac subspt_known_elist_globals
+           \\ asm_exists_tac \\ simp []
+           \\ goal_assum drule
+           \\ fs [unique_set_globals_def,elist_globals_append]
+           \\ fs [BAG_ALL_DISTINCT_BAG_UNION])
+    \\ `subspt g2 g'` by metis_tac [subspt_trans]
+    \\ patresolve `known _ [_] _ _ = _` (el 1) known_preserves_esgc_free
+    \\ simp [] \\ strip_tac
+    \\ `ssgc_free s2`
+       by (patresolve `ssgc_free _` (el 2) evaluate_changed_globals
+           \\ rpt (disch_then drule \\ simp []))
+    \\ drule co_disjoint_globals_evaluate \\ disch_then drule \\ strip_tac
+    \\ REPEAT (first_x_assum drule
+               \\ rpt (disch_then drule)
+               \\ fs [] \\ strip_tac)
+    \\ Cases_on `res1` \\ fs [] \\ rveq \\ fs []
+    \\ Cases_on `res2` \\ fs [] \\ rveq \\ fs [])
+  THEN1
+   (say "Var"
+    \\ fs [evaluate_def, bool_case_eq] \\ rveq
+    \\ fs [any_el_ALT] \\ fs [LIST_REL_EL_EQN])
+  THEN1
+   (say "If"
+    \\ rpt (pairarg_tac \\ fs []) \\ rveq
+    \\ imp_res_tac known_sing_EQ_E \\ fs [] \\ rveq
+    \\ rename1 `known limit [x1] aenv g1 = ([(e1,a1)], g2)`
+    \\ rename1 `known limit [x2] aenv g2 = ([(e2,a2)], g3)`
+    \\ rename1 `known limit [x3] aenv g3 = ([(e3,a3)], g4)`
+    \\ imp_res_tac unique_set_globals_subexps
+    \\ fs [evaluate_def]
+    \\ fs [pair_case_eq]
+    \\ `subspt g1 g2 /\ subspt g2 g3 /\ subspt g3 g4`
+       by (`?unused. known limit [x1;x2] aenv g1 = (unused, g3)` by simp [known_def]
+           \\ drule subspt_known_elist_globals
+           \\ rpt (disch_then drule)
+           \\ impl_tac THEN1 fs [unique_set_globals_def,BAG_ALL_DISTINCT_BAG_UNION]
+           \\ strip_tac \\ simp []
+           \\ match_mp_tac subspt_known_elist_globals
+           \\ asm_exists_tac \\ simp []
+           \\ goal_assum drule
+           \\ fs [unique_set_globals_def,BAG_ALL_DISTINCT_BAG_UNION])
+    \\ `subspt g2 g' /\ subspt g3 g'` by metis_tac [subspt_trans]
+    \\ first_x_assum drule
+    \\ rpt (disch_then drule)
+    \\ strip_tac
+    \\ rename1 `evaluate ([e1],env,s1) = (res1, s2)`
+    \\ Cases_on `res1` \\ fs [] \\ rveq \\ fs []
+    \\ rename1 `evaluate ([e1],env,s1) = (Rval [vcond],s2)`
+    \\ Cases_on `Boolv T = vcond \/ Boolv F = vcond`
+    \\ fs [] \\ rveq \\ fs []
+    \\ rename1 `evaluate ([e_taken_branch],env,s2) = (res, s)`
+    \\ rename1 `known limit [x_taken_branch] aenv _ = ([e_taken_branch,_],_)`
+    \\ `unique_set_globals [x_taken_branch] s2.compile_oracle`
+         by metis_tac [unique_set_globals_evaluate]
+    \\ rpt (qpat_x_assum `unique_set_globals _ s1.compile_oracle` kall_tac)
+    \\ drule co_disjoint_globals_evaluate \\ disch_then drule \\ strip_tac
+    \\ patresolve `known _ _ _ g1 = _` (el 1) known_preserves_esgc_free
+    \\ simp [] \\ strip_tac
+    \\ patresolve `known _ _ _ g2 = _` (el 1) known_preserves_esgc_free
+    \\ simp [] \\ strip_tac
+    \\ `ssgc_free s2`
+       by (patresolve `ssgc_free _` (el 2) evaluate_changed_globals
+           \\ rpt (disch_then drule \\ simp []))
+    \\ first_x_assum drule
+    \\ rpt (disch_then drule)
+    \\ strip_tac
+    \\ Cases_on `res` \\ fs [] \\ rveq
+    \\ fs [val_approx_val_merge_I])
+  THEN1
+   (say "Let"
+    \\ rpt (pairarg_tac \\ fs []) \\ rveq
+    \\ imp_res_tac known_sing_EQ_E \\ fs [] \\ rveq
+    \\ rename1 `known limit xs aenv g1 = (ea1, g2)`
+    \\ rename1 `known limit [x2] _ g2 = ([(e2,a2)], g3)`
+    \\ imp_res_tac unique_set_globals_subexps
+    \\ fs [evaluate_def, pair_case_eq]
+    \\ `subspt g1 g2 /\ subspt g2 g3`
+       by (match_mp_tac subspt_known_elist_globals
+           \\ rpt (asm_exists_tac \\ simp [])
+           \\ fs [unique_set_globals_def,
+                  BAG_ALL_DISTINCT_BAG_UNION, BAG_DISJOINT_SYM])
+    \\ `subspt g2 g'` by metis_tac [subspt_trans]
+    \\ first_x_assum drule
+    \\ rpt (disch_then drule)
+    \\ strip_tac
+    \\ fs [case_eq_thms] \\ rveq \\ fs []
+    \\ rename1 `evaluate (MAP FST ea1,env,s1) = (Rval vs, s2)`
+    \\ `unique_set_globals [x2] s2.compile_oracle`
+         by metis_tac [unique_set_globals_evaluate]
+    \\ drule co_disjoint_globals_evaluate \\ disch_then drule \\ strip_tac
+    \\ patresolve `known _ _ _ g1 = _` (el 1) known_preserves_esgc_free
+    \\ simp [] \\ strip_tac \\ fs []
+    \\ `ssgc_free s2 /\ EVERY vsgc_free vs`
+       by (patresolve `ssgc_free _` (el 2) evaluate_changed_globals
+           \\ rpt (disch_then drule \\ simp []))
+    \\ first_x_assum irule \\ simp []
+    \\ qexists_tac `vs ++ env`
+    \\ qexists_tac `s2` \\ fs []
+    \\ irule EVERY2_APPEND_suff \\ fs [])
+  THEN1
+   (say "Raise"
+    \\ rpt (pairarg_tac \\ fs []) \\ rveq
+    \\ imp_res_tac known_sing_EQ_E \\ fs [] \\ rveq
+    \\ rename1 `known limit [x1] aenv g1 = ([(e1,a1)], g2)`
+    \\ imp_res_tac unique_set_globals_subexps
+    \\ fs [evaluate_def, pair_case_eq]
+    \\ first_x_assum drule
+    \\ rpt (disch_then drule)
+    \\ strip_tac
+    \\ fs [case_eq_thms] \\ rveq
+    \\ simp [])
+  THEN1
+   (say "Tick"
+    \\ rpt (pairarg_tac \\ fs []) \\ rveq
+    \\ imp_res_tac known_sing_EQ_E \\ fs [] \\ rveq
+    \\ imp_res_tac unique_set_globals_subexps
+    \\ fs [evaluate_def, pair_case_eq]
+    \\ Cases_on `s1.clock = 0` \\ fs [] \\ rveq \\ fs []
+    \\ first_x_assum (qpat_assum `evaluate _ = _` o mp_then Any match_mp_tac)
+    \\ fs [dec_clock_def])
+  THEN1
+   (say "Handle"
+    \\ rpt (pairarg_tac \\ fs []) \\ rveq
+    \\ imp_res_tac known_sing_EQ_E \\ fs [] \\ rveq
+    \\ rename1 `known limit [x1] _ g1 = ([(e1,a1)], g2)`
+    \\ rename1 `known limit [x2] _ g2 = ([(e2,a2)], g3)`
+    \\ imp_res_tac unique_set_globals_subexps
+    \\ fs [evaluate_def, pair_case_eq]
+    \\ `subspt g1 g2 /\ subspt g2 g3`
+       by (match_mp_tac subspt_known_elist_globals
+           \\ rpt (asm_exists_tac \\ simp [])
+           \\ fs [unique_set_globals_def,
+                  BAG_ALL_DISTINCT_BAG_UNION, BAG_DISJOINT_SYM])
+    \\ `subspt g2 g'` by metis_tac [subspt_trans]
+    \\ first_x_assum drule
+    \\ rpt (disch_then drule)
+    \\ strip_tac
+    \\ fs [case_eq_thms] \\ rveq \\ fs []
+    THEN1 (fs [val_approx_val_merge_I])
+    \\ rename1 `evaluate (_,_,s1) = (Rerr (Rraise v), s2)`
+    \\ `unique_set_globals [x2] s2.compile_oracle`
+         by metis_tac [unique_set_globals_evaluate]
+    \\ drule co_disjoint_globals_evaluate \\ disch_then drule \\ strip_tac
+    \\ patresolve `known _ _ _ g1 = _` (el 1) known_preserves_esgc_free
+    \\ simp [] \\ strip_tac \\ fs []
+    \\ `ssgc_free s2 /\ vsgc_free v`
+       by (patresolve `ssgc_free _` (el 2) evaluate_changed_globals
+           \\ rpt (disch_then drule \\ simp []))
+    \\ first_x_assum (qpat_assum `evaluate (_,_,s2) = _` o mp_then Any mp_tac)
+    \\ simp []
+    \\ rpt (disch_then drule)
+    \\ strip_tac
+    \\ Cases_on `res`
+    \\ fs [val_approx_val_merge_I])
+  THEN1
+   (say "Call"
+    \\ rpt (pairarg_tac \\ fs []) \\ rveq
+    \\ fs [evaluate_def, pair_case_eq]
+    \\ imp_res_tac unique_set_globals_subexps
+    \\ first_x_assum drule
+    \\ rpt (disch_then drule)
+    \\ strip_tac
+    \\ patresolve `known _ _ _ g1 = _` (el 1) known_preserves_esgc_free
+    \\ simp [] \\ strip_tac
+    \\ fs [case_eq_thms] \\ rveq \\ fs []
+    \\ fs [pair_case_eq] \\ rveq
+    \\ rename1 `evaluate (_,_,s1) = (Rval vs, s2)`
+    \\ Cases_on `s2.clock < ticks + 1`
+    \\ fs [] \\ rveq \\ fs []
+    \\ `ssgc_free s2 /\ EVERY vsgc_free vs`
+       by (patresolve `ssgc_free _` (el 2) evaluate_changed_globals
+           \\ rpt (disch_then drule \\ simp []))
+    \\ rename1 `find_code _ _ _ = SOME (args, exp)`
+    \\ `set_globals exp = {||} /\ EVERY vsgc_free args`
+       by (fs [find_code_def, case_eq_thms, pair_case_eq]
+           \\ metis_tac [ssgc_free_def])
+    \\ patresolve `evaluate ([exp],_,_) = _` (el 1) evaluate_changed_globals
+    \\ simp [dec_clock_def, set_globals_empty_esgc_free]
+    \\ strip_tac
+    \\ drule mglobals_extend_DISJOINT_state_globals_approx
+    \\ disch_then drule
+    \\ impl_tac
+    THEN1 metis_tac [co_disjoint_globals_first_n_exps, co_disjoint_globals_evaluate]
+    \\ metis_tac [evaluate_SING])
+  THEN1
+   (say "Op"
+    \\ rpt (pairarg_tac \\ fs []) \\ rveq
+    \\ rename1 `known limit xs aenv g1 = (ea1, g2)`
+    \\ rename1 `[Op _ opn _]`
+    \\ imp_res_tac unique_set_globals_subexps
+    \\ `subspt g1 g2 /\ subspt g2 g`
+       by (match_mp_tac subspt_known_op_elist_globals
+           \\ rpt (goal_assum drule)
+           \\ fs [unique_set_globals_def, BAG_ALL_DISTINCT_BAG_UNION])
+    \\ `subspt g2 g'` by metis_tac [subspt_trans]
+    \\ Cases_on `opn = Install`
+    THEN1
+     (rveq \\ fs [isGlobal_def]
+      \\ reverse conj_tac
+      THEN1 (Cases_on `res` \\ fs [known_op_def]
+             \\ imp_res_tac evaluate_SING
+             \\ rveq \\ simp [])
+      \\ fs [evaluate_def]
+      \\ fs [pair_case_eq]
+      \\ first_x_assum drule
+      \\ rpt (disch_then drule)
+      \\ strip_tac
+      \\ reverse (fs [case_eq_thms, pair_case_eq]) \\ rveq \\ fs []
+      THEN1 (fs [do_install_def, case_eq_thms] \\ rveq \\ fs []
+             \\ pairarg_tac \\ fs []
+             \\ fs [bool_case_eq, pair_case_eq, case_eq_thms] \\ rveq \\ fs [])
+      \\ rename1 `do_install _ s2 = (_, s3)`
+      \\ `ssgc_free s2`
+         by (patresolve `ssgc_free _` (el 2) evaluate_changed_globals
+             \\ rpt (disch_then drule)
+             \\ drule known_preserves_esgc_free \\ simp [])
+      \\ imp_res_tac EVERY2_REVERSE \\ simp []
+      \\ match_mp_tac known_op_install_correct_approx
+      \\ rpt (goal_assum drule \\ simp [])
+      \\ metis_tac [co_disjoint_globals_evaluate])
+    \\ Cases_on `isGlobal opn` \\ fs []
+    THENL
+     [Cases_on `opn` \\ fs [isGlobal_def]
+      \\ rename1 `gO_destApx apx`
+      \\ Cases_on `gO_destApx apx` \\ fs []
+      \\ fs [evaluate_def]
+      THEN1 (fs [do_app_def] \\ rveq
+             \\ Cases_on `apx` \\ fs [gO_destApx_def, bool_case_eq])
+      THEN1 (fs [do_app_def] \\ rveq
+             \\ Cases_on `apx` \\ fs [gO_destApx_def, bool_case_eq, NULL_EQ]),
+      fs [evaluate_def]]
+    \\ fs [pair_case_eq]
+    \\ first_x_assum drule
+    \\ rpt (disch_then drule)
+    \\ strip_tac
+    \\ fs [case_eq_thms, pair_case_eq] \\ rveq \\ fs []
+    \\ irule known_op_correct_approx
+    \\ rpt (goal_assum drule \\ simp [])
+    \\ irule EVERY2_REVERSE \\ simp [])
+  THEN1
+   (say "App"
+    \\ rpt (pairarg_tac \\ fs []) \\ rveq
+    \\ imp_res_tac known_sing_EQ_E \\ fs [] \\ rveq
+    \\ rename1 `known _ [_] _ g2 = (_, g3)`
+    \\ Cases_on `SND limit = 0 \/ body_opt = NONE`
+    THEN1 (* depth_limit = 0 *)
+     (fs [] THEN (fs [] \\ rveq \\ fs []
+      \\ fs [evaluate_def, bool_case_eq, pair_case_eq]
+      \\ imp_res_tac unique_set_globals_subexps
+      \\ `subspt g1 g2 /\ subspt g2 g`
+         by (match_mp_tac subspt_known_elist_globals
+             \\ rpt (goal_assum drule)
+             \\ fs [unique_set_globals_def, BAG_ALL_DISTINCT_BAG_UNION, BAG_DISJOINT_SYM])
+      \\ `subspt g2 g'` by metis_tac [subspt_trans]
+      \\ first_x_assum drule
+      \\ rpt (disch_then drule)
+      \\ strip_tac
+      \\ fs [result_case_eq] \\ rveq \\ fs []
+      \\ rename1 `evaluate (MAP FST ea2, env, s1) = (Rval args, s2)`
+      \\ `unique_set_globals [x] s2.compile_oracle`
+         by metis_tac [unique_set_globals_evaluate]
+      \\ drule co_disjoint_globals_evaluate \\ disch_then drule \\ strip_tac
+      \\ patresolve `known _ _ _ g1 = _` (el 1) known_preserves_esgc_free
+      \\ simp [] \\ strip_tac
+      \\ `ssgc_free s2 /\ EVERY vsgc_free args`
+         by (patresolve `ssgc_free _` (el 2) evaluate_changed_globals
+             \\ rpt (disch_then drule \\ simp []))
+      \\ fs [pair_case_eq]
+      \\ first_x_assum drule
+      \\ rpt (disch_then drule)
+      \\ strip_tac
+      \\ fs [result_case_eq] \\ rveq \\ fs [] \\ rveq \\ fs []
+      \\ reverse conj_tac
+      THEN1 (Cases_on `res` \\ imp_res_tac evaluate_app_IMP_LENGTH
+             \\ fs [LENGTH_EQ_NUM_compute])
+      \\ rename1 `evaluate ([_], _, s2) = (Rval [fval], s3)`
+      \\ patresolve `known _ _ _ g2 = _` (el 1) known_preserves_esgc_free
+      \\ simp [] \\ strip_tac
+      \\ `ssgc_free s3 /\ vsgc_free fval`
+         by (patresolve `ssgc_free _` (el 2) evaluate_changed_globals
+             \\ rpt (disch_then drule \\ simp []))
+      \\ drule evaluate_app_changed_globals \\ simp [] \\ strip_tac
+      \\ drule co_disjoint_globals_evaluate \\ disch_then drule \\ strip_tac
+      \\ qmatch_asmsub_abbrev_tac `mglobals_extend _ gd _`
+      \\ `DISJOINT (domain g') gd` by metis_tac [co_disjoint_globals_first_n_exps]
+      \\ metis_tac [mglobals_extend_DISJOINT_state_globals_approx]))
+    \\ Cases_on `body_opt` \\ fs []
+    \\ fs [bool_case_eq]
+    \\ rpt (pairarg_tac \\ fs []) \\ rveq
+    \\ rename1 `known limit [_] _ g2 = (_, g)`
+    \\ fs [evaluate_def, pair_case_eq]
+    \\ imp_res_tac known_sing_EQ_E \\ fs [] \\ rveq
+    THEN1 (* pure *)
+     (imp_res_tac unique_set_globals_subexps
+      \\ `subspt g1 g2 /\ subspt g2 g`
+         by (match_mp_tac subspt_known_elist_globals
+             \\ rpt (goal_assum drule)
+             \\ fs [unique_set_globals_def, BAG_ALL_DISTINCT_BAG_UNION, BAG_DISJOINT_SYM])
+      \\ `subspt g2 g'` by metis_tac [subspt_trans]
+      \\ first_x_assum drule
+      \\ rpt (disch_then drule)
+      \\ strip_tac
+      \\ fs [result_case_eq] \\ rveq \\ fs []
+      \\ fs [case_eq_thms, pair_case_eq, bool_case_eq] \\ rveq
+      \\ fs [dest_Clos_def] \\ rveq
+      \\ imp_res_tac evaluate_mk_Ticks \\ fs []
+      \\ last_x_assum (pop_assum o mp_then Any match_mp_tac)
+      \\ simp [dec_clock_def]
+      \\ simp [EVERY2_APPEND_suff]
+      \\ rename1 `evaluate (MAP FST ea2, env, s1) = (Rval args, s2)`
+      \\ drule co_disjoint_globals_evaluate \\ disch_then drule
+      \\ simp [] \\ disch_then kall_tac
+      \\ patresolve  `known _ _ _ g1 = _` hd known_preserves_esgc_free
+      \\ simp [] \\ strip_tac
+      \\ patresolve  `known _ _ _ g2 = _` hd known_preserves_esgc_free
+      \\ simp [] \\ strip_tac
+      \\ imp_res_tac set_globals_empty_esgc_free \\ simp []
+      \\ simp [ALL_EL_MAP]
+      \\ patresolve `evaluate (_,_,s1) = _` hd evaluate_changed_globals
+      \\ simp [ALL_EL_MAP] \\ disch_then kall_tac
+      \\ rename1 `known _ [xbody] _ g = (_, gdead)`
+      \\ `unique_set_globals [xbody] s2.compile_oracle`
+         by (match_mp_tac unique_set_globals_evaluate
+             \\ goal_assum (first_assum o mp_then (Pos (el 2)) mp_tac)
+             \\ fs [unique_set_globals_def, BAG_ALL_DISTINCT_BAG_UNION])
+      \\ simp []
+      \\ `g = gdead`
+         by (match_mp_tac known_unchanged_globals
+             \\ goal_assum drule \\ simp [])
+      \\ fs [])
+    THEN1 (* not pure *)
+     (fs [evaluate_append, pair_case_eq]
+      \\ rename1 `evaluate (_, _, s1) = (res1, s2)`
+      \\ imp_res_tac unique_set_globals_subexps
+      \\ `subspt g1 g2 /\ subspt g2 g`
+         by (match_mp_tac subspt_known_elist_globals
+             \\ rpt (goal_assum drule)
+             \\ fs [unique_set_globals_def, BAG_ALL_DISTINCT_BAG_UNION, BAG_DISJOINT_SYM])
+      \\ `subspt g2 g'` by metis_tac [subspt_trans]
+      \\ first_x_assum drule
+      \\ rpt (disch_then drule)
+      \\ strip_tac
+      \\ Cases_on `res1`
+      \\ fs [] \\ rveq \\ fs [] \\ rveq \\ fs []
+      \\ rename1 `evaluate (_, _, s1) = (Rval args, _)`
+      \\ fs [pair_case_eq]
+      \\ rename1 `evaluate (_, _, s2) = (res2, s3)`
+      \\ patresolve  `known _ _ _ g1 = _` hd known_preserves_esgc_free
+      \\ simp [] \\ strip_tac
+      \\ patresolve `ssgc_free _` (el 2) evaluate_changed_globals
+      \\ rpt (disch_then drule \\ simp []) \\ strip_tac
+      \\ drule co_disjoint_globals_evaluate \\ disch_then drule \\ strip_tac
+      \\ `unique_set_globals [x] s2.compile_oracle`
+         by metis_tac [unique_set_globals_evaluate]
+      \\ first_x_assum drule
+      \\ rpt (disch_then drule)
+      \\ strip_tac
+      \\ Cases_on `res2`
+      \\ fs [] \\ rveq \\ fs [] \\ rveq \\ fs []
+      \\ patresolve  `known _ _ _ g2 = _` hd known_preserves_esgc_free
+      \\ simp [] \\ strip_tac
+      \\ patresolve `ssgc_free _` (el 2) evaluate_changed_globals
+      \\ rpt (disch_then drule \\ simp []) \\ strip_tac
+      \\ imp_res_tac evaluate_mk_Ticks \\ fs []
+      \\ last_x_assum (pop_assum o mp_then Any match_mp_tac)
+      \\ simp [dec_clock_def, SNOC_APPEND, EVERY2_APPEND_suff]
+      \\ simp [co_disjoint_globals_shift_seq]
+      \\ fs [case_eq_thms, pair_case_eq, bool_case_eq] \\ rveq
+      \\ fs [dest_Clos_def] \\ rveq \\ fs [] \\ rveq
+      \\ simp [set_globals_empty_esgc_free]
+      \\ rename1 `known _ [xbody] _ g = (_, gdead)`
+      \\ `unique_set_globals [xbody] s1.compile_oracle`
+         by fs [unique_set_globals_def, BAG_ALL_DISTINCT_BAG_UNION]
+      \\ simp [unique_set_globals_shift_seq]
+      \\ `g = gdead` by (match_mp_tac known_unchanged_globals \\ goal_assum drule \\ simp [])
+      \\ fs []))
+  THEN1
+   (say "Fn"
+    \\ rpt (pairarg_tac \\ fs []) \\ rveq
+    \\ fs [evaluate_def]
+    \\ fs [bool_case_eq] \\ rveq
+    \\ Cases_on `loc_opt` \\ simp []
+    \\ simp [clos_approx_def]
+    \\ IF_CASES_TAC \\ simp [])
+  THEN1
+   (say "Letrec"
+    \\ rpt (pairarg_tac \\ fs []) \\ rveq
+    \\ imp_res_tac known_sing_EQ_E \\ fs [] \\ rveq
+    \\ imp_res_tac unique_set_globals_subexps
+    \\ fs [evaluate_def, bool_case_eq, clos_gen_noinline_eq]
+    \\ fixeqs
+    \\ qmatch_assum_abbrev_tac `closSem$evaluate([_], GENLIST (_ (MAP ff _)) _ ++ _, _) = _`
+    \\ rename1 `closSem$evaluate ([body'],
+                                  GENLIST (Recclosure lopt [] env (MAP ff fns))
+                                  (LENGTH fns) ++ env,
+                                  s0) = (result, s)`
+    \\ first_x_assum (qpat_assum `evaluate ([_],_,_) = _` o mp_then Any match_mp_tac)
+    \\ simp []
+    \\ Cases_on `lopt` \\ fs []
+    THEN1
+     (fs [REPLICATE_GENLIST]
+      \\ conj_tac
+      THEN1 (irule EVERY2_APPEND_suff \\ simp []
+             \\ fs [LIST_REL_GENLIST])
+      \\ reverse conj_tac
+      THEN1 fs [EVERY_GENLIST]
+      \\ fs [EVERY_GENLIST]
+      \\ fs [elglobals_EQ_EMPTY, MEM_MAP, PULL_EXISTS, FORALL_PROD]
+      \\ simp [Abbr `ff`] \\ rpt strip_tac
+      \\ qmatch_abbrev_tac `set_globals (FST (HD (FST (known _ [_] ENV g1)))) = {||}`
+      \\ rename1 `MEM (num_args, fbody) fns`
+      \\ `set_globals fbody = {||}` by metis_tac[]
+      \\ Cases_on `known limit [fbody] ENV g1` \\ simp []
+      \\ imp_res_tac known_sing_EQ_E \\ fs [] \\ rveq
+      \\ patresolve `known _ [fbody] _ _ = _` (el 1) known_elglobals_dont_grow
+      \\ fs [set_globals_empty_esgc_free]
+      \\ simp [Abbr `ENV`, EVERY_GENLIST])
+    THEN1
+     (conj_tac
+      THEN1 (irule EVERY2_APPEND_suff \\ simp []
+             \\ fs [LIST_REL_GENLIST, EL_MAP]
+             \\ rpt strip_tac
+             \\ simp [Abbr `ff`]
+             \\ pairarg_tac \\ simp [])
+      \\ reverse conj_tac
+      THEN1 fs [EVERY_GENLIST]
+      \\ fs [EVERY_GENLIST]
+      \\ fs [elglobals_EQ_EMPTY]
+      \\ simp [MEM_MAP, PULL_EXISTS, FORALL_PROD]
+      \\ simp [Abbr `ff`] \\ rpt strip_tac
+      \\ qmatch_abbrev_tac `set_globals (FST (HD (FST (known _ [_] ENV g1)))) = {||}`
+      \\ rename1 `MEM (num_args, fbody) fns`
+      \\ `set_globals fbody = {||}`
+         by (fs [MEM_MAP, PULL_EXISTS, FORALL_PROD] \\ metis_tac [])
+      \\ Cases_on `known limit [fbody] ENV g1` \\ simp []
+      \\ imp_res_tac known_sing_EQ_E \\ fs [] \\ rveq
+      \\ patresolve `known _ [fbody] _ _ = _` (el 1) known_elglobals_dont_grow
+      \\ fs [set_globals_empty_esgc_free]
+      \\ disch_then match_mp_tac
+      \\ simp [Abbr `ENV`]
+      \\ simp [EVERY_REPLICATE, EVERY_GENLIST])));
+
+
+(* code relation *)
+
+val exp_rel_def = Define `
+  exp_rel limit aenv g' e1 e2 <=>
+    ?g0 g apx.
+      subspt g g' /\
+      EVERY val_approx_sgc_free aenv /\
+      globals_approx_sgc_free g0 /\
+      known limit [e1] aenv g0 = ([(e2, apx)], g)`;
+
+(* value relation *)
+
+val f_rel_def = Define `
+  f_rel limit aenv g (a1, e1) (a2, e2) <=>
+     a1 = a2 /\ exp_rel limit (REPLICATE a1 Other ++ aenv) g e1 e2`;
+
+val (v_rel_rules, v_rel_ind, v_rel_cases) = Hol_reln `
+  (!i. v_rel l g (Number i) (Number i)) /\
+  (!w. v_rel l g (Word64 w) (Word64 w)) /\
+  (!w. v_rel l g (ByteVector w) (ByteVector w)) /\
+  (!n. v_rel l g (RefPtr n) (RefPtr n)) /\
+  (!tag xs ys.
+     LIST_REL (v_rel l g) xs ys ==>
+       v_rel l g (Block tag xs) (Block tag ys)) /\
+  (!loc args1 args2 env1 env2 num_args e1 e2 aenv.
+     LIST_REL (v_rel l g) env1 env2 /\
+     LIST_REL (v_rel l g) args1 args2 /\
+     LIST_REL val_approx_val aenv env2 /\
+     exp_rel l (REPLICATE num_args Other ++ aenv) g e1 e2 ==>
+       v_rel l g (Closure loc args1 env1 num_args e1) (Closure loc args2 env2 num_args e2)) /\
+  (!loc_opt funs1 funs2 args1 args2 env1 env2 k aenv.
+     LIST_REL (v_rel l g) env1 env2 /\
+     LIST_REL (v_rel l g) args1 args2 /\
+     (clos = case loc_opt of
+               | NONE => REPLICATE (LENGTH funs1) Other
+               | SOME loc => clos_gen_noinline loc 0 funs1) /\
+     LIST_REL (f_rel l (clos ++ aenv) g) funs1 funs2 ==>
+       v_rel l g (Recclosure loc_opt args1 env1 funs1 k) (Recclosure loc_opt args2 env2 funs2 k))`;
+
+
+val v_rel_simps = save_thm("v_rel_simps[simp]",LIST_CONJ [
+  SIMP_CONV (srw_ss()) [v_rel_cases] ``v_rel l g (Number n) x``,
+  SIMP_CONV (srw_ss()) [v_rel_cases] ``v_rel l g (Block n p) x``,
+  SIMP_CONV (srw_ss()) [v_rel_cases] ``v_rel l g (Word64 p) x``,
+  SIMP_CONV (srw_ss()) [v_rel_cases] ``v_rel l g (ByteVector p) x``,
+  SIMP_CONV (srw_ss()) [v_rel_cases] ``v_rel l g (RefPtr p) x``,
+  SIMP_CONV (srw_ss()) [v_rel_cases] ``v_rel l g (Closure x1 x2 x3 x4 x5) x``,
+  SIMP_CONV (srw_ss()) [v_rel_cases] ``v_rel l g (Recclosure y1 y2 y3 y4 y5) x``,
+  prove(``v_rel l g (Boolv b) x <=> x = Boolv b``,
+        Cases_on `b` \\ fs [Boolv_def,Once v_rel_cases]),
+  prove(``v_rel l g Unit x <=> x = Unit``,
+        fs [closSemTheory.Unit_def,Once v_rel_cases])])
+
+val v_rel_vsgc_free = Q.store_thm(
+  "v_rel_vsgc_free",
+  `!l g v1 v2. v_rel l g v1 v2 ==> (vsgc_free v1 ==> vsgc_free v2)`,
+  cheat);
+
+(*
+
+  ntac 2 gen_tac \\ ho_match_mp_tac v_rel_ind \\ simp [] \\ rpt strip_tac
+  THEN1 (fs [EVERY_MEM, LIST_REL_EL_EQN] \\ metis_tac [MEM_EL])
+  THEN1 (
+         fs [EVERY_MEM, LIST_REL_EL_EQN] \\ fs [exp_rel_def]
+         \\ eq_tac \\ strip_tac
+         \\ drule known_elglobals_dont_grow
+         \\ fs [EVERY_REPLICATE, set_globals_empty_esgc_free]
+         \\ fs [MEM_EL, PULL_EXISTS]
+
+ \\ simp [set_globals_empty_esgc_free] >>
+         fs[] >> metis_tac[MEM_EL])
+  >- (fs[EVERY_MEM, LIST_REL_EL_EQN, elglobals_EQ_EMPTY, MEM_MAP, PULL_EXISTS,
+         FORALL_PROD]>>
+      EQ_TAC >> rpt strip_tac
+      >- (imp_res_tac (MEM_EL |> SPEC_ALL |> EQ_IMP_RULE |> #1 |> GSYM) >>
+          rename1 `m < LENGTH fns2` >>
+          Cases_on `EL m fns1` >> fs[] >>
+          first_x_assum (qspec_then `m` mp_tac) >> simp[] >>
+          rw[exp_rel_def] >>
+          imp_res_tac known_preserves_setGlobals >> fs[] >>
+          metis_tac[MEM_EL])
+      >- metis_tac[MEM_EL]
+      >- metis_tac[MEM_EL]
+      >- (imp_res_tac (MEM_EL |> SPEC_ALL |> EQ_IMP_RULE |> #1 |> GSYM) >>
+          rename1 `m < LENGTH fns1` >>
+          Cases_on `EL m fns2` >> fs[] >>
+          first_x_assum (qspec_then `m` mp_tac) >> simp[] >>
+          rw[exp_rel_def] >>
+          imp_res_tac known_preserves_setGlobals >> fs[] >>
+          metis_tac[MEM_EL])
+      >- metis_tac[MEM_EL]
+      >- metis_tac[MEM_EL]))
+*)
+
+val v_rel_Boolv = Q.store_thm(
+  "v_rel_Boolv[simp]",
+  `(v_rel l g (Boolv b) v ⇔ v = Boolv b) ∧
+   (v_rel l g v (Boolv b) ⇔ v = Boolv b)`,
+  simp [closSemTheory.Boolv_def] >> Cases_on `v` >> simp[] >> metis_tac[]);
+
+val v_rel_Unit = Q.store_thm(
+  "v_rel_Unit[simp]",
+  `(v_rel l g Unit v ⇔ v = Unit) ∧ (v_rel l g v Unit ⇔ v = Unit)`,
+  simp[Unit_def] >> Cases_on `v` >> simp[] >> metis_tac[])
+
+val v_rel_EVERY_vsgc_free = Q.store_thm(
+  "v_rel_EVERY_vsgc_free",
+  `!vs1 vs2.
+     LIST_REL (v_rel l g) vs1 vs2 ==>
+     (EVERY vsgc_free vs1 ==> EVERY vsgc_free vs2)`,
+  Induct_on `LIST_REL` >> simp[] >> metis_tac [v_rel_vsgc_free]);
+
+
+val v_rel_val_approx = Q.store_thm(
+  "v_rel_val_approx",
+  `!l g v1 v2.
+     v_rel l g v1 v2 ==> ∀a. val_approx_val a v1 <=> val_approx_val a v2`,
+
+
+(*
+
+This doesn't hold any longer.
+
+known_correct_approx
+
+val v_rel_val_approx = Q.store_thm(
+  "v_rel_val_approx",
+  `!l g v1 v2.
+     v_rel l g v1 v2 ==> ∀a. val_approx_val a v1 <=> val_approx_val a v2`,
+
+  ntac 2 gen_tac \\ ho_match_mp_tac v_rel_ind \\ rw []
+  THEN1 (Cases_on `a` \\ simp []
+         THEN1 (rename1 `Clos _ _ body_opt`
+                \\ Cases_on `body_opt` \\ simp [])                
+         THEN1 (fs [LIST_REL_EL_EQN] \\ metis_tac [MEM_EL]))
+
+  THEN1 (Cases_on `a` \\ simp []
+         \\ rename1 `Clos _ _ body_opt`
+         \\ Cases_on `body_opt` \\ simp []
+         THEN1 (fs [LIST_REL_EL_EQN] \\ metis_tac [LENGTH_NIL])
+         \\ fs [LIST_REL_EL_EQN]
+
+
+         )
+
+  THEN1 (Cases_on `a` \\ fs [LIST_REL_EL_EQN]
+         \\ rename1 `lopt = SOME _`
+         \\ Cases_on `lopt` \\ simp [] \\ rename1 `EL j`
+         \\ rename1 `j < LENGTH fns2` \\ Cases_on `j < LENGTH fns2` \\ simp []
+         \\ rename1 `vvs = []` \\ reverse (Cases_on `vvs`)
+         THEN1 (simp [] \\ rename1 `vvs' = []` \\ Cases_on `vvs'` \\ fs [])
+         \\ fs [] \\ rfs [] \\ res_tac
+         \\ Cases_on `EL j fns2` \\ rename1 `EL j fns1` \\ Cases_on `EL j fns1`
+         \\ fs [f_rel_def]))
+
+val v_rel_LIST_REL_val_approx = Q.store_thm(
+  "v_rel_LIST_REL_val_approx",
+  `!vs1 vs2 l g axs. LIST_REL (v_rel l g) vs1 vs2 ==>
+   (LIST_REL val_approx_val axs vs1 <=> LIST_REL val_approx_val axs vs2)`,
+   fs [LIST_REL_EL_EQN] \\ rpt strip_tac
+   \\ eq_tac \\ rpt strip_tac \\ fs []
+   \\ metis_tac [v_rel_val_approx])
+
+*)
+
+(* state relation *)
+
+val (ref_rel_rules, ref_rel_ind, ref_rel_cases) = Hol_reln `
+  (!b bs. ref_rel l g (ByteArray b bs) (ByteArray b bs)) /\
+  (!xs ys.
+    LIST_REL (v_rel l g) xs ys ==>
+    ref_rel l g (ValueArray xs) (ValueArray ys))`;
+
+val ref_rel_simps = save_thm("ref_rel_simps[simp]",LIST_CONJ [
+  SIMP_CONV (srw_ss()) [ref_rel_cases] ``ref_rel l g (ValueArray vs) x``,
+  SIMP_CONV (srw_ss()) [ref_rel_cases] ``ref_rel l g (ByteArray b bs) x``])
+
+val compile_inc_def = Define `
+  compile_inc l g (e,xs) =
+    let (ea, g') = known l [e] [] g in (g', FST (HD ea), xs)`;
+
+val state_rel_def = Define `
+  state_rel l g (s:(val_approx num_map#'c,'ffi) closSem$state) (t:('c,'ffi) closSem$state) <=>
+    (!n. SND (SND (s.compile_oracle n)) = []) /\
+    s.code = FEMPTY /\ t.code = FEMPTY /\
+    s.clock = t.clock /\ s.ffi = t.ffi /\ s.max_app = t.max_app /\
+    LIST_REL (OPTREL (v_rel l g)) s.globals t.globals /\
+    fmap_rel (ref_rel l g) s.refs t.refs /\
+    s.compile = state_cc (compile_inc l) t.compile  /\
+    t.compile_oracle = state_co (compile_inc l) s.compile_oracle`;
+
+
+(* No longer true
+val state_rel_state_globals_approx = Q.store_thm(
+  "state_rel_state_globals_approx",
+  `!l g0 s t g. state_rel l g0 s t ⇒ (state_globals_approx s g ⇔ state_globals_approx t g)`,
+  simp [state_rel_def, state_globals_approx_def, get_global_def, LIST_REL_EL_EQN] >>
+  csimp[] >> rpt strip_tac >> eq_tac >> rpt strip_tac >>
+  rename1 `EL kk (ss:('a,'b) closSem$state).globals = SOME vv` >>
+  rename1 `lookup kk gg` >>
+  nailIHx mp_tac >>
+  simp[optionTheory.OPTREL_def] >>
+    \\ strip_tac
+    \\ res_tac
+  metis_tac [v_rel_val_approx])
+*)
+
+val oracle_state_sgc_free_def = Define `
+  oracle_state_sgc_free co = !n. globals_approx_sgc_free (FST (FST (co n)))`;
+
+val oracle_state_sgc_free_shift_seq =
+  Q.store_thm("oracle_state_sgc_free_shift_seq",
+  `!co n. oracle_state_sgc_free co ==> oracle_state_sgc_free (shift_seq n co)`,
+  rpt strip_tac \\ fs [oracle_state_sgc_free_def, shift_seq_def])
+
+val state_rel_ssgc_free = Q.store_thm(
+  "state_rel_ssgc_free",
+  `!l g s1 s2. state_rel l g s1 s2 /\ oracle_state_sgc_free s1.compile_oracle  /\ ssgc_free s1 ==> ssgc_free s2`,
+  simp [state_rel_def, ssgc_free_def]
+  \\ rpt strip_tac
+  \\ fs [fmap_rel_OPTREL_FLOOKUP]
+  THEN1
+   (rename1 `FLOOKUP s2.refs kk = SOME (ValueArray vvl)`
+    \\ `OPTREL (ref_rel l g) (FLOOKUP s1.refs kk) (FLOOKUP s2.refs kk)` by simp[]
+    \\ pop_assum mp_tac
+    \\ simp_tac (srw_ss()) [OPTREL_def]
+    \\ simp [PULL_EXISTS]
+    \\ Cases \\ simp[]
+    \\ metis_tac [v_rel_EVERY_vsgc_free])
+  THEN1
+   (fs [LIST_REL_EL_EQN]
+    \\ imp_res_tac (MEM_EL |> SPEC_ALL |> EQ_IMP_RULE |> #1 |> GSYM)
+    \\ rename1 `EL kk s2.globals`
+    \\ `OPTREL (v_rel l g) (EL kk s1.globals) (EL kk s2.globals)` by simp[]
+    \\ pop_assum mp_tac \\ simp_tac(srw_ss()) [OPTREL_def] \\ simp[]
+    \\ metis_tac [v_rel_vsgc_free, MEM_EL])
+  THEN1
+   (fs [state_co_def]
+    \\ rpt (pairarg_tac \\ fs []) \\ rveq
+    \\ rename1 `s1.compile_oracle nn = _`
+    \\ Cases_on `SND (s1.compile_oracle nn)`
+    \\ res_tac
+    \\ rfs [] \\ rveq \\ fs []
+    \\ fs [compile_inc_def]
+    \\ pairarg_tac \\ fs [] \\ rveq
+    \\ imp_res_tac known_sing_EQ_E \\ rveq \\ fs []
+    \\ drule known_preserves_esgc_free \\ fs []
+    \\ fs [oracle_state_sgc_free_def]
+    \\ rename1 `known _ _ _ ss`
+    \\ `ss = FST (FST (s1.compile_oracle nn))` by simp []
+    \\ metis_tac [])
+  THEN1
+   (fs [state_co_def]
+    \\ rpt (pairarg_tac \\ fs []) \\ rveq
+    \\ rename1 `compile_inc _ _ progs`
+    \\ PairCases_on `progs` \\ fs [compile_inc_def]
+    \\ pairarg_tac \\ fs [] \\ rveq
+    \\ rename1 `s1.compile_oracle nn = _`
+    \\ qpat_x_assum `!n. _ = []` (qspec_then `nn` mp_tac)
+    \\ simp []))
+
+
+val loptrel_def = Define`
+  loptrel fv numargs lopt1 lopt2 ⇔
+     lopt2 = lopt1 ∨
+     lopt1 = NONE ∧
+     case (fv,lopt2) of
+       | (Closure (SOME loc1) ae _ n bod, SOME loc2) =>
+            loc1 = loc2 ∧ n = numargs ∧ ae = []
+       | (Recclosure (SOME loc1) ae _ fns i, SOME loc2) =>
+         i < LENGTH fns ∧ loc2 = loc1 + 2 * i ∧ numargs = FST (EL i fns) ∧
+         ae = []
+       | _ => F
+`;
+
+
+val evaluate_changed_globals_inst = INST_TYPE [``:'c`` |-> ``:val_approx num_map#'c``] evaluate_changed_globals
+val known_correct_approx_inst = INST_TYPE [``:'c`` |-> ``:val_approx num_map#'c``] known_correct_approx
+
+val co_every_Fn_vs_NONE_def = Define `
+  co_every_Fn_vs_NONE co =
+    !n exp aux. SND (co n) = (exp, aux) ==>
+      every_Fn_vs_NONE [exp] /\
+      every_Fn_vs_NONE (MAP (SND o SND) aux)`
+
+val co_every_Fn_vs_NONE_shift_seq =
+  Q.store_thm("co_every_Fn_vs_NONE_shift_seq",
+  `!co n. co_every_Fn_vs_NONE co ==> co_every_Fn_vs_NONE (shift_seq n co)`,
+  rpt strip_tac \\ fs [co_every_Fn_vs_NONE_def, shift_seq_def] \\ metis_tac [])
+
+val state_rel_co_set_globals = Q.store_thm("state_rel_co_set_globals",
+  `state_rel l g s t /\ ssgc_free s /\ oracle_state_sgc_free s.compile_oracle ==>
+     set_globals (FST (SND (t.compile_oracle n))) <= set_globals (FST (SND (s.compile_oracle n)))`,
+  strip_tac \\ fs [state_rel_def]
+  \\ fs [state_co_def]
+  \\ rpt (pairarg_tac \\ fs [])
+  \\ rename1 `compile_inc _ _ p1 = (_, p2)`
+  \\ PairCases_on `p1`
+  \\ fs [compile_inc_def]
+  \\ pairarg_tac \\ fs [] \\ rveq
+  \\ imp_res_tac known_sing_EQ_E \\ rveq \\ fs []
+  \\ drule known_elglobals_dont_grow \\ fs []
+  \\ impl_tac \\ simp []
+  \\ rename1 `s.compile_oracle nn = _`
+  \\ fs [oracle_state_sgc_free_def]
+  \\ qpat_x_assum `!n. globals_approx_sgc_free _` (qspec_then `nn` mp_tac) \\ simp []
+  \\ fs [ssgc_free_def]
+  \\ qpat_x_assum `!n e a. _` (qspec_then `nn` mp_tac) \\ simp []);
+
+val state_rel_first_n_exps = Q.store_thm("state_rel_first_n_exps",
+  `state_rel l g s t /\ ssgc_free s /\ oracle_state_sgc_free s.compile_oracle ==>
+     elist_globals (first_n_exps t.compile_oracle n) <= elist_globals (first_n_exps s.compile_oracle n)`,
+  strip_tac
+  \\ imp_res_tac state_rel_co_set_globals
+  \\ fs [first_n_exps_def] \\ Induct_on `n`
+  \\ fs [GENLIST]
+  \\ simp [SNOC_APPEND, elist_globals_append]
+  \\ simp [SUB_BAG_UNION]);
+
+val state_rel_unique_set_globals = Q.store_thm("state_rel_unique_set_globals",
+  `!xs. state_rel l g s t /\ ssgc_free s /\ oracle_state_sgc_free s.compile_oracle /\
+   unique_set_globals xs s.compile_oracle ==> unique_set_globals xs t.compile_oracle`,
+  rpt strip_tac
+  \\ imp_res_tac state_rel_first_n_exps
+  \\ fs [unique_set_globals_def]
+  \\ fs [elist_globals_append, BAG_ALL_DISTINCT_BAG_UNION]
+  \\ gen_tac
+  \\ rpt (qpat_x_assum `!n. _` (qspec_then `n` assume_tac))
+  \\ fs []
+  \\ imp_res_tac SUB_BAG_DIFF_EQ \\ pop_assum (fn th => fs [Once th])
+  \\ fs [BAG_ALL_DISTINCT_BAG_UNION])
+
+val state_rel_co_disjoint_globals = Q.store_thm("state_rel_co_disjoint_globals",
+  `!g : val_approx num_map. state_rel l g0 s t /\ ssgc_free s /\ oracle_state_sgc_free s.compile_oracle /\
+   co_disjoint_globals g s.compile_oracle ==> co_disjoint_globals g t.compile_oracle`,
+  rpt strip_tac
+  \\ imp_res_tac state_rel_co_set_globals
+  \\ fs [co_disjoint_globals_def]
+  \\ assume_tac (BAG_DISJOINT |> GSYM |> ISPEC ``BAG_OF_SET (domain (g : val_approx num_map))``)
+  \\ fs [] \\ pop_assum kall_tac
+  \\ gen_tac
+  \\ rpt (qpat_x_assum `!n. _` (qspec_then `n` assume_tac))
+  \\ imp_res_tac SUB_BAG_DIFF_EQ \\ pop_assum (fn th => fs [Once th]));
+
+val state_rel_get_global_IMP = Q.store_thm("state_rel_get_global_IMP",
+  `!l g s t n v1. state_rel l g s t /\ get_global n s.globals = SOME (SOME v1) ==>
+   ?v2. get_global n t.globals = SOME (SOME v2) /\ v_rel l g v1 v2`,
+  rw [state_rel_def, get_global_def, LIST_REL_EL_EQN]
+  \\ metis_tac [OPTREL_SOME]);
+
+val do_app_lemma = Q.prove(
+  `!l g s t xs ys opp. state_rel l g s t /\ LIST_REL (v_rel l g) xs ys ==>
+    case do_app opp xs s of
+      | Rerr err1 => ?err2. do_app opp ys t = Rerr err2 /\
+                            exc_rel (v_rel l g) err1 err2
+      | Rval (x, s1) => ?y t1. v_rel l g x y /\ state_rel l g s1 t1 /\
+                               do_app opp ys t = Rval (y, t1)`,
+  rpt gen_tac
+  \\ match_mp_tac simple_val_rel_do_app
+  \\ conj_tac THEN1 (fs [simple_val_rel_def] \\ rw [] \\ fs [v_rel_cases])
+  \\ fs [simple_state_rel_def, state_rel_def]
+  \\ rw [] \\ fs [fmap_rel_def, FLOOKUP_DEF]
+  \\ rfs []
+  \\ TRY (first_x_assum drule \\ fs [ref_rel_cases])
+  \\ fs [FAPPLY_FUPDATE_THM]
+  \\ rw [] \\ fs [ref_rel_cases]);
+
+(*
+val evaluate_app_lemma = Q.store_thm(
+  "evaluate_app_lemma",
+  `evaluate_app app_lopt
+     (Closure clos_lopt clos_args env arity body)
+     args s0 = (res, s) /\ res <> Rerr (Rabort Rtype_error) ==>
+     app_lopt = clos_lopt`,
+  Cases_on `args` \\ simp [evaluate_def]
+  \\ strip_tac
+
+val v_caseT = v_case_eq |> INST_TYPE [alpha |-> bool] |> Q.INST [`v` |-> `T`]
+                        |> REWRITE_RULE []
+val optcaset = ``option$option_CASE``
+val opt_caseT = case_eq_thms |> CONJUNCTS
+                    |> List.find (fn th => th |> concl |> lhs |> lhs
+                                              |> strip_comb
+                                              |> #1 |> same_const optcaset)
+                    |> valOf
+                    |> INST_TYPE [beta |-> bool]
+                    |> Q.INST [`v'` |-> `T`]
+                    |> SIMP_RULE (srw_ss()) []
+
+
+val loptrel_arg1_SOME = save_thm(
+  "loptrel_arg1_SOME",
+  loptrel_def |> SPEC_ALL |> Q.INST [`lopt1` |-> `SOME loc1`]
+              |> SIMP_RULE (srw_ss()) [opt_caseT, v_caseT])
+
+val loptrel_arg1_NONE = save_thm(
+  "loptrel_arg1_NONE",
+  loptrel_def |> SPEC_ALL |> Q.INST [`lopt1` |-> `NONE`]
+              |> SIMP_RULE (srw_ss()) [opt_caseT, v_caseT])
+*)
+
+val clos_arity_def = Define `
+  (clos_arity (Closure _ _ _ num_args _) = num_args) /\
+  (clos_arity (Recclosure _ _ _ fns k) = FST (EL k fns)) /\
+  (clos_arity _ = 0)`;
+
+
+val inline_lemma = Q.store_thm("inline_lemma",
+  `!loc arity body f env. val_approx_val (Clos loc arity (SOME body)) f /\
+   loptrel f arity lopt (SOME loc) /\
+   evaluate_app lopt f args s0 = (res, s1) /\
+   arity = LENGTH args /\
+   1 <= arity ==>
+   evaluate ([mk_Ticks tr trc arity body], args ++ env, s0) = (res, s1)`,
+
+   \\ rw []
+   \\ Cases_on `args` \\ fs [evaluate_def]
+   \\ fs [loptrel_def] \\ rveq
+   \\ fs [dest_closure_def, check_loc_def]
+   \\ simp [evaluate_mk_Ticks_EQ]
+
+   THEN1 (fs [bool_case_eq]
+          \\ fs [pair_case_eq, result_case_eq]
+          \\ imp_res_tac evaluate_SING \\ fs []
+          \\ rveq \\ fs []
+
+val say = say0 "known_correct0";
+
+val known_correct0 = Q.prove(
+  `(!xs env1 (s0:(val_approx num_map#'c,'ffi) closSem$state) res1 s env2 t0 limit g0 g g' aenv eas.
+      evaluate (xs, env1, s0) = (res1, s) /\
+      known limit xs aenv g0 = (eas, g) /\
+      LIST_REL (v_rel limit g') env1 env2 /\
+      state_rel limit g' s0 t0 /\
+      every_Fn_vs_NONE xs /\
+      co_every_Fn_vs_NONE s0.compile_oracle /\
+      EVERY esgc_free xs /\ ssgc_free s0 /\
+      EVERY vsgc_free env1 /\
+      subspt g0 g /\ subspt g g' /\
+      LIST_REL val_approx_val aenv env2 /\
+      oracle_state_sgc_free s0.compile_oracle /\
+      globals_approx_sgc_free g0 /\
+      state_globals_approx t0 g' /\
+      EVERY val_approx_sgc_free aenv /\
+      unique_set_globals xs s0.compile_oracle /\
+      co_disjoint_globals g' s0.compile_oracle /\
+      res1 <> Rerr (Rabort Rtype_error) ==>
+      ?res2 t.
+        evaluate (MAP FST eas, env2, t0) = (res2, t) /\
+        result_rel (LIST_REL (v_rel limit g')) (v_rel limit g') res1 res2 /\
+        state_rel limit g' s t) /\
+   (!lopt1 f1 args1 (s0:(val_approx num_map#'c,'ffi) closSem$state) res1 s lopt2 f2 args2 t0 limit g.
+      evaluate_app lopt1 f1 args1 s0 = (res1, s) /\
+      ssgc_free s0 /\
+      v_rel limit g f1 f2 /\ LIST_REL (v_rel limit g) args1 args2 /\
+      state_rel limit g s0 t0 /\ state_globals_approx s0 g /\
+      vsgc_free f1 /\ oracle_state_sgc_free s0.compile_oracle /\
+      loptrel f2 (LENGTH args1) lopt1 lopt2 ==>
+      ?res2 t.
+        evaluate_app lopt2 f2 args2 t0 = (res2, t) /\
+        result_rel (LIST_REL (v_rel limit g)) (v_rel limit g) res1 res2 /\
+        state_rel limit g s t)`,
+
+  ho_match_mp_tac (evaluate_ind |> Q.SPEC `\(x1,x2,x3). P0 x1 x2 x3`
+                   |> Q.GEN `P0` |> SIMP_RULE std_ss [FORALL_PROD])
+  \\ rpt strip_tac
+  THEN1
+   (say "NIL"
+    \\ fs [known_def, evaluate_def] \\ rveq
+    \\ goal_assum (first_assum o mp_then Any mp_tac)
+    \\ simp [])
+  THEN1
+   (say "CONS"
+    \\ fs [known_def, evaluate_def]
+    \\ rpt (pairarg_tac \\ fs []) \\ rveq
+    \\ imp_res_tac unique_set_globals_subexps \\ fs []
+    \\ fs [pair_case_eq]
+    \\ patresolve `subspt g0 g` (el 3) subspt_known_elist_globals
+    \\ rpt (disch_then drule)
+    \\ impl_tac THEN1 (imp_res_tac unique_set_globals_IMP_es_distinct_elist_globals
+                       \\ fs [BAG_ALL_DISTINCT_BAG_UNION])
+    \\ strip_tac
+    \\ rename1 `known _ [_] _ g0 = (_, g1)`
+    \\ `subspt g1 g'` by metis_tac [subspt_trans]
+    \\ first_x_assum drule
+    \\ rpt (disch_then drule \\ simp [])
+    \\ fs [result_case_eq] \\ rveq \\ fs []
+    \\ strip_tac \\ simp [evaluate_append]
+    \\ fs [pair_case_eq] \\ rveq \\ fs []
+    \\ first_x_assum drule
+    \\ rpt (disch_then drule \\ simp [])
+    \\ patresolve `evaluate ([_], _, _) = _` hd evaluate_changed_globals_inst
+    \\ simp [] \\ strip_tac \\ fs []
+    \\ fs [co_disjoint_globals_shift_seq,
+           unique_set_globals_shift_seq,
+           co_every_Fn_vs_NONE_shift_seq,
+           oracle_state_sgc_free_shift_seq]
+    \\ patresolve `known _ [_] _ _ = _` hd known_preserves_esgc_free
+    \\ simp [] \\ strip_tac
+    \\ patresolve `known _ [_] _ _ = _` hd known_correct_approx
+    \\ disch_then drule \\ simp []
+    \\ imp_res_tac known_sing_EQ_E \\ rveq \\ fs []
+    \\ rename1 `known _ [_] _ g0 = ([(e1,a1)],g1)`
+    \\ simp []
+    \\ patresolve `LIST_REL _ env1 env2` hd v_rel_EVERY_vsgc_free
+    \\ simp [] \\ strip_tac
+    \\ qpat_x_assum `state_rel _ _ s0 _` assume_tac
+    \\ drule state_rel_ssgc_free \\ simp []
+    \\ strip_tac \\ fs []
+    \\ disch_then (qpat_assum `state_globals_approx _ _` o mp_then Any mp_tac)
+    \\ simp []
+    \\ drule state_rel_unique_set_globals \\ simp []
+    \\ disch_then kall_tac
+    \\ drule state_rel_co_disjoint_globals \\ simp []
+    \\ disch_then kall_tac
+    \\ strip_tac \\ rveq \\ fs []
+    \\ qpat_x_assum `state_rel _ _ s1 _` assume_tac
+    \\ fs [result_case_eq] \\ rveq \\ fs []
+    \\ strip_tac \\ simp [])
+  THEN1
+   (say "Var"
+    \\ fs [known_def] \\ rveq \\ fs []
+    \\ fs [evaluate_def]
+    \\ imp_res_tac LIST_REL_LENGTH \\ fs []
+    \\ fs [bool_case_eq] \\ rveq
+    \\ metis_tac [LIST_REL_EL_EQN])
+
+  THEN1
+   (say "If"
+    \\ cheat)
+  THEN1
+   (say "Let"
+    \\ cheat)
+  THEN1
+   (say "Raise"
+    \\ fs [known_def] \\ rpt (pairarg_tac \\ fs []) \\ rveq
+    \\ fs [evaluate_def, pair_case_eq, result_case_eq]
+    \\ rveq \\ fs []
+    \\ imp_res_tac unique_set_globals_subexps
+    \\ first_x_assum drule
+    \\ rpt (disch_then drule \\ simp [])
+    \\ strip_tac
+    \\ imp_res_tac known_sing_EQ_E \\ rveq \\ fs [] \\ rveq
+    \\ fs [result_case_eq] \\ rveq \\ fs [] \\ rveq
+    \\ imp_res_tac evaluate_SING \\ rveq \\ fs [])
+  THEN1
+   (say "Handle"
+    \\ cheat)
+
+  THEN1
+   (say "Op"
+    \\ fs [known_def] \\ rpt (pairarg_tac \\ fs []) \\ rveq
+    \\ rename1 `known _ _ _ g0 = (_, g1)`
+    \\ imp_res_tac unique_set_globals_subexps
+    \\ drule subspt_known_op_elist_globals
+    \\ rpt (disch_then drule)
+    \\ impl_tac THEN1 (imp_res_tac unique_set_globals_IMP_es_distinct_elist_globals
+                       \\ fs [BAG_ALL_DISTINCT_BAG_UNION])
+    \\ strip_tac
+    \\ `subspt g1 g'` by metis_tac [subspt_trans]
+    \\ rename [`isGlobal opn`, `gO_destApx apx`]
+    \\ fs [evaluate_def, pair_case_eq]
+    \\ first_x_assum drule
+    \\ rpt (disch_then drule \\ simp [])
+    \\ reverse (fs [result_case_eq]) \\ rveq \\ fs []
+    THEN1 (strip_tac \\ rveq \\ fs []
+           \\ Cases_on `opn` \\ simp [isGlobal_def, evaluate_def]
+           \\ Cases_on `apx` \\ simp [gO_destApx_def] \\ rveq
+           \\ fs [known_op_def, NULL_EQ, bool_case_eq] \\ rveq
+           \\ fs [evaluate_def])
+    \\ strip_tac
+    \\ Cases_on `opn = Install` \\ fs []
+    THEN1 cheat
+    \\ Cases_on `isGlobal opn /\ gO_destApx apx <> gO_None`
+    THEN1
+     (fs []
+      \\ Cases_on `opn` \\ fs [isGlobal_def]
+      \\ Cases_on `apx` \\ fs[gO_destApx_def] \\ rveq
+      \\ fs [known_op_def, NULL_EQ, bool_case_eq] \\ rveq
+      \\ imp_res_tac known_LENGTH_EQ_E \\ fs [LENGTH_NIL_SYM] \\ rveq
+      \\ fs [evaluate_def, do_app_def] \\ rveq \\ fs []
+      \\ fs [case_eq_thms, pair_case_eq] \\ rveq \\ fs [] \\ rveq
+      \\ rename1 `lookup nn gg`
+      \\ Cases_on `lookup nn gg` \\ fs [] \\ rveq
+      \\ fs [state_globals_approx_def, subspt_def]
+      \\ qmatch_asmsub_abbrev_tac `lookup nn gg = SOME apx`
+      \\ `lookup nn g' = SOME apx` by metis_tac [domain_lookup]
+      \\ drule state_rel_get_global_IMP
+      \\ disch_then drule \\ strip_tac
+      \\ res_tac
+      \\ unabbrev_all_tac
+      \\ fs [val_approx_val_def])
+    THEN1
+     (rename1 `Op tr opn (MAP FST ea1)`
+      \\ qmatch_goalsub_abbrev_tac `evaluate ([opexp],_,_)`
+      \\ `opexp = Op tr opn (MAP FST ea1)`
+         by (Cases_on `isGlobal opn` \\ fs [] \\ rfs [])
+      \\ pop_assum SUBST_ALL_TAC
+      \\ qpat_x_assum `~(_ /\  _)` kall_tac
+      \\ simp [evaluate_def]
+      \\ qmatch_asmsub_abbrev_tac `do_app _ vvs _`
+      \\ qmatch_goalsub_abbrev_tac `do_app _ wws _`
+      \\ drule do_app_lemma
+      \\ disch_then (qspecl_then [`vvs`, `wws`, `opn`] mp_tac)
+      \\ impl_tac THEN1 metis_tac [EVERY2_REVERSE]
+      \\ fs [case_eq_thms, pair_case_eq]
+      \\ rveq \\ fs []
+      \\ strip_tac \\ fs []))
+  THEN1
+   (say "Fn"
+    \\ fs [known_def] \\ rpt (pairarg_tac \\ fs []) \\ rveq
+    \\ fs [evaluate_def, bool_case_eq] \\ rveq
+    \\ dsimp []
+    \\ qexists_tac `aenv`
+    \\ goal_assum (qpat_assum `LIST_REL val_approx_val _ _` o mp_then Any mp_tac)
+    \\ conj_tac
+    THEN1 fs [state_rel_def]
+    THEN1 (simp [exp_rel_def, EVERY_REPLICATE]
+           \\ imp_res_tac known_sing_EQ_E \\ rveq \\ fs [] \\ rveq
+           \\ rpt (goal_assum drule)))
+  THEN1
+   (say "Letrec"
+    \\ cheat)
+
+
+  THEN1
+   (say "App"
+    \\ fs [known_def] \\ rpt (pairarg_tac \\ fs []) \\ rveq
+    \\ imp_res_tac unique_set_globals_subexps
+    \\ imp_res_tac known_LENGTH_EQ_E
+    \\ rename1 `known _ _ _ g0 = (_, g1)`
+    \\ rename1 `known _ _ _ g1 = (_, g2)`
+    \\ `g2 = g` by (fs [bool_case_eq, case_eq_thms]
+                    \\ rpt (pairarg_tac \\ fs []))
+    \\ rveq
+    \\ patresolve `subspt g0 g` (el 3) subspt_known_elist_globals
+    \\ rpt (disch_then drule)
+    \\ impl_tac THEN1 (imp_res_tac unique_set_globals_IMP_es_distinct_elist_globals
+                       \\ fs [BAG_ALL_DISTINCT_BAG_UNION, BAG_DISJOINT_SYM])
+    \\ strip_tac
+    \\ `subspt g1 g'` by metis_tac [subspt_trans]
+    (* Cases split on annotate or inline *)
+    \\ Cases_on `SND limit = 0 \/ body_opt = NONE`
+    THEN1
+     (`eas = [(App v9 new_loc_opt e1 (MAP FST ea2),Other)]` by (fs [] \\ fs [])
+      \\ qpat_x_assum `_ \/ _` kall_tac
+      \\ qpat_x_assum `(if SND limit = 0 then _ else _) = _` kall_tac
+      \\ rveq
+      \\ fs [evaluate_def, bool_case_eq, pair_case_eq]
+      \\ first_x_assum drule
+      \\ rpt (disch_then drule \\ simp [])
+      \\ fs [result_case_eq] \\ rveq \\ fs []
+      \\ strip_tac \\ fs [] \\ rveq
+      \\ fs [pair_case_eq]
+      \\ first_x_assum drule
+      \\ rpt (disch_then drule \\ simp [])
+      \\ patresolve `evaluate (_, _, s0) = _` hd evaluate_changed_globals_inst
+      \\ simp [] \\ strip_tac \\ fs []
+      \\ fs [co_disjoint_globals_shift_seq,
+             unique_set_globals_shift_seq,
+             co_every_Fn_vs_NONE_shift_seq,
+             oracle_state_sgc_free_shift_seq]
+      \\ patresolve `known _ _ _ g0 = _` hd known_preserves_esgc_free
+      \\ simp [] \\ strip_tac
+      \\ patresolve `known _ _ _ g0 = _` hd known_correct_approx
+      \\ disch_then drule \\ simp []
+      \\ imp_res_tac known_sing_EQ_E \\ fs [] \\ rveq
+      \\ patresolve `LIST_REL _ env1 env2` hd v_rel_EVERY_vsgc_free
+      \\ simp [] \\ strip_tac
+      \\ patresolve `LIST_REL _ env1 env2` hd v_rel_LIST_REL_val_approx
+      \\ strip_tac \\ fs []
+      \\ qpat_x_assum `state_rel _ _ s0 _` assume_tac
+      \\ drule state_rel_ssgc_free \\ simp []
+      \\ strip_tac
+      \\ drule state_rel_state_globals_approx
+      \\ strip_tac \\ fs []
+      \\ disch_then (qpat_assum `state_globals_approx _ _` o mp_then Any mp_tac)
+      \\ simp []
+      \\ drule state_rel_unique_set_globals \\ simp []
+      \\ disch_then kall_tac
+      \\ drule state_rel_co_disjoint_globals \\ simp []
+      \\ disch_then kall_tac
+      \\ strip_tac \\ rveq \\ fs []
+      \\ qpat_x_assum `state_rel _ _ s1 _` assume_tac
+      \\ drule state_rel_state_globals_approx \\ strip_tac \\ fs []
+      \\ fs [result_case_eq] \\ fs [] \\ rveq
+      \\ strip_tac \\ rveq \\ fs []
+      \\ imp_res_tac evaluate_SING
+      \\ rveq \\ fs []
+      \\ patresolve `evaluate (_, _, s1) = _` hd evaluate_changed_globals_inst
+      \\ simp [] \\ strip_tac \\ fs []
+      \\ first_x_assum match_mp_tac \\ fs []
+      \\ `oracle_state_sgc_free s2.compile_oracle` by fs [oracle_state_sgc_free_shift_seq]
+      \\ rfs []
+      \\ patresolve `known _ _ _ g1 = _` hd known_correct_approx
+      \\ simp []
+      \\ disch_then drule \\ simp []
+      \\ disch_then (qspec_then `g'` mp_tac) \\ simp []
+      \\ qpat_x_assum `state_rel _ _ s1 _` assume_tac
+      \\ drule state_rel_ssgc_free
+      \\ simp [oracle_state_sgc_free_shift_seq]
+      \\ strip_tac
+      \\ `oracle_state_sgc_free s1.compile_oracle` by fs [oracle_state_sgc_free_shift_seq]
+      \\ `unique_set_globals [x1] s1.compile_oracle` by fs [unique_set_globals_shift_seq]
+      \\ `co_disjoint_globals g' s1.compile_oracle` by fs [co_disjoint_globals_shift_seq]
+      \\ rfs []
+      \\ drule state_rel_unique_set_globals \\ simp []
+      \\ disch_then kall_tac
+      \\ drule state_rel_co_disjoint_globals \\ simp []
+      \\ disch_then kall_tac
+      \\ strip_tac
+      \\ qpat_x_assum `state_rel _ _ s2 _` assume_tac
+      \\ drule state_rel_state_globals_approx
+      \\ strip_tac \\ simp []
+      \\ rename1 `dest_Clos fapx`
+      \\ Cases_on `dest_Clos fapx` \\ fs []
+      THEN1 fs [loptrel_def] \\ rveq \\ fs []
+      \\ Cases_on `lopt1` \\ fs []
+      THEN1 (simp [loptrel_def]
+             \\ rename1 `dest_Clos fapx = SOME clos_apx`
+             \\ `?clos_loc clos_arity clos_body. clos_apx = (clos_loc, clos_arity, clos_body)`
+                by (Cases_on `fapx` \\ fs [] \\ metis_tac [])
+             \\ fs [bool_case_eq] \\ metis_tac [evaluate_IMP_LENGTH])
+      \\ simp [loptrel_def]
+      \\ fs [pair_case_eq, bool_case_eq])
+    
+    (* Inlining *)
+    \\ fs []
+    \\ `?body. body_opt = SOME body` by (Cases_on `body_opt` \\ fs [])
+    \\ rveq \\ fs []
+    \\ fs [evaluate_def]
+    \\ Cases_on `LENGTH xs > 0` \\ fs []
+    \\ fs [pair_case_eq]
+    \\ Cases_on `dest_Clos a1` \\ fs []
+
+    \\ reverse (Cases_on `pure x1`) \\ fs []
+    \\ rpt (pairarg_tac \\ fs []) \\ rveq
+    \\ simp [evaluate_def]
+
+
+    THEN1
+
+      \\ simp [evaluate_append]
+
+      \\ first_x_assum drule
+      \\ rpt (disch_then drule \\ simp [])
+      \\ fs [result_case_eq] \\ rveq \\ fs []
+      \\ strip_tac \\ fs [] \\ rveq
+      \\ fs [pair_case_eq] \\ rveq
+
+
+      \\ simp [PULL_EXISTS]
+
+
+      \\ simp [evaluate_mk_Ticks_EQ]
+
+
+      \\ imp_res_tac known_sing_EQ_E \\ fs [] \\ rveq
+
+
+      \\ first_x_assum drule
+      \\ rpt (disch_then drule \\ simp [])
+
+      \\ patresolve `evaluate (_, _, s0) = _` hd evaluate_changed_globals_inst
+      \\ simp [] \\ strip_tac \\ fs []
+      \\ fs [co_disjoint_globals_shift_seq,
+             unique_set_globals_shift_seq,
+             co_every_Fn_vs_NONE_shift_seq,
+             oracle_state_sgc_free_shift_seq]
+      \\ patresolve `known _ _ _ g0 = _` hd known_preserves_esgc_free
+      \\ simp [] \\ strip_tac
+      \\ patresolve `known _ _ _ g0 = _` hd known_correct_approx
+      \\ disch_then drule \\ simp []
+      \\ imp_res_tac known_sing_EQ_E \\ fs [] \\ rveq
+      \\ patresolve `LIST_REL _ env1 env2` hd v_rel_EVERY_vsgc_free
+      \\ simp [] \\ strip_tac
+      \\ patresolve `LIST_REL _ env1 env2` hd v_rel_LIST_REL_val_approx
+      \\ strip_tac \\ fs []
+      \\ qpat_x_assum `state_rel _ _ s0 _` assume_tac
+      \\ drule state_rel_ssgc_free \\ simp []
+      \\ strip_tac
+      \\ drule state_rel_state_globals_approx
+      \\ strip_tac \\ fs []
+      \\ disch_then (qpat_assum `state_globals_approx _ _` o mp_then Any mp_tac)
+      \\ simp []
+      \\ drule state_rel_unique_set_globals \\ simp []
+      \\ disch_then kall_tac
+      \\ drule state_rel_co_disjoint_globals \\ simp []
+      \\ disch_then kall_tac
+      \\ strip_tac \\ rveq \\ fs []
+
+      \\ qpat_x_assum `state_rel _ _ s1 _` assume_tac
+      \\ drule state_rel_state_globals_approx \\ strip_tac \\ fs []
+      \\ fs [result_case_eq] \\ fs [] \\ rveq
+      \\ strip_tac \\ rveq \\ fs []
+      \\ imp_res_tac evaluate_SING
+      \\ rveq \\ fs []
+
+
+      \\ patresolve `known _ _ _ g1 = _` hd known_preserves_esgc_free
+      \\ simp [] \\ strip_tac
+
+      \\ patresolve `known _ _ _ g1 = _` hd known_correct_approx
+      \\ simp []
+      \\ disch_then drule \\ simp []
+      \\ disch_then (qspec_then `g'` mp_tac) \\ simp []
+
+
+      \\ qpat_x_assum `state_rel _ _ s1 _` assume_tac
+      \\ drule state_rel_ssgc_free \\ simp []
+      \\ simp [oracle_state_sgc_free_shift_seq]
+      \\ strip_tac
+      \\ `oracle_state_sgc_free s1.compile_oracle` by simp [oracle_state_sgc_free_shift_seq]
+      \\ `unique_set_globals [x1] s1.compile_oracle` by simp [unique_set_globals_shift_seq]
+      \\ `co_disjoint_globals g' s1.compile_oracle` by simp [co_disjoint_globals_shift_seq]
+      \\ rfs []
+      \\ drule state_rel_unique_set_globals \\ simp []
+      \\ disch_then kall_tac
+      \\ drule state_rel_co_disjoint_globals \\ simp []
+      \\ disch_then kall_tac
+      \\ strip_tac
+
+
+      \\ patresolve `evaluate (_, _, s1) = _` hd evaluate_changed_globals_inst
+      \\ simp [] \\ strip_tac
+
+
+      \\ first_x_assum drule
+      \\ rpt (disch_then drule \\ simp [])
+
+
+
+      \\ Cases_on `a1` \\ fs [] \\ rveq \\ fs []
+
+
+
+      \\ known_preserves_ssgc_free
+      \\ imp_res_tac unique_set_globals_shift_seq
+
+(*
+      \\ patresolve `evaluate (_, _, s1) = _` hd evaluate_changed_globals_inst
+      \\ simp [] \\ strip_tac
+*)
+
+)
+  THEN1
+   (say "Tick"
+    \\ fs [known_def] \\ rpt (pairarg_tac \\ fs []) \\ rveq
+    \\ fs [evaluate_def, pair_case_eq]
+    \\ `t0.clock = s0.clock` by fs [state_rel_def]
+    \\ fs [bool_case_eq] \\ fixeqs
+    \\ first_x_assum drule
+    \\ rpt (disch_then drule \\ simp [])
+    \\ disch_then (qspec_then `dec_clock 1 t0` mp_tac)
+    \\ fs [dec_clock_def]
+    \\ impl_tac THEN1 fs [state_rel_def]
+    \\ imp_res_tac unique_set_globals_subexps \\ simp []
+    \\ strip_tac
+    \\ imp_res_tac known_sing_EQ_E
+    \\ rveq \\ fs [] \\ rveq \\ fs [])
+  THEN1
+   (say "Call"
+    \\ fs [known_def] \\ rpt (pairarg_tac \\ fs []) \\ rveq
+    \\ fs [evaluate_def, pair_case_eq]
+    \\ imp_res_tac unique_set_globals_subexps
+    \\ first_x_assum drule
+    \\ rpt (disch_then drule \\ simp [])
+    \\ strip_tac \\ fs []
+    \\ rename1 `state_rel _ _ sss t`
+    \\ `sss.code = FEMPTY /\ t.code = FEMPTY` by fs [state_rel_def]
+    \\ fs [find_code_def]
+    \\ fs [result_case_eq]
+    \\ rveq \\ fs [])
+  THEN1
+   (say "evaluate_app NIL"
+    \\ fs [evaluate_def] \\ rveq \\ fs [])
+  THEN1
+   (say "evaluate_app CONS"
+    \\ cheat)
+
+
+
+
+(*
+  `(∀a es env1 env2 (s01:('a,'b) closSem$state) s02 res1 s1 g0 g g' as ealist.
+
+
+
+
+       ⇒
+      ∃res2 s2.
+        evaluate(MAP FST ealist, env2, s02) = (res2, s2) ∧
+        krrel g' (res1,s1) (res2,s2)) ∧
+   (∀lopt1 f1 args1 (s01:('a,'b) closSem$state) res1 s1 lopt2 f2 args2 s02 g.
+      evaluate_app lopt1 f1 args1 s01 = (res1,s1) ∧ ssgc_free s01 ∧
+      kvrel g f1 f2 ∧ LIST_REL (kvrel g) args1 args2 ∧
+      ksrel g s01 s02 ∧ state_globals_approx s01 g ∧ vsgc_free f1 ∧
+      EVERY vsgc_free args1 ∧ loptrel f2 (LENGTH args1) lopt1 lopt2 ⇒
+      ∃res2 s2.
+        evaluate_app lopt2 f2 args2 s02 = (res2,s2) ∧
+        krrel g (res1,s1) (res2,s2))`,
+  ho_match_mp_tac evaluate_ind >> rpt conj_tac
+  >- (say "nil" >> simp[evaluate_def, known_def])
+  >- (say "cons" >>
+      simp[evaluate_def, known_def, pair_case_eq, result_case_eq,
+           BAG_ALL_DISTINCT_BAG_UNION] >>
+      rpt strip_tac >> rveq >> rpt (pairarg_tac >> fs[]) >> rveq >> simp[] >>
+      first_x_assum (patresolve `known [_] _ _ = _` last) >>
+      disch_then (resolve_selected (el 4)) >> simp[] >>
+      patresolve `known [_] _ _ = _` hd subspt_known_elist_globals >> simp[] >>
+      disch_then (resolve_selected hd) >> simp[] >> strip_tac >>
+      disch_then (resolve_selected last) >> simp[] >>
+      (impl_keep_tac >- metis_tac[subspt_trans]) >>
+      rw[]
+      >- (imp_res_tac known_sing_EQ_E >> rveq >> fs[] >>
+          sel_ihpc last >> simp[] >> disch_then (resolve_selected (el 3)) >>
+          simp[] >> disch_then (resolve_selected hd) >> simp[] >> impl_tac
+          >- (conj_tac
+              >- (resolve_selected hd (GEN_ALL kca_sing_sga) >> simp[] >>
+                  disch_then (resolve_selected last) >> simp[] >>
+                  metis_tac[kvrel_LIST_REL_val_approx, kvrel_EVERY_vsgc_free,
+                            ksrel_sga, ksrel_ssgc_free]) >>
+              metis_tac[ssgc_free_preserved_SING']) >> rw[] >>
+          simp[Once evaluate_CONS] >> imp_res_tac evaluate_SING >> rveq >>
+          fs[])
+      >- (imp_res_tac known_sing_EQ_E >> rveq >> fs[] >> sel_ihpc last >>
+          simp[] >> disch_then (resolve_selected (el 3)) >> simp[] >>
+          disch_then (resolve_selected hd) >> simp[] >> impl_tac
+          >- (conj_tac
+              >- (resolve_selected hd (GEN_ALL kca_sing_sga) >> simp[] >>
+                  disch_then (resolve_selected last) >> simp[] >>
+                  metis_tac[kvrel_LIST_REL_val_approx, kvrel_EVERY_vsgc_free,
+                            ksrel_sga, ksrel_ssgc_free]) >>
+              metis_tac[ssgc_free_preserved_SING']) >> rw[] >>
+          simp[Once evaluate_CONS, result_case_eq] >> fs[krrel_err_rw] >>
+          dsimp[] >> metis_tac[result_CASES])
+      >- (imp_res_tac known_sing_EQ_E >> rveq >> fs[] >>
+          simp[Once evaluate_CONS, result_case_eq, pair_case_eq] >>
+          dsimp[] >> fs[krrel_err_rw] >> metis_tac[pair_CASES, result_CASES]))
+  >- (say "var" >>
+      simp[evaluate_def, bool_case_eq, known_def] >>
+      rpt strip_tac >> fs[LIST_REL_EL_EQN])
+  >- (say "if" >>
+      simp[evaluate_def, pair_case_eq, bool_case_eq, BAG_ALL_DISTINCT_BAG_UNION,
+           result_case_eq, known_def] >> rpt strip_tac >> rveq >> fs[] >>
+      rpt (pairarg_tac >> fs[]) >> rveq >> fs[] >> fixeqs >>
+      imp_res_tac known_sing_EQ_E >> rveq >> fs[] >> rveq >>
+      map_every rename1 [`ksrel g' s01 s02`, `subspt g g'`,
+                           `known [eb] as g2 = ([(eb',eapx)], g)`,
+                           `known [tb] as g1 = ([(tb',tapx)], g2)`,
+                           `known [gd] as g0 = ([(gd',gapx)], g1)`] >>
+      `known [gd;tb] as g0 = ([(gd',gapx); (tb',tapx)], g2)`
+        by simp[known_def] >>
+      resolve_selected hd (subspt_known_elist_globals)>> simp[] >>
+      disch_then (resolve_selected hd) >> simp[] >> strip_tac >>
+      patresolve `known [gd] _ _ = _` hd subspt_known_elist_globals >> simp[] >>
+      disch_then (resolve_selected hd) >> simp[] >> strip_tac
+      >- (first_x_assum (patresolve `state_globals_approx _ _` (el 6)) >>
+          rpt (disch_then (resolve_selected last) >> simp[]) >>
+          impl_keep_tac >- metis_tac[subspt_trans] >> rw[] >>
+          simp[evaluate_def] >> imp_res_tac evaluate_SING >> fs[] >> rveq >>
+          fs[] >> rveq >> sel_ihpc last >> simp[] >> disch_then irule >>
+          simp[]
+          >- metis_tac[ssgc_free_preserved_SING']
+          >- (patresolve `known [gd] _ _ = _` hd (GEN_ALL kca_sing_sga) >>
+              simp[] >> disch_then (resolve_selected last) >> simp[] >>
+              metis_tac[ksrel_sga, kvrel_LIST_REL_val_approx,
+                        kvrel_EVERY_vsgc_free, ksrel_ssgc_free])
+          >- metis_tac[subspt_trans])
+      >- (first_x_assum (patresolve `state_globals_approx _ _` (el 6)) >>
+          rpt (disch_then (resolve_selected last) >> simp[]) >>
+          impl_keep_tac >- metis_tac[subspt_trans] >> rw[] >>
+          simp[evaluate_def] >> imp_res_tac evaluate_SING >> fs[] >> rveq >>
+          fs[] >> rveq >> sel_ihpc last >> simp[] >> disch_then irule >>
+          simp[]
+          >- metis_tac[ssgc_free_preserved_SING']
+          >- (patresolve `known [gd] _ _ = _` hd (GEN_ALL kca_sing_sga) >>
+              simp[] >> disch_then (resolve_selected last) >> simp[] >>
+              metis_tac[ksrel_sga, kvrel_LIST_REL_val_approx,
+                        kvrel_EVERY_vsgc_free, ksrel_ssgc_free,
+                        state_approx_better_definedg, known_better_definedg]))
+      >- ((* guard doesn't evaluate to T or F *) sel_ihpc (el 6) >> simp[] >>
+          rpt (disch_then (resolve_selected last) >> simp[]) >>
+          impl_keep_tac >- metis_tac[subspt_trans] >> rw[] >>
+          simp[evaluate_def] >> imp_res_tac evaluate_SING >> fs[] >> rveq >>
+          fs[] >> rveq >> dsimp[bool_case_eq] >> rpt disj2_tac >>
+          rpt strip_tac >> rveq >> fs[])
+      >- ((* guard errors *) sel_ihpc (el 6) >> simp[] >>
+          rpt (disch_then (resolve_selected last) >> simp[]) >>
+          impl_keep_tac >- metis_tac[subspt_trans] >> rw[] >>
+          dsimp[evaluate_def, result_case_eq, bool_case_eq] >>
+          fs[krrel_err_rw] >> metis_tac[pair_CASES, result_CASES]))
+  >- (say "let" >>
+      simp[evaluate_def, pair_case_eq, result_case_eq] >>
+      rpt strip_tac >> rveq >> fs[known_def] >>
+      rpt (pairarg_tac >> fs[]) >> rveq >> fs[BAG_ALL_DISTINCT_BAG_UNION] >>
+      map_every rename1 [`known [bod] _ g1 = (_, g)`,
+                           `known _ _ g0 = (_, g1)`,
+                           `subspt g gg`] >>
+      patresolve `known _ _ g0 = _` hd subspt_known_elist_globals >> simp[] >>
+      disch_then (resolve_selected hd) >> simp[] >>
+      (impl_tac >- fs[BAG_DISJOINT, DISJOINT_SYM]) >> strip_tac >>
+      first_x_assum (patresolve `known _ _ g0 = _` last) >> simp[] >>
+      rpt (disch_then (resolve_selected last) >> simp[]) >>
+      (impl_keep_tac >- metis_tac[subspt_trans]) >> rw[] >>
+      simp[evaluate_def, result_case_eq]
+      >- (imp_res_tac known_sing_EQ_E >> rveq >> fs[] >>
+          rveq >> sel_ihpc last >> simp[] >> disch_then irule >> simp[]
+          >- metis_tac[ssgc_evaluate]
+          >- metis_tac[ssgc_evaluate,rsgc_free_def]
+          >- (resolve_selected last known_correct_approx >> simp[] >>
+              rpt (disch_then (resolve_selected hd) >> simp[]) >>
+              metis_tac[ksrel_sga, kvrel_EVERY_vsgc_free,
+                        kvrel_LIST_REL_val_approx, ksrel_ssgc_free])
+          >- simp[EVERY2_APPEND_suff]
+          >- (irule EVERY2_APPEND_suff >> simp[] >>
+              resolve_selected last known_correct_approx >> simp[] >>
+              rpt (disch_then (resolve_selected hd) >> simp[]) >>
+              metis_tac[ksrel_sga, kvrel_EVERY_vsgc_free,
+                        kvrel_LIST_REL_val_approx, ksrel_ssgc_free]))
+      >- (fs[krrel_err_rw, result_case_eq] >> dsimp[] >>
+          metis_tac[pair_CASES, result_CASES]))
+  >- (say "raise" >>
+      simp[evaluate_def, pair_case_eq, result_case_eq] >>
+      rpt strip_tac >> rveq >> fs[known_def] >> pairarg_tac >> fs[] >>
+      imp_res_tac known_sing_EQ_E >> fs[] >> rveq >> fs[] >>
+      simp[evaluate_def, pair_case_eq, result_case_eq] >>
+      nailIHx strip_assume_tac >> simp[] >> fs[]
+      >- (imp_res_tac evaluate_SING >> fs[])
+      >- (dsimp[] >> fs[krrel_err_rw] >> metis_tac[result_CASES]))
+  >- (say "handle" >>
+      simp[evaluate_def, pair_case_eq, result_case_eq,
+           BAG_ALL_DISTINCT_BAG_UNION, error_case_eq, known_def] >>
+      rpt strip_tac >> rveq >> fs[] >>
+      rpt (pairarg_tac >> fs[]) >> rveq >>
+      imp_res_tac known_sing_EQ_E >> rveq >> fs[] >> rveq >>
+      map_every rename1 [`known _ (_ :: _) g1 = (_, g)`,
+                           `known _ _ g0 = (_, g1)`,
+                           `subspt g gg`] >>
+      patresolve `known _ _ g0 = _` hd subspt_known_elist_globals >> simp[] >>
+      rpt (disch_then (resolve_selected hd) >> simp[]) >> strip_tac >>
+      first_x_assum (patresolve `state_globals_approx _ _`  (el 6)) >> simp[] >>
+      rpt (disch_then (resolve_selected last) >> simp[]) >>
+      (impl_keep_tac >- metis_tac[subspt_trans]) >> rw[] >>
+      simp[evaluate_def, pair_case_eq, result_case_eq, error_case_eq]
+      >- (dsimp[] >> fs[PULL_EXISTS] >> sel_ihpc last >> simp[] >>
+          fs[krrel_err_rw] >> disch_then irule >> simp[]
+          >- metis_tac[ssgc_free_preserved_SING']
+          >- first_assum
+               (mp_then (Pos last) (mp_tac >~ (simp[] >> NO_TAC)) ssgc_evaluate)
+          >- (patresolve `known _ _ g0 = _` hd (GEN_ALL kca_sing_sga) >>
+              simp[] >> disch_then (resolve_selected last) >> simp[] >>
+              metis_tac[ksrel_ssgc_free,kvrel_EVERY_vsgc_free,ksrel_sga,
+                        kvrel_LIST_REL_val_approx]))
+      >- (fs[krrel_err_rw, result_case_eq, error_case_eq] >> dsimp[] >>
+          metis_tac[pair_CASES, result_CASES, error_CASES]))
+  >- (say "op" >>
+      simp[evaluate_def, pair_case_eq, result_case_eq, known_def,
+           BAG_ALL_DISTINCT_BAG_UNION] >>
+      rpt gen_tac >> strip_tac >> rpt gen_tac >>
+      Cases_on `op = Install` >- cheat >>
+      rpt (pairarg_tac >> fs[]) >>
+      rename[`isGlobal opn`, `gO_destApx apx`] >>
+      cheat (*
+      Cases_on `isGlobal opn ∧ gO_destApx apx ≠ gO_None`
+      >- (pop_assum strip_assume_tac >> simp[] >>
+          Cases_on `opn` >> fs[isGlobal_def] >>
+          Cases_on `apx` >> fs[gO_destApx_def] >> rveq >>
+          fs[known_op_def, NULL_EQ, bool_case_eq, case_eq_thms] >> rveq >>
+          imp_res_tac known_LENGTH_EQ_E >> fs[LENGTH_NIL_SYM] >> rveq >>
+          simp[evaluate_def] >>
+          rpt strip_tac >> rveq >> fs[evaluate_def, do_app_def, case_eq_thms] >>
+          fs[state_globals_approx_def, subspt_def] >> rveq >> simp[] >>
+          fs[known_def] >> rveq
+          >- (rename[`lookup n g0 = SOME (Tuple tg [])`,
+                     `kvrel g1 v (Block tg [])`] >>
+              `lookup n g1 = SOME (Tuple tg [])` by metis_tac[domain_lookup] >>
+              res_tac >> fs[] >> rveq >> fs[val_approx_val_def]) >>
+          (* TODO: clos_known$ is only necessary because of HOL issue #430 *)
+          rename[`lookup n g0 = SOME (clos_known$Int i)`, `kvrel g1 v (Number i)`] >>
+          `lookup n g1 = SOME (Int i)` by metis_tac[domain_lookup] >>
+          metis_tac[val_rel_def, val_approx_val_def, SOME_11]) >>
+      rename[`closLang$Op tr opn (MAP FST es)`,
+             `closSem$evaluate(MAP FST ealist,_,_)`] >>
+      rpt strip_tac >>
+      `ealist = [(Op tr opn (MAP FST es), apx)]`
+         by (Cases_on `isGlobal opn` >> fs[] >>
+             Cases_on `apx` >> fs[gO_destApx_def] >> every_case_tac >> fs[]) >>
+      pop_assum SUBST_ALL_TAC >> rveq >>
+      qpat_x_assum `¬(_ ∧ _)` kall_tac >> fs[] >>
+      dsimp[evaluate_def, result_case_eq, pair_case_eq] >>
+      sel_ihpc last >> simp[PULL_EXISTS] >>
+      rpt (disch_then (resolve_selected last) >> simp[]) >>
+      resolve_selected hd subspt_known_op_elist_globals >> simp[] >>
+      rpt (disch_then (resolve_selected hd) >> simp[]) >> strip_tac >>
+      (impl_keep_tac >- metis_tac[subspt_trans])
+      >- ((* args evaluate OK, do_app evaluates OK *)
+          metis_tac[kvrel_op_correct_Rval, EVERY2_REVERSE])
+      >- ((* args evaluate OK, do_app errors *)
+          rw[] >> imp_res_tac do_app_EQ_Rerr >> rw[] >>
+          metis_tac[result_CASES, pair_CASES])
+      >- ((* args error *) rw[] >> fs[krrel_err_rw] >>
+         metis_tac[result_CASES, pair_CASES]) *))
+  >- (say "fn" >>
+      simp[evaluate_def, pair_case_eq, result_case_eq,
+           known_def, bool_case_eq, case_eq_thms] >> rpt strip_tac >> rveq >> fs[] >>
+      rpt (pairarg_tac >> fs[]) >> rveq >> fs[] >>
+      imp_res_tac state_rel_max_app >> fs[] >>
+      dsimp[evaluate_def, case_eq_thms] >> imp_res_tac known_sing_EQ_E >> rveq >> fs[] >>
+      rveq >>
+      simp[exp_rel_def, PULL_EXISTS] >> metis_tac[kvrel_LIST_REL_val_approx])
+  >- (say "letrec" >>
+      simp[evaluate_def, pair_case_eq, result_case_eq, known_def, bool_case_eq,
+           case_eq_thms] >> rpt strip_tac >> rveq >> fs[letrec_case_eq] >>
+      rpt (pairarg_tac >> fs[]) >> rveq >> fs[] >>
+      fs[BAG_ALL_DISTINCT_BAG_UNION] >>
+      imp_res_tac state_rel_max_app >> fs[] >>
+      simp[evaluate_def, case_eq_thms, bool_case_eq] >> dsimp[] >>
+      simp[EVERY_MAP, EXISTS_MAP]
+      >- (disj1_tac >> simp[EVERY_MEM, FORALL_PROD] >>
+          imp_res_tac known_sing_EQ_E >> rveq >> fs[] >> rveq >>
+          sel_ihpc last >> simp[EVERY_GENLIST] >>
+          rpt (disch_then (resolve_selected last) >> simp[]) >>
+          rename1 `BAG_ALL_DISTINCT (elist_globals (MAP SND fns1))` >>
+          `∀n e. MEM (n,e) fns1 ⇒ n ≤ s02.max_app ∧ n ≠ 0`
+            by fs[EVERY_MEM, FORALL_PROD] >> simp[] >> strip_tac >>
+          simp[GSYM PULL_EXISTS] >> simp[Once EQ_SYM_EQ] >>
+          imp_res_tac LIST_REL_LENGTH >> fs[] >>
+          first_x_assum irule
+          >- (simp[LIST_REL_EL_EQN, EL_APPEND_EQN] >> qx_gen_tac `mm` >>
+              strip_tac >> rw[]
+              >- (fs[Once every_Fn_vs_NONE_EVERY] >>
+                  fs[EVERY_MAP] >> fs[EVERY_MEM, FORALL_PROD] >>
+                  metis_tac[])
+              >- (rename1 `LIST_REL val_approx_val apxs env1` >>
+                  qexists_tac `apxs` >> conj_tac
+                  >- metis_tac[kvrel_LIST_REL_val_approx] >>
+                  simp[LIST_REL_EL_EQN, EL_MAP] >>
+                  qx_gen_tac `nn` >> strip_tac >> pairarg_tac >>
+                  simp[] >> simp[exp_rel_def] >>
+                  map_every rename1 [`ksrel gg ss1 ss2`, `subspt g gg`,
+                                       `subspt g0 g`] >>
+                  ntac 2 (qexists_tac `g0`) >> simp[] >>
+                  rename1 `known [e1] env g0` >>
+                  Cases_on `known [e1] env g0` >>
+                  imp_res_tac known_sing_EQ_E >> fs[] >> rveq >>
+                  conj_tac >- metis_tac[subspt_trans] >>
+                  rename1 `known [subexp] env g0 = _` >>
+                  `elist_globals [subexp] = {||}`
+                    suffices_by metis_tac[known_emptySetGlobals_unchanged_g] >>
+                  fs[elglobals_EQ_EMPTY, MEM_MAP, PULL_EXISTS, FORALL_PROD] >>
+                  metis_tac[MEM_EL])
+              >- fs[LIST_REL_EL_EQN])
+          >- (irule EVERY2_APPEND_suff >> simp[] >>
+              simp[LIST_REL_GENLIST] >> qx_gen_tac `ii` >> strip_tac >>
+              rename1 `option_CASE lloc` >> Cases_on `lloc` >> simp[])) >>
+      disj2_tac >> fs[EXISTS_MEM, EXISTS_PROD] >> metis_tac[])
+  >- (say "app" >>
+      rpt gen_tac >> strip_tac >>
+      simp[evaluate_def, pair_case_eq, result_case_eq,
+           bool_case_eq, known_def, BAG_ALL_DISTINCT_BAG_UNION] >>
+      rpt strip_tac >> rveq >>
+      rpt (pairarg_tac >> fs[]) >> rveq >> fs[] >>
+      map_every imp_res_tac [known_sing_EQ_E, evaluate_SING] >> rveq >> fs[] >>
+      rveq
+      >- (map_every rename1 [
+            `known [fexp] apxs g1 = ([(fexp',fapx)], g)`,
+            `known args apxs g0 = (alist, g1)`,
+            `subspt g gg`] >>
+          patresolve `known [_] _ _ = _` (el 2) subspt_known_elist_globals >>
+          simp[] >> disch_then (resolve_selected (el 1)) >> simp[] >>
+          impl_tac >- fs[BAG_DISJOINT, DISJOINT_SYM] >> strip_tac >>
+          first_x_assum (patresolve `known args _ _ = _` last) >> simp[] >>
+          `subspt g1 gg` by metis_tac[subspt_trans] >>
+          rpt (disch_then (resolve_selected last) >> simp[]) >> rw[] >>
+          simp[evaluate_def] >> imp_res_tac known_LENGTH_EQ_E >> fs[] >>
+          first_x_assum (patresolve `known [_] _ _ = _` last) >> simp[] >>
+          disch_then (resolve_selected (el 2)) >> simp[] >>
+          disch_then (resolve_selected hd) >> simp[] >>
+          resolve_selected hd ssgc_evaluate >> simp[] >>
+          rpt (disch_then (resolve_selected hd) >> simp[]) >> strip_tac >>
+          impl_keep_tac
+          >- (patresolve `closSem$evaluate (MAP FST _, _, _) = _` last
+                         known_correct_approx >>
+              simp[] >> disch_then (resolve_selected hd) >> simp[] >>
+              metis_tac[ksrel_ssgc_free,kvrel_EVERY_vsgc_free,ksrel_sga,
+                        kvrel_LIST_REL_val_approx]) >>
+          rw[] >> simp[] >>
+          rename1 `evaluate_app loption1 v1 vs1 s21 = (result,ss1)` >>
+          `ssgc_free s21`
+            by metis_tac[ksrel_ssgc_free, ssgc_free_preserved_SING'] >> fs[] >>
+          first_x_assum (resolve_selected hd) >> simp[] >>
+          rpt (disch_then (resolve_selected hd) >> simp[]) >> strip_tac >>
+          `state_globals_approx s21 gg`
+            by (patresolve `known [_] _ _ = _` hd known_correct_approx >>
+                simp[] >> disch_then (resolve_selected last) >> simp[] >>
+                metis_tac[ksrel_ssgc_free,kvrel_EVERY_vsgc_free,ksrel_sga,
+                          kvrel_LIST_REL_val_approx]) >> fs[] >>
+          `vsgc_free v1`
+            by (patresolve `closSem$evaluate ([_],_,_) = (Rval [v1],_)` last
+                           ssgc_evaluate >> simp[]) >> fs[] >>
+          reverse (Cases_on `loption1`) >> simp[]
+          >- (first_x_assum irule >> simp[loptrel_def]) >>
+          rename1 `dest_Clos fapprox` >> Cases_on `dest_Clos fapprox` >>
+          simp[]
+          >- (first_x_assum irule >> simp[loptrel_def]) >>
+          rename1 `dest_Clos fapprox = SOME closapxvalue` >>
+          `∃clloc clarity. closapxvalue = (clloc, clarity)`
+            by metis_tac[pair_CASES] >> pop_assum SUBST_ALL_TAC >>
+          simp[] >> rename1 `LENGTH args > 0` >>
+          reverse (Cases_on `clarity = LENGTH args`) >> simp[]
+          >- (first_x_assum irule >> simp[loptrel_def]) >>
+          first_x_assum irule >> simp[loptrel_def] >>
+          qspecl_then [`[fexp]`, `apxs`, `g1`, `[(fexp',fapprox)]`, `g`]
+             mp_tac known_correct_approx >> simp[] >>
+          disch_then (resolve_selected last) >> simp[] >>
+          disch_then (qspec_then `gg` mp_tac) >> impl_tac
+          >- metis_tac[kvrel_LIST_REL_val_approx, ksrel_ssgc_free,
+                       kvrel_EVERY_vsgc_free, ksrel_sga] >>
+          fs[dest_Clos_eq_SOME] >> rveq >> rw[] >> simp[] >>
+          metis_tac[evaluate_length_imp])
+      >- (map_every rename1 [
+            `known [fexp] apxs g1 = ([(fexp',fapx)], g)`,
+            `known args apxs g0 = (alist, g1)`,
+            `subspt g gg`] >>
+          patresolve `known [_] _ _ = _` (el 2) subspt_known_elist_globals >>
+          simp[] >> disch_then (resolve_selected (el 1)) >> simp[] >>
+          impl_tac >- fs[BAG_DISJOINT, DISJOINT_SYM] >> strip_tac >>
+          first_x_assum (patresolve `known args _ _ = _` last) >> simp[] >>
+          `subspt g1 gg` by metis_tac[subspt_trans] >>
+          rpt (disch_then (resolve_selected last) >> simp[]) >> rw[] >>
+          simp[evaluate_def] >> imp_res_tac known_LENGTH_EQ_E >> fs[] >>
+          sel_ihpc last >> simp[] >>
+          disch_then (resolve_selected (el 2)) >> simp[] >>
+          disch_then (resolve_selected hd) >> simp[] >> reverse impl_tac
+          >- (rw[] >> simp[] >> fs[krrel_err_rw] >>
+              dsimp[result_case_eq] >> metis_tac[pair_CASES, result_CASES]) >>
+          conj_tac
+          >- (patresolve `closSem$evaluate (MAP FST _, _, _) = _` last
+                         known_correct_approx >>
+              simp[] >> disch_then (resolve_selected hd) >> simp[] >>
+              metis_tac[ksrel_ssgc_free,kvrel_EVERY_vsgc_free,ksrel_sga,
+                        kvrel_LIST_REL_val_approx]) >>
+          metis_tac [ssgc_evaluate])
+      >- (map_every rename1 [
+            `known [fexp] apxs g1 = ([(fexp',fapx)], g)`,
+            `known args apxs g0 = (alist, g1)`,
+            `subspt g gg`] >>
+          patresolve `known [_] _ _ = _` (el 2) subspt_known_elist_globals >>
+          simp[] >> disch_then (resolve_selected (el 1)) >> simp[] >>
+          impl_tac >- fs[BAG_DISJOINT, DISJOINT_SYM] >> strip_tac >>
+          first_x_assum (patresolve `known args _ _ = _` last) >> simp[] >>
+          `subspt g1 gg` by metis_tac[subspt_trans] >> strip_tac >>
+          nailIHx strip_assume_tac >>
+          simp[evaluate_def, bool_case_eq, result_case_eq, pair_case_eq] >>
+          imp_res_tac known_LENGTH_EQ_E >> rveq >> fs[] >>
+          fs[krrel_err_rw] >> dsimp[] >>
+          metis_tac[result_CASES,pair_CASES])
+      >- (map_every imp_res_tac [evaluate_IMP_LENGTH, known_LENGTH_EQ_E] >>
+          fs[] >> rw[] >> simp[evaluate_def]))
+  >- (say "tick" >> simp[dec_clock_def] >> rpt gen_tac >> strip_tac >>
+      simp[evaluate_def, bool_case_eq, known_def] >>
+      rename1 `(s0:('a,'b) closSem$state).clock = 0` >> Cases_on `s0.clock = 0` >>
+      fs[] >> rpt strip_tac >> rpt (pairarg_tac >> fs[]) >> rveq >> fs[] >>
+      simp[evaluate_def] >- fs[ksrel_def] >>
+      fs[dec_clock_def] >> fixeqs >> imp_res_tac known_sing_EQ_E >> rveq >>
+      fs[] >> rveq >>
+      map_every rename1 [
+        `known [exp1] apxs g0 = ([(exp2,apx)],g)`,
+        `evaluate([exp1],env1,s01 with clock := s01.clock - 1) = (res1,s1)`,
+        `ksrel gg s01 s02`] >>
+      sel_ihpc last >> simp[] >>
+      disch_then
+        (qspecl_then [`env2`, `s02 with clock := s02.clock - 1`, `gg`]
+                     mp_tac) >>
+      simp[] >> impl_keep_tac >- fs[ksrel_def] >>
+      `s02.clock = s01.clock` by fs[ksrel_def] >> simp[])
+  >- (say "call" >>
+      simp[evaluate_def, pair_case_eq, result_case_eq, case_eq_thms, bool_case_eq,
+           known_def] >> rw[]
+      >- (simp[] >> metis_tac[pair_CASES])
+      >- (rpt (pairarg_tac >> fs[]) >> rveq >> nailIHx strip_assume_tac >>
+          simp[evaluate_def] >> rw[] >>
+          imp_res_tac ksrel_find_code >> fs[])
+      >- (fixeqs >> rpt (pairarg_tac >> fs[]) >> rveq >> fs[] >>
+          nailIHx strip_assume_tac >>
+          imp_res_tac ksrel_find_code >> fs[])
+      >- (rpt (pairarg_tac >> fs[]) >> rveq >> fs[] >>
+          nailIHx strip_assume_tac >> simp[evaluate_def] >>
+          fs[krrel_err_rw] >>
+          dsimp[result_case_eq, case_eq_thms, pair_case_eq, bool_case_eq] >>
+          metis_tac[option_CASES, pair_CASES, result_CASES]))
+  >- (say "evaluate_app(nil)" >> simp[evaluate_def])
+  >- (say "evaluate_app(cons)" >> rpt gen_tac >> strip_tac >>
+      simp[evaluate_def, case_eq_thms, bool_case_eq, pair_case_eq, result_case_eq] >>
+      rpt strip_tac >> rveq >> fs[]
+      >- metis_tac[pair_CASES]
+      >- (simp[evaluate_def, case_eq_thms, bool_case_eq, pair_case_eq] >>
+          resolve_selected hd (GEN_ALL kvrel_dest_closure_SOME_Partial) >>
+          simp[PULL_EXISTS] >> imp_res_tac LIST_REL_LENGTH >> fs[] >>
+          rpt (disch_then (resolve_selected hd) >> simp[]) >>
+          strip_tac >> simp[] >> fs[ksrel_def])
+      >- (simp[evaluate_def, case_eq_thms, bool_case_eq, pair_case_eq] >>
+          resolve_selected hd (GEN_ALL kvrel_dest_closure_SOME_Partial) >>
+          simp[PULL_EXISTS] >> imp_res_tac LIST_REL_LENGTH >> fs[] >>
+          rpt (disch_then (resolve_selected hd) >> simp[]) >> strip_tac >>
+          simp[] >> fs[ksrel_def, dec_clock_def])
+      >- (simp[evaluate_def, case_eq_thms, bool_case_eq, pair_case_eq] >>
+          resolve_selected hd (GEN_ALL kvrel_dest_closure_SOME_Full) >>
+          simp[PULL_EXISTS] >> imp_res_tac LIST_REL_LENGTH >> fs[] >>
+          rpt (disch_then (resolve_selected hd) >> simp[]) >> strip_tac >>
+          simp[] >> imp_res_tac LIST_REL_LENGTH >> fs[ksrel_def])
+      >- (simp[evaluate_def, case_eq_thms, bool_case_eq, pair_case_eq] >>
+          resolve_selected hd (GEN_ALL kvrel_dest_closure_SOME_Full) >>
+          simp[PULL_EXISTS] >> imp_res_tac LIST_REL_LENGTH >> fs[] >>
+          rpt (disch_then (resolve_selected hd) >> simp[]) >> strip_tac >>
+          simp[] >> rename1 `ksrel g s01 s02` >>
+          `s02.clock = s01.clock` by fs[ksrel_def] >>
+          `s02.max_app = s01.max_app` by fs[ksrel_def] >>
+          imp_res_tac LIST_REL_LENGTH >> fs[] >> simp[PULL_EXISTS] >>
+          dsimp[] >> fs[PULL_EXISTS] >>
+          map_every rename1 [
+            `dest_closure _ lopt1 f1 (iarg1 :: iargs) =
+               SOME (Full_app exp1 env1 args1)`,
+            `evaluate([exp1],env1,dec_clock _ s01) = (Rval [v1], s11)`,
+            `kerel envapx gg exp1 exp2`] >> fs[exp_rel_def] >>
+          rpt disj1_tac >>
+          first_x_assum (patresolve `known [exp1] _ _ = _` last) >> simp[] >>
+          map_every rename1 [
+            `evaluate([exp1],env1,
+                      dec_clock (SUC (LENGTH iargs1) - LENGTH args2) s01)`,
+            `LIST_REL (kvrel gg) env1 env2`] >>
+          disch_then (qspecl_then [
+             `env2`,
+             `dec_clock (SUC (LENGTH iargs1) - LENGTH args2) s02`,
+             `gg`] mp_tac) >> simp[] >>
+          `set_globals exp1 = {||} ∧ EVERY vsgc_free env1 ∧
+           EVERY vsgc_free args1 ∧ esgc_free exp1`
+            by metis_tac[vsgc_free_Full_app_set_globals, EVERY_DEF,
+                         set_globals_empty_esgc_free] >> simp[] >>
+          qspec_then `[exp1]` mp_tac known_emptySetGlobals_unchanged_g >>
+          disch_then (resolve_selected hd) >> simp[] >>
+          disch_then SUBST_ALL_TAC >>
+          rename1 `LIST_REL val_approx_val envapx env1` >>
+          `LIST_REL val_approx_val envapx env1`
+            by metis_tac[kvrel_LIST_REL_val_approx] >>
+          `every_Fn_vs_NONE [exp1]`
+            by metis_tac[kvrel_dest_closure_every_Fn_vs_NONE] >>
+          impl_tac >- (simp[] >> fs[ksrel_def, dec_clock_def]) >> rw[] >>
+          simp[] >>
+          rename1 `loptrel f2 _ lopt1 lopt2` >>
+          reverse (Cases_on `lopt1`)
+          >- (fs[loptrel_arg1_SOME] >> rveq >>
+              imp_res_tac dest_closure_SOME_Full_app_args_nil >> fs[] >>
+              rveq >> simp[]) >>
+          qpat_x_assum `loptrel _ _ _ _` mp_tac >>
+          simp[loptrel_arg1_NONE] >> reverse strip_tac >> rveq
+          >- (imp_res_tac dest_closure_SOME_Full_app_args_nil >> fs[] >>
+              rveq >> simp[])
+          >- (imp_res_tac dest_closure_SOME_Full_app_args_nil >> fs[] >>
+              rveq >> simp[]) >>
+          first_x_assum irule >> simp[]
+          >- metis_tac[ssgc_free_preserved_SING', ssgc_free_dec_clock]
+          >- (patresolve `evaluate([exp1],_,_) = _` last ssgc_evaluate >>
+              simp[])
+          >- (patresolve `known [exp1] _ _ = _` hd known_correct_approx >>
+              simp[] >> disch_then (resolve_selected last) >> simp[] >>
+              metis_tac[ksrel_sga, ksrel_ssgc_free, kvrel_EVERY_vsgc_free])
+          >- simp[loptrel_def])
+      >- (imp_res_tac evaluate_SING >> fs[])
+      >- (simp[evaluate_def, case_eq_thms, bool_case_eq, pair_case_eq] >>
+          resolve_selected hd (GEN_ALL kvrel_dest_closure_SOME_Full) >>
+          simp[PULL_EXISTS] >> imp_res_tac LIST_REL_LENGTH >> fs[] >>
+          rpt (disch_then (resolve_selected hd) >> simp[]) >> strip_tac >>
+          simp[] >> rename1 `ksrel g s01 s02` >>
+          `s02.clock = s01.clock` by fs[ksrel_def] >>
+          imp_res_tac LIST_REL_LENGTH >> fs[] >> simp[PULL_EXISTS] >>
+          dsimp[] >>
+          map_every rename1 [
+            `dest_closure _ lopt1 f1 (iarg1 :: iargs) =
+               SOME (Full_app exp1 env1 args1)`,
+            `evaluate([exp1],env1,dec_clock _ s01) = (Rerr err1, s1)`,
+            `kerel envapx gg exp1 exp2`] >> fs[exp_rel_def] >>
+          first_x_assum (patresolve `known [exp1] _ _ = _` last) >> simp[] >>             map_every rename1 [
+            `evaluate([exp1],env1,
+                      dec_clock (SUC (LENGTH iargs1) - LENGTH args2) s01)`,
+            `LIST_REL (kvrel gg) env1 env2`] >>
+          disch_then (qspecl_then [
+             `env2`,
+             `dec_clock (SUC (LENGTH iargs1) - LENGTH args2) s02`,
+             `gg`] mp_tac) >> simp[] >>
+          `set_globals exp1 = {||} ∧ EVERY vsgc_free env1 ∧
+           EVERY vsgc_free args1 ∧ esgc_free exp1`
+            by metis_tac[vsgc_free_Full_app_set_globals, EVERY_DEF,
+                         set_globals_empty_esgc_free] >> simp[] >>
+          qspec_then `[exp1]` mp_tac known_emptySetGlobals_unchanged_g >>
+          disch_then (resolve_selected hd) >> simp[] >>
+          disch_then SUBST_ALL_TAC >>
+          rename1 `LIST_REL val_approx_val envapx env1` >>
+          `LIST_REL val_approx_val envapx env1`
+            by metis_tac[kvrel_LIST_REL_val_approx] >>
+          `every_Fn_vs_NONE [exp1]`
+            by metis_tac[kvrel_dest_closure_every_Fn_vs_NONE] >>
+          impl_tac >- (simp[] >> fs[ksrel_def, dec_clock_def]) >> rw[] >>
+          imp_res_tac state_rel_max_app >>
+          simp[] >> fs[krrel_err_rw] >>
+          rename1 `evaluate([exp2],_,_) = (res2,_)` >>
+          Cases_on `res2`
+          >- (imp_res_tac evaluate_SING >> simp[] >> metis_tac[pair_CASES]) >>
+          simp[])))
+
+
+
+
+
+(*******************************************************)
+
+
+(* TODO: MOVE candidates *)
+fun sel_ihpc f = first_x_assum (first_assum o mp_then (Pos f) mp_tac)
+fun resolve_selected f th = first_assum (mp_then (Pos f) mp_tac th)
+
+fun patresolve p f th = Q.PAT_ASSUM p (mp_then (Pos f) mp_tac th)
+
+(* repeated resolution, requiring that all preconditions get removed *)
+fun nailIHx k =
+  first_x_assum
+    (REPEAT_GTCL
+       (fn ttcl => fn th => first_assum (mp_then (Pos hd) ttcl th))
+       (k o assert (not o is_imp o #2 o strip_forall o concl)) o
+     assert (is_imp o #2 o strip_forall o concl))
+
+infix >~
+fun (f >~ g) th = f th >> g
+
+(* TODO: MOVE-HOL candidate; unused here *)
+val union_idem = Q.store_thm(
+  "union_idem[simp]",
+  `∀spt. union spt spt = spt`,
+  Induct >> simp[union_def]);
+
+val FINITE_BAG_FOLDR = Q.store_thm(
+  "FINITE_BAG_FOLDR",
+  `∀l f a.
+     FINITE_BAG a ∧ (∀e a. FINITE_BAG a ∧ MEM e l ⇒ FINITE_BAG (f e a)) ⇒
+     FINITE_BAG (FOLDR f a l)`,
+  Induct >> simp[]);
+
+val FINITE_set_globals = Q.store_thm(
+  "FINITE_set_globals[simp]",
+  `(∀e. FINITE_BAG (set_globals e)) ∧ ∀es. FINITE_BAG (elist_globals es)`,
+  ho_match_mp_tac set_globals_ind >> simp[] >> rpt strip_tac >>
+  rename1 `op_gbag opn` >> Cases_on `opn` >> simp[op_gbag_def]);
+
+val state_approx_better_definedg = Q.store_thm(
+  "state_approx_better_definedg",
+  `better_definedg g1 g2 ∧ state_globals_approx s g1 ⇒
+   state_globals_approx s g2`,
+  csimp[better_definedg_def, state_globals_approx_def, domain_lookup,
+        PULL_EXISTS] >>
+  metis_tac[val_approx_better_approx]);
+
+val evaluate_t = ``closSem$evaluate``
+val fixeqs = let
+  fun c t =
+    let
+      val r = rhs t
+      val (f, _) = strip_comb r
+    in
+      if same_const evaluate_t f then REWR_CONV EQ_SYM_EQ
+      else NO_CONV
+    end t
+in
+  RULE_ASSUM_TAC (CONV_RULE (TRY_CONV c))
+end
+
+
+
 
 val lem = Q.prove(
   `(∀a es env (s0:('a,'b) closSem$state) res s.
@@ -489,205 +3283,6 @@ val mapped_globals_grow = save_thm(
 fun say0 pfx s g = (print (pfx ^ ": " ^ s ^ "\n"); ALL_TAC g)
 val say = say0 "ssgc_evaluate0"
 
-val ssgc_evaluate0 = Q.prove(
-  `(∀a es env (s0:('a,'b) closSem$state) res s.
-      ssgc_free s0 ∧ EVERY vsgc_free env ∧
-      EVERY esgc_free es ∧ a = (es,env,s0) ∧
-      evaluate a = (res,s) ⇒
-      ssgc_free s ∧ rsgc_free res ∧
-      mglobals_extend s0 (SET_OF_BAG (elist_globals es)) s) ∧
-   (∀lopt f args (s0:('a,'b) closSem$state) res s.
-      ssgc_free s0 ∧ vsgc_free f ∧ EVERY vsgc_free args ∧
-      evaluate_app lopt f args s0 = (res, s) ⇒
-      ssgc_free s ∧ rsgc_free res ∧ mglobals_extend s0 ∅ s)`,
-  ho_match_mp_tac evaluate_ind >> rpt conj_tac >> simp[]
-  >- (* nil *) simp[evaluate_def]
-  >- ((* cons *) say "cons" >> rpt gen_tac >> strip_tac >>
-      simp[evaluate_def, pair_case_eq, result_case_eq,
-           PULL_EXISTS] >>
-      rename1 `evaluate([e1], env, s0)` >>
-      rpt gen_tac >> strip_tac >> rveq >> fs[]
-      >- (imp_res_tac evaluate_SING >> rveq >> fs[SET_OF_BAG_UNION] >>
-          metis_tac[mglobals_extend_trans])
-      >- (fs[SET_OF_BAG_UNION] >> metis_tac[mglobals_extend_trans])
-      >- (fs[SET_OF_BAG_UNION] >>
-          metis_tac[mglobals_extend_SUBSET, SUBSET_UNION]))
-  >- ((* var *) say "var" >> simp[evaluate_def] >> rw[] >> rw[] >>
-      metis_tac[EVERY_MEM, MEM_EL])
-  >- ((* If *) say "if" >> rpt gen_tac >> strip_tac >>
-      simp[evaluate_def, pair_case_eq, result_case_eq,
-           bool_case_eq] >>
-      rpt gen_tac >> reverse strip_tac >> rveq >> fixeqs >>
-      fs[SET_OF_BAG_UNION]
-      >- metis_tac[mglobals_extend_SUBSET, SUBSET_UNION, UNION_ASSOC,
-                   UNION_COMM]
-      >- metis_tac[mglobals_extend_SUBSET, SUBSET_UNION, UNION_ASSOC,
-                   UNION_COMM] >>
-      rename1 `evaluate ([gd], env, s0) = (Rval vs, s1)` >>
-      rename1 `mglobals_extend s0 set1 s1` >>
-      rename1 `mglobals_extend s1 set2 s` >>
-      `mglobals_extend s0 (set1 ∪ set2) s` by metis_tac[mglobals_extend_trans]>>
-      metis_tac[mglobals_extend_SUBSET, SUBSET_UNION, UNION_ASSOC, UNION_COMM])
-  >- ((* let *) say "let" >> rpt gen_tac >> strip_tac >>
-      simp[evaluate_def, pair_case_eq, result_case_eq] >>
-      rpt gen_tac >> strip_tac >> rveq >> fs[SUBSET_DEF, SET_OF_BAG_UNION] >>
-      metis_tac[mglobals_extend_trans, UNION_COMM, SUBSET_UNION,
-                mglobals_extend_SUBSET])
-  >- ((* raise *) say "raise" >> rpt gen_tac >> strip_tac >>
-      simp[evaluate_def, pair_case_eq, result_case_eq] >>
-      rpt gen_tac >> strip_tac >> rveq >> fs[SUBSET_DEF, SET_OF_BAG_UNION] >>
-      metis_tac[evaluate_SING, HD, EVERY_DEF])
-  >- ((* handle *) say "handle" >> rpt gen_tac >> strip_tac >>
-      simp[evaluate_def, pair_case_eq, result_case_eq,
-           error_case_eq] >>
-      rpt gen_tac >> strip_tac >> rveq >> fs[SUBSET_DEF, SET_OF_BAG_UNION] >>
-      metis_tac[mglobals_extend_SUBSET, SUBSET_UNION, mglobals_extend_trans])
-  >- ((* op *) say "op" >> rpt gen_tac >> strip_tac >>
-      Cases_on `op = Install` >- cheat >>
-      simp[evaluate_def, pair_case_eq, result_case_eq] >>
-      rpt gen_tac >> strip_tac >> rveq >> fs[]
-      >- (IMP_RES_THEN mp_tac do_app_ssgc >> simp[EVERY_REVERSE] >>
-          fs[SET_OF_BAG_UNION] >>
-          metis_tac[mglobals_extend_trans, UNION_COMM])
-      >- (IMP_RES_THEN mp_tac do_app_ssgc >> simp[EVERY_REVERSE] >>
-          rename1 `Rerr err` >> Cases_on `err` >> simp[] >>
-          fs[SET_OF_BAG_UNION] >>
-          metis_tac[SUBSET_UNION, mglobals_extend_SUBSET])
-      >- (fs[SET_OF_BAG_UNION] >>
-          metis_tac[SUBSET_UNION, mglobals_extend_SUBSET]))
-  >- ((* Fn *) say "fn" >>
-      simp[evaluate_def, case_eq_thms, bool_case_eq] >> rpt gen_tac >>
-      strip_tac >> rveq >> fs[] >> metis_tac[EVERY_lookup_vars])
-  >- ((* Letrec *) say "letrec" >>
-      simp[evaluate_def, bool_case_eq, case_eq_thms] >>
-      rpt (gen_tac ORELSE disch_then strip_assume_tac) >> rveq >>
-      fs[EVERY_GENLIST] >>
-      imp_res_tac EVERY_lookup_vars >> fs[] >>
-      metis_tac[mglobals_extend_SUBSET, SUBSET_UNION])
-  >- ((* App *) say "app" >>
-      rpt gen_tac >> strip_tac >>
-      simp[evaluate_def, bool_case_eq, pair_case_eq,
-           result_case_eq] >>
-      rpt (gen_tac ORELSE disch_then strip_assume_tac) >> rveq >> fs[]
-      >- (imp_res_tac evaluate_SING >> rveq >>
-          fs[SET_OF_BAG_UNION] >>
-          metis_tac[mglobals_extend_trans, UNION_COMM, UNION_EMPTY])
-      >- (fs[SET_OF_BAG_UNION] >> metis_tac[mglobals_extend_trans, UNION_COMM])
-      >- (fs[SET_OF_BAG_UNION] >>
-          metis_tac[mglobals_extend_SUBSET, SUBSET_UNION]))
-  >- ((* Tick *)
-      say "tick" >> simp[evaluate_def, bool_case_eq] >>
-      rpt (gen_tac ORELSE disch_then strip_assume_tac) >> rveq >> fixeqs >>
-      fs[])
-  >- ((* Call *)
-      say "call" >> rpt gen_tac >> strip_tac >>
-      simp[evaluate_def, pair_case_eq, result_case_eq, case_eq_thms,
-           bool_case_eq] >>
-      rpt (gen_tac ORELSE disch_then strip_assume_tac) >> rveq >> fixeqs >>
-      fs[] >> fs[find_code_def, case_eq_thms, pair_case_eq] >> rveq >>
-      rename1 `FLOOKUP _.code _ = SOME (_, fbody)` >>
-      `set_globals fbody = {||}` suffices_by
-        (strip_tac >> fs[] >> imp_res_tac set_globals_empty_esgc_free >>
-         fs[] >> metis_tac[mglobals_extend_trans, UNION_EMPTY]) >>
-      fs[ssgc_free_def] >> metis_tac[])
-  >- ((* evaluate_app *)
-      say "evaluate_app" >> rpt gen_tac >> strip_tac >>
-      simp[evaluate_def, case_eq_thms, bool_case_eq, pair_case_eq] >>
-      rpt (gen_tac ORELSE disch_then strip_assume_tac) >> rveq >> fixeqs >>
-      fs[]
-      >- (fs[dest_closure_def, case_eq_thms, bool_case_eq] >> rveq >>
-          fs[] >> pairarg_tac >> fs[bool_case_eq])
-      >- (fs[dest_closure_def, case_eq_thms, bool_case_eq] >> rveq >>
-          fs[EVERY_REVERSE, EVERY_DROP, EVERY_TAKE]
-          >- (imp_res_tac set_globals_empty_esgc_free >> fs[] >>
-              metis_tac[mglobals_extend_trans, UNION_EMPTY]) >>
-          pairarg_tac >>
-          fs[elglobals_EQ_EMPTY, bool_case_eq] >> rveq >>
-          fs[EVERY_DROP, EVERY_TAKE, EVERY_REVERSE, EVERY_GENLIST,
-             elglobals_EQ_EMPTY, MEM_MAP, PULL_EXISTS] >>
-          rename1 `EL ii fns = (_, fbody)` >>
-          `ii < LENGTH fns` by simp[] >>
-          `set_globals fbody = {||}` by metis_tac[MEM_EL,SND] >>
-          imp_res_tac set_globals_empty_esgc_free >> fs[] >>
-          metis_tac[mglobals_extend_trans, UNION_EMPTY])
-      >- (fs[dest_closure_def, case_eq_thms, bool_case_eq] >> rveq >>
-          fs[EVERY_TAKE, EVERY_REVERSE, EVERY_DROP]
-          >- (imp_res_tac set_globals_empty_esgc_free >> fs[]) >>
-          pairarg_tac >>
-          fs[elglobals_EQ_EMPTY, bool_case_eq] >> rveq >>
-          fs[EVERY_DROP, EVERY_TAKE, EVERY_REVERSE, EVERY_GENLIST,
-             elglobals_EQ_EMPTY, MEM_MAP, PULL_EXISTS] >>
-          rename1 `EL ii fns = (_, fbody)` >>
-          `ii < LENGTH fns` by simp[] >>
-          `set_globals fbody = {||}` by metis_tac[MEM_EL,SND] >>
-          imp_res_tac set_globals_empty_esgc_free >> fs[])
-      >- (fs[dest_closure_def, case_eq_thms, bool_case_eq] >> rveq >>
-          fs[EVERY_TAKE, EVERY_REVERSE, EVERY_DROP]
-          >- (imp_res_tac set_globals_empty_esgc_free >> fs[]) >>
-          pairarg_tac >>
-          fs[elglobals_EQ_EMPTY, bool_case_eq] >> rveq >>
-          fs[EVERY_DROP, EVERY_TAKE, EVERY_REVERSE, EVERY_GENLIST,
-             elglobals_EQ_EMPTY, MEM_MAP, PULL_EXISTS] >>
-          rename1 `EL ii fns = (_, fbody)` >>
-          `ii < LENGTH fns` by simp[] >>
-          `set_globals fbody = {||}` by metis_tac[MEM_EL,SND] >>
-          imp_res_tac set_globals_empty_esgc_free >> fs[])))
-
-val ssgc_evaluate = save_thm(
-  "ssgc_evaluate",
-  ssgc_evaluate0 |> CONJUNCT1 |> SIMP_RULE bool_ss []);
-
-val known_preserves_setGlobals = Q.store_thm(
-  "known_preserves_setGlobals",
-  `∀es as g0 all g.
-      known es as g0 = (all,g) ⇒
-      elist_globals (MAP FST all) = elist_globals es`,
-  ho_match_mp_tac known_ind >> simp[known_def] >> rpt strip_tac >>
-  rpt (pairarg_tac >> fs[]) >> rw[] >> fs[] >> imp_res_tac known_sing_EQ_E >>
-  rw[] >> fs[] >> rw[] >> simp[elist_globals_FOLDR]
-  >- (rename [`isGlobal opn`] >> Cases_on `opn` >> fs[isGlobal_def] >>
-      rename [`gO_destApx a`] >> Cases_on `a` >>
-      fs[gO_destApx_def, op_gbag_def, elist_globals_FOLDR] >>
-      fs[known_op_def, bool_case_eq, case_eq_thms, NULL_EQ] >> rw[op_gbag_def]) >>
-  irule FOLDR_CONG >> simp[] >>
-  simp[LIST_EQ_REWRITE, EL_MAP] >>
-  rpt strip_tac >> pairarg_tac >>
-  simp[]>> rw[] >>
-  qmatch_abbrev_tac `set_globals (FST (HD (FST (known [X] ENV G0)))) =
-                     set_globals X` >>
-  rename1 `EL x fns = (nn,X)` >> `MEM (nn,X) fns` by metis_tac[MEM_EL] >>
-  res_tac >> rfs[] >>
-  `∃X' APX g'. known [X] ENV G0 = ([(X',APX)], g')` by metis_tac[known_sing] >>
-  fs[])
-
-val mglobals_extend_EMPTY_state_globals_approx = Q.store_thm(
-  "mglobals_extend_EMPTY_state_globals_approx",
-  `mglobals_extend s1 ∅ s2 ∧ mapped_globals s1 ⊆ mapped_globals s2 ⇒
-   (state_globals_approx s1 g ⇔ state_globals_approx s2 g)`,
-  simp[mglobals_extend_def, state_globals_approx_def, EXTENSION, SUBSET_DEF,
-       mapped_globals_def] >>
-  metis_tac[]);
-
-val known_preserves_esgc_free = Q.store_thm(
-  "known_preserves_esgc_free",
-  `∀es as g0 all g.
-     known es as g0 = (all,g) ∧ EVERY esgc_free es ⇒
-     EVERY (esgc_free o FST) all`,
-  ho_match_mp_tac known_ind >> simp[known_def] >> rpt strip_tac >>
-  rpt (pairarg_tac >> fs[]) >> rw[] >> fs[] >> imp_res_tac known_sing_EQ_E >>
-  rw[] >> fs[] >> rw[ALL_EL_MAP]
-  >- (every_case_tac >> simp[] >> fs[EVERY_MEM, MEM_MAP, PULL_EXISTS])
-  >- (imp_res_tac known_preserves_setGlobals >> fs[])
-  >- (fs[elglobals_EQ_EMPTY, MEM_MAP, PULL_EXISTS] >> rpt strip_tac >>
-      pairarg_tac >> rw[] >> fs[FORALL_PROD] >>
-      qmatch_abbrev_tac
-        `set_globals (FST (HD (FST (known [X] ENV g00)))) = _` >>
-      rename1 `MEM (nn, X) fns` >>
-      rpt (first_x_assum (qspecl_then [`nn`, `X`] mp_tac)) >> simp[] >>
-      `∃X' APX gg. known [X] ENV g00 = ([(X',APX)], gg)`
-        by metis_tac[known_sing] >> simp[] >>
-      imp_res_tac known_preserves_setGlobals >> fs[]))
-
 val ssgc_free_preserved_SING = Q.store_thm(
   "ssgc_free_preserved_SING",
   `known [e1] as g0 = ([(e1',a)], g) ∧ esgc_free e1 ∧ ssgc_free s0 ∧
@@ -698,33 +3293,6 @@ val ssgc_free_preserved_SING = Q.store_thm(
      by metis_tac[known_preserves_esgc_free] >>
   `EVERY esgc_free [e1']` by fs[] >>
   metis_tac[ssgc_evaluate]);
-
-val known_op_correct_approx = Q.store_thm(
-  "known_op_correct_approx",
-  `known_op opn args g0 = (a,g) ∧ LIST_REL val_approx_val args vs ∧
-   subspt g g' ∧
-   state_globals_approx s0 g' ∧
-   do_app opn vs s0 = Rval (v, s) ⇒
-   state_globals_approx s g' ∧ val_approx_val a v`,
-  Cases_on `opn` >>
-  simp[known_op_def, do_app_def, case_eq_thms, va_case_eq, bool_case_eq,
-       pair_case_eq] >>
-  rpt strip_tac >> rveq >> fs[]
-  >- (fs[state_globals_approx_def] >> res_tac >>
-      fs[subspt_def] >> metis_tac[SOME_11, domain_lookup])
-  >- (fs[state_globals_approx_def, get_global_def, EL_LUPDATE,
-         lookup_insert, bool_case_eq] >> rw[] >> simp[] >>
-      fs[subspt_def])
-  >- (fs[state_globals_approx_def, get_global_def, EL_LUPDATE,
-         bool_case_eq, lookup_insert] >> rw[] >> fs[subspt_def] >>
-      metis_tac[val_approx_val_merge_I])
-  >- (fs[state_globals_approx_def, get_global_def, EL_APPEND_EQN,
-         bool_case_eq] >> rw[]
-      >- metis_tac[]
-      >- (rename1 `nn - LENGTH (ss:('a,'b) closSem$state).globals` >>
-          `nn - LENGTH ss.globals = 0` by simp[] >>
-          pop_assum (fn th => fs[th])))
-  >- (rveq >> fs[LIST_REL_EL_EQN]));
 
 val LENGTH_clos_gen = Q.prove(`
   ∀ls x c.
@@ -744,287 +3312,6 @@ val letrec_case_eq = Q.prove(`
   | SOME n => clos_gen n 0 fns) =
   GENLIST (case loc of NONE => K Other | SOME n => λi. Clos (n+ 2*i) (FST (EL i fns))) (LENGTH fns)`,
   Cases_on`loc`>>fs[clos_gen_eq,REPLICATE_GENLIST])
-
-val say = say0 "known_correct_approx"
-val known_correct_approx = Q.store_thm(
-  "known_correct_approx",
-  `∀es as g0 all g env s0 s result g'.
-     known es as g0 = (all,g) ∧ BAG_ALL_DISTINCT (elist_globals es) ∧
-     LIST_REL val_approx_val as env ∧ subspt g0 g ∧ subspt g g' ∧
-     state_globals_approx s0 g' ∧ ssgc_free s0 ∧ EVERY vsgc_free env ∧
-     EVERY esgc_free es ∧ evaluate(MAP FST all, env, s0) = (result, s)
-    ⇒
-     state_globals_approx s g' ∧
-     ∀vs. result = Rval vs ⇒ LIST_REL val_approx_val (MAP SND all) vs`,
-  ho_match_mp_tac known_ind >> simp[known_def] >>
-  rpt conj_tac >> rpt (gen_tac ORELSE disch_then strip_assume_tac)
-  >- (* nil *) (say "nil" >> fs[evaluate_def] >> rw[])
-  >- (say "cons" >> rpt (pairarg_tac >> fs[]) >> rveq >>
-      rename1 `known [exp1] as g0` >>
-      `∃exp1' a1 g1. known [exp1] as g0 = ([(exp1',a1)], g1)`
-         by metis_tac[known_sing] >> fs[] >> rveq >> fs[] >>
-      rename1 `known [exp1] EA g0 = ([(exp1',a1)], g1)` >>
-      rename1 `known (exp2::erest) EA g1 = (al2,g)` >>
-      `LENGTH al2 = LENGTH (exp2::erest)` by metis_tac[known_LENGTH, FST] >>
-      fs[] >>
-      `∃exp2' a2 arest. al2 = (exp2',a2)::arest`
-        by (Cases_on `al2` >> fs[] >> metis_tac[pair_CASES]) >> rveq >>
-      patresolve `known [_] _ _ = _` hd subspt_known_elist_globals >> simp[] >>
-      disch_then (resolve_selected hd) >>
-      fs[BAG_ALL_DISTINCT_BAG_UNION] >> strip_tac >>
-      fs[evaluate_def, pair_case_eq, result_case_eq] >> rveq
-      >- (rename1 `evaluate ([exp1'], env, s0) = (Rval v1, s1)` >>
-          first_x_assum (Q.PAT_ASSUM `closSem$evaluate([_],_,_) = _` o
-                         mp_then (Pos last) mp_tac) >>
-          simp[] >>
-          disch_then (resolve_selected last) >> simp[] >>
-          impl_keep_tac >- metis_tac[subspt_trans] >> strip_tac >>
-          simp[] >> rveq >> fs[] >> sel_ihpc last >> simp[] >>
-          metis_tac[ssgc_free_preserved_SING])
-      >- (simp[] >>
-          first_x_assum (Q.PAT_ASSUM `closSem$evaluate ([_],_,_) = _` o
-                         mp_then (Pos last) mp_tac) >>
-          simp[] >>
-          disch_then (resolve_selected last) >> simp[] >>
-          impl_tac >- metis_tac[subspt_trans] >> rw[] >>
-          sel_ihpc last >> simp[] >> disch_then irule >> simp[]>>
-          metis_tac[ssgc_free_preserved_SING])
-      >- (simp[] >> sel_ihpc last >> simp[] >> metis_tac[subspt_trans]))
-  >- ((* Var *) say "var" >>
-      fs[any_el_ALT, evaluate_def, bool_case_eq] >>
-      fs[LIST_REL_EL_EQN])
-  >- ((* If *) say "if" >>
-      rpt (pairarg_tac >> fs[]) >> rveq >> fs[BAG_ALL_DISTINCT_BAG_UNION] >>
-      rename1 `known [ge] as g0 = (_, g1)` >>
-      `∃ge' apx1. known [ge] as g0 = ([(ge',apx1)], g1)`
-         by metis_tac[known_sing, PAIR_EQ] >>
-      rename1 `known [tb] as g1 = (_, g2)` >>
-      `∃tb' apx2. known [tb] as g1 = ([(tb',apx2)], g2)`
-         by metis_tac[known_sing, PAIR_EQ] >>
-      rename1 `known [eb] as g2 = (_, g3)` >>
-      `∃eb' apx3. known [eb] as g2 = ([(eb',apx3)], g3)`
-         by metis_tac[known_sing, PAIR_EQ] >> fs[] >> rveq >> fs[] >> rveq >>
-      `subspt g0 g1 ∧ subspt g1 g2 ∧ subspt g2 g3`
-         by (`∃al01. known [ge;tb] as g0 = (al01,g2)` by simp[known_def] >>
-             first_assum (mp_then (Pos hd) mp_tac subspt_known_elist_globals) >>
-             simp[] >>
-             disch_then (first_assum o mp_then (Pos hd) mp_tac) >>
-             simp[] >> strip_tac >>
-             qpat_x_assum `known [_] _ g0 = (_,g1)`
-               (mp_then (Pos hd) mp_tac subspt_known_elist_globals) >>
-             simp[] >> disch_then (first_assum o mp_then (Pos hd) mp_tac) >>
-             simp[]) >>
-      reverse
-        (fs[evaluate_def, pair_case_eq, result_case_eq,
-            bool_case_eq]) >> rveq >> fixeqs >> simp[]
-      >- (first_x_assum (first_assum o mp_then (Pos last) mp_tac) >> simp[] >>
-          metis_tac[subspt_trans])
-      >- (sel_ihpc last >> simp[] >> metis_tac[subspt_trans]) >>
-      (* two cases from here on *)
-      rename1 `evaluate ([ge'], env, s0) = (Rval gvs, s1)` >>
-      first_x_assum
-        (Q.PAT_ASSUM `evaluate ([ge'], _, _) = _` o mp_then (Pos last) mp_tac) >>
-      simp[] >> disch_then (resolve_selected last) >> simp[] >>
-      (impl_keep_tac >- metis_tac[subspt_trans]) >>
-      strip_tac >> rveq >> fs[] >> rveq >> sel_ihpc last >> simp[] >>
-      disch_then (resolve_selected (el 2)) >> simp[] >>
-      impl_tac
-      >- metis_tac[ssgc_free_preserved_SING]
-      >- metis_tac[val_approx_val_merge_I]
-      >- (conj_tac >- metis_tac[subspt_trans] >>
-          irule (GEN_ALL ssgc_free_preserved_SING) >> metis_tac[])
-      >- metis_tac[val_approx_val_merge_I])
-  >- ((* let *) say "let" >>
-      rpt (pairarg_tac >> fs[]) >> rveq >> fs[] >>
-      fs[evaluate_def, case_eq_thms, pair_case_eq, result_case_eq] >>
-      rveq >> sel_ihpc last >> simp[] >> disch_then (resolve_selected last) >>
-      simp[] >> fs[BAG_ALL_DISTINCT_BAG_UNION] >>
-      map_every rename1 [`known [bod] _ g1 = (_, g)`,
-                           `known _ _ g0 = (_, g1)`] >>
-      patresolve `known [_] _ _ = _` (el 2) subspt_known_elist_globals >>
-      simp[] >> disch_then (resolve_selected hd) >> simp[] >>
-      (impl_tac >- fs[BAG_DISJOINT, DISJOINT_SYM]) >> strip_tac >> simp[] >>
-      (impl_tac >- metis_tac[subspt_trans]) >> strip_tac >> simp[] >>
-      imp_res_tac known_sing_EQ_E >> rveq >> fs[] >> rveq >>
-      sel_ihpc last >> simp[EVERY2_APPEND_suff] >>
-      disch_then (resolve_selected (el 2)) >> simp[] >> reverse impl_tac
-      >- rw[] >> resolve_selected hd ssgc_evaluate >> simp[] >>
-      disch_then (resolve_selected last) >> simp[] >>
-      imp_res_tac known_preserves_esgc_free >> simp[ALL_EL_MAP])
-  >- ((* raise *) say "raise" >>
-      pairarg_tac >> fs[] >> imp_res_tac known_sing_EQ_E >> fs[] >> rveq >>
-      fs[evaluate_def, pair_case_eq, result_case_eq] >> rveq >>
-      simp[] >> metis_tac[])
-  >- ((* tick *) say "tick" >>
-      pairarg_tac >> fs[] >> imp_res_tac known_sing_EQ_E >> fs[] >> rveq >>
-      fs[evaluate_def, pair_case_eq, result_case_eq,
-         bool_case_eq] >> rveq >> simp[] >>
-      fixeqs >> first_x_assum irule >> simp[] >>
-      metis_tac[state_globals_approx_dec_clock, ssgc_free_dec_clock])
-  >- ((* handle *) say "handle" >>
-      rpt (pairarg_tac >> fs[]) >> rveq >> fs[] >>
-      map_every rename1 [`known _ (_ :: _) g1 = (_, g)`,
-                           `known _ _ g0 = (_, g1)`] >>
-      patresolve `known _ (_ :: _) _ = _` (el 2) subspt_known_elist_globals >>
-      simp[] >> disch_then (resolve_selected hd) >> simp[] >>
-      fs[BAG_ALL_DISTINCT_BAG_UNION] >> strip_tac >>
-      fs[evaluate_def, pair_case_eq, result_case_eq,
-         error_case_eq] >> rveq >> fs[] >>
-      imp_res_tac known_sing_EQ_E >> rveq >> fs[] >> rveq
-      >- (sel_ihpc last >> simp[] >> disch_then (resolve_selected last) >>
-          simp[] >> reverse impl_keep_tac
-          >- metis_tac[val_approx_val_merge_I] >>
-          metis_tac[subspt_trans])
-      >- (first_x_assum (Q.PAT_ASSUM `closSem$evaluate _ = (Rerr _, _)` o
-                         mp_then (Pos last) mp_tac) >>
-          simp[] >> disch_then (resolve_selected last) >> simp[] >>
-          impl_keep_tac >- metis_tac[subspt_trans] >>
-          strip_tac >> sel_ihpc last >> simp[PULL_EXISTS] >>
-          disch_then (resolve_selected (el 2)) >> simp[] >> reverse impl_tac
-          >- metis_tac[val_approx_val_merge_I] >>
-          conj_tac >- metis_tac[ssgc_free_preserved_SING] >>
-          resolve_selected hd ssgc_evaluate >>
-          disch_then (resolve_selected last) >> simp[] >> reverse impl_tac
-          >- simp[] >>
-          imp_res_tac known_preserves_esgc_free >> fs[])
-      >- (sel_ihpc last >> simp[] >> metis_tac[subspt_trans]))
-  >- ((* call *) say "call" >> pairarg_tac >> fs[] >> rveq >> fs[] >>
-      fs[evaluate_def, pair_case_eq, result_case_eq, case_eq_thms,
-         bool_case_eq] >>
-      rveq >> fs[] >> sel_ihpc last >> simp[] >> fixeqs >>
-      disch_then (resolve_selected last) >> simp[] >>
-      reverse (rpt strip_tac)
-      >- (rveq >> imp_res_tac evaluate_SING >> simp[]) >>
-      map_every rename1 [
-        `evaluate([body],args,dec_clock (ticks+1) s1) = (result,s)`,
-        `evaluate(MAP FST alist,env,s0) = (Rval vs, s1)`] >>
-      `ssgc_free s1 ∧ EVERY vsgc_free vs`
-         by (resolve_selected hd ssgc_evaluate >> simp[] >>
-             disch_then (resolve_selected last) >> simp[] >>
-             reverse impl_tac >- simp[] >>
-             imp_res_tac known_preserves_esgc_free >> simp[ALL_EL_MAP]) >>
-      `set_globals body = {||}`
-         by (Q.UNDISCH_THEN `ssgc_free s1` mp_tac >>
-             simp[ssgc_free_def] >> fs[find_code_def, case_eq_thms, pair_case_eq] >>
-             metis_tac[])  >>
-      `mapped_globals s1 ⊆ mapped_globals s`
-         by metis_tac[mapped_globals_grow, mapped_globals_dec_clock] >>
-      `mglobals_extend s1 {} s`
-         by (qspecl_then [`[body]`, `args`, `dec_clock (ticks+1) s1`, `result`, `s`]
-                         mp_tac ssgc_evaluate >> simp[] >>
-             fs[find_code_def, case_eq_thms, pair_case_eq] >> rveq >>
-             simp[set_globals_empty_esgc_free]) >>
-      metis_tac[mglobals_extend_EMPTY_state_globals_approx])
-  >- ((* op *) say "op" >> rpt (pairarg_tac >> fs[]) >> rveq >>
-      Cases_on `op = Install` >- cheat >>
-      fs[BAG_ALL_DISTINCT_BAG_UNION] >>
-      resolve_selected hd subspt_known_op_elist_globals >> simp[] >>
-      disch_then (resolve_selected hd) >> simp[] >> strip_tac >>
-      rename[`known_op opn`] >> Cases_on `isGlobal opn` >> fs[] >| [
-        rename[`gO_destApx apx`] >> Cases_on `gO_destApx apx` >| [
-          fs[evaluate_def, do_app_def] >> rveq >> simp[] >> Cases_on `apx` >>
-          fs[gO_destApx_def, bool_case_eq, NULL_EQ],
-          fs[evaluate_def, do_app_def] >> rveq >> simp[] >> Cases_on `apx` >>
-          fs[gO_destApx_def, bool_case_eq, NULL_EQ],
-          ALL_TAC
-        ],
-        ALL_TAC
-      ] >>
-      fs[evaluate_def, pair_case_eq, result_case_eq] >> rveq >>
-      fs[] >> sel_ihpc last >> simp[] >> disch_then (resolve_selected last) >>
-      simp[] >> (impl_keep_tac >- metis_tac[subspt_trans]) >>
-      simp[] >> strip_tac >>
-      metis_tac[known_op_correct_approx, LIST_REL_REVERSE_EQ])
-  >- (say "app" >> rpt (pairarg_tac >> fs[]) >> rveq >>
-      imp_res_tac known_sing_EQ_E >> rveq >> fs[] >> rveq >>
-      patresolve `known [_] _ _ = _` (el 2) subspt_known_elist_globals >>
-      simp[] >> fs[BAG_ALL_DISTINCT_BAG_UNION] >>
-      disch_then (resolve_selected hd) >> simp[] >> impl_tac
-      >- fs[BAG_DISJOINT, DISJOINT_SYM] >> strip_tac >>
-      fs[evaluate_def, bool_case_eq, pair_case_eq,
-         result_case_eq] >> rveq >> fs[]
-      >- (rename1 `evaluate(MAP FST args, env, s0) = (Rval argvs, s1)` >>
-          rename1 `known exps apxs g0 = (args, g1)` >>
-          rename1 `state_globals_approx s0 g'` >>
-          `subspt g1 g'` by metis_tac[subspt_trans] >>
-          nailIHx strip_assume_tac >> fs[] >>
-          sel_ihpc last >> simp[] >> disch_then (resolve_selected (el 2)) >>
-          simp[] >> resolve_selected hd ssgc_evaluate >> simp[] >>
-          disch_then (resolve_selected last) >> simp[] >>
-          impl_keep_tac
-          >- (imp_res_tac known_preserves_esgc_free >> fs[ALL_EL_MAP]) >>
-          simp[] >> rpt (disch_then strip_assume_tac) >> rveq >> fs[] >>
-          rename1 `evaluate_app _ fval argvs s2 = (result, s)` >>
-          reverse conj_tac
-          >- (Cases_on `result` >> simp[] >>
-              imp_res_tac evaluate_app_length_imp >>
-              rename1 `LENGTH aa = 1` >> Cases_on `aa` >> fs[LENGTH_NIL]) >>
-          rename1 `evaluate([fexp],env,s1) = (Rval[fval],s2)` >>
-          qspecl_then [`[fexp]`, `env`, `s1`, `Rval [fval]`, `s2`]
-                      mp_tac ssgc_evaluate >> simp[] >>
-          impl_tac
-          >- (IMP_RES_THEN mp_tac known_preserves_esgc_free >> simp[]) >>
-          strip_tac >>
-          qpat_x_assum `evaluate_app _ _ _ _ = _`
-             (fn th =>
-                 (mp_tac o PART_MATCH (last o strip_conj o #1 o dest_imp)
-                                      (CONJUNCT2 ssgc_evaluate0) o concl) th >>
-                 assume_tac th) >> simp[] >>
-          strip_tac >>
-          `mapped_globals s2 ⊆ mapped_globals s` suffices_by
-            metis_tac[mglobals_extend_EMPTY_state_globals_approx] >>
-          metis_tac[lem])
-      >- (rename1 `evaluate(MAP FST args, env, s0) = (Rval argvs, s1)` >>
-          rename1 `known exps apxs g0 = (args, g1)` >>
-          rename1 `state_globals_approx s0 g'` >>
-          `subspt g1 g'` by metis_tac[subspt_trans] >>
-          nailIHx strip_assume_tac >> fs[] >> sel_ihpc last >> simp[] >>
-          disch_then irule >>
-          qspecl_then [`MAP FST args`, `env`, `s0`, `Rval argvs`, `s1`]
-                      mp_tac ssgc_evaluate >> simp[] >>
-          impl_tac
-          >- (simp[ALL_EL_MAP] >> metis_tac[known_preserves_esgc_free]) >>
-          simp[])
-      >- (sel_ihpc last >> simp[] >> metis_tac[subspt_trans]))
-  >- (say "fn" >> rpt (pairarg_tac >> fs[]) >> rveq >>
-      imp_res_tac known_sing_EQ_E >> rveq >> fs[] >> rveq >>
-      fs[evaluate_def, bool_case_eq, case_eq_thms] >> rveq >> fs[] >> every_case_tac >>
-      simp[])
-  >- (say "letrec" >> rpt (pairarg_tac >> fs[]) >> imp_res_tac known_sing_EQ_E>>
-      rveq >> fs[] >> rveq >>
-      fs[evaluate_def, bool_case_eq,clos_gen_eq]
-      >- (fixeqs >>
-          qmatch_assum_abbrev_tac
-            `closSem$evaluate([_], GENLIST (_ (MAP ff _)) _ ++ _, _) = _` >>
-          rename1
-            `closSem$evaluate([body'],
-                              GENLIST (Recclosure lopt [] env (MAP ff fns))
-                                      (LENGTH fns) ++ env,
-                              s0) = (result, s)` >>
-          first_x_assum (qspecl_then [
-            `GENLIST (Recclosure lopt [] env (MAP ff fns)) (LENGTH fns) ++ env`,
-            `s0`] mp_tac) >> simp[] >>
-          imp_res_tac LIST_REL_LENGTH >>
-          simp[LIST_REL_EL_EQN, EL_GENLIST, EL_APPEND_EQN, EVERY_MEM,
-               MEM_GENLIST, PULL_EXISTS] >>
-          disch_then match_mp_tac
-          >- (rpt conj_tac >> simp[]
-              >- (Cases_on`lopt`>>fs[LENGTH_REPLICATE,LENGTH_clos_gen])
-              >- (qx_gen_tac `i` >> reverse (Cases_on `i < LENGTH fns`) >>
-                  Cases_on`lopt`>> simp[LENGTH_REPLICATE,LENGTH_clos_gen]>>
-                  fs[LIST_REL_EL_EQN] >>
-                  simp[Abbr`ff`,EL_REPLICATE,EL_MAP] >>
-                  pairarg_tac >> simp[])
-              >- (fs[elglobals_EQ_EMPTY, MEM_MAP, PULL_EXISTS, FORALL_PROD] >>
-                  simp[Abbr`ff`] >> rpt strip_tac >>
-                  qmatch_abbrev_tac `
-                    set_globals (FST (HD (FST (known [_] ENV g0)))) = {||}` >>
-                  rename1 `MEM (nargs, fbody) fns` >>
-                  `set_globals fbody = {||}` by metis_tac[] >>
-                  Cases_on `known [fbody] ENV g0` >> simp[] >>
-                  imp_res_tac known_sing_EQ_E >> fs[] >> rveq >>
-                  first_x_assum (mp_tac o MATCH_MP known_preserves_setGlobals)>>
-                  simp[])))))
 
 val kca_sing_sga =
     known_correct_approx
@@ -1542,36 +3829,6 @@ val ksrel_subspt = Q.store_thm(
       metis_tac[kvrel_subspt])
   >- (irule fmap_rel_mono >> qexists_tac `ref_rel (kvrel g)` >> simp[] >>
       Cases >> simp[PULL_EXISTS] >> metis_tac[kvrel_LIST_REL_subspt]));
-
-val vsgc_free_Full_app_set_globals = Q.store_thm(
-  "vsgc_free_Full_app_set_globals",
-  `∀fval lopt args fe env args'.
-     vsgc_free fval ∧ EVERY vsgc_free args ∧
-     dest_closure max_app lopt fval args = SOME (Full_app fe env args')
-   ⇒
-     set_globals fe = {||} ∧ EVERY vsgc_free env ∧ EVERY vsgc_free args'`,
-  simp[dest_closure_def, v_case_eq, bool_case_eq] >> rpt strip_tac >> fs[]
-  >- (rveq >> simp[EVERY_REVERSE, EVERY_TAKE])
-  >- (rveq >> simp[EVERY_REVERSE, EVERY_DROP])
-  >- (pairarg_tac >> fs[bool_case_eq] >> rveq >>
-      fs[elglobals_EQ_EMPTY, MEM_MAP, PULL_EXISTS, FORALL_PROD,
-         NOT_LESS_EQUAL] >>
-      metis_tac[MEM_EL])
-  >- (pairarg_tac >> fs[bool_case_eq] >>
-      simp[EVERY_REVERSE, EVERY_TAKE, EVERY_GENLIST])
-  >- (pairarg_tac >> fs[bool_case_eq] >>
-      simp[EVERY_REVERSE, EVERY_DROP, EVERY_GENLIST]))
-
-val known_emptySetGlobals_unchanged_g = Q.store_thm(
-  "known_emptySetGlobals_unchanged_g",
-  `∀es as g0 alist g.
-     known es as g0 = (alist, g) ∧ elist_globals es = {||} ⇒
-     g = g0`,
-  ho_match_mp_tac known_ind >> simp[known_def] >> rpt strip_tac >>
-  rpt (pairarg_tac >> fs[]) >> imp_res_tac known_sing_EQ_E >> rveq >> fs[] >>
-  rveq >> fs[] >>
-  rename1 `known_op opn` >> Cases_on `opn` >>
-  fs[known_op_def, case_eq_thms, op_gbag_def, va_case_eq, bool_case_eq]);
 
 val krrel_better_subspt = Q.store_thm(
   "krrel_better_subspt",
@@ -2475,6 +4732,8 @@ compile_correct
 state_globals_approx_def
 clos_knownTheory.compile_def
 val_rel_def
+*)
+
 *)
 
 val _ = export_theory();
